format-version: 1.2
data-version: https://w3id.org/elmo/elmo/releases/2025-04-22/elmo-full.owl
idspace: dce http://purl.org/dc/elements/1.1/ 
idspace: dcterms http://purl.org/dc/terms/ 
idspace: doap http://usefulinc.com/ns/doap# 
idspace: foaf http://xmlns.com/foaf/0.1/ 
idspace: oboInOwl http://www.geneontology.org/formats/oboInOwl# 
ontology: https://w3id.org/elmo/elmo/elmo-full.owl
property_value: dcterms:description "None" xsd:string
property_value: dcterms:license https://creativecommons.org/public-domain/
property_value: dcterms:title "Ecolink Model Ontology (ELMO)" xsd:string
property_value: owl:versionInfo "2025-04-22" xsd:string

[Term]
id: BFO:0000015
name: process

[Term]
id: ELMO:0000000
name: root node

[Term]
id: ENVO:01001170
name: active ecosystem management process
def: "A process during which an ecosystem, its parts, or the processes it participates in are modified by human intervention to accomplish an objective." [https://www.iucn.org/theme/protected-areas/about/protected-areas-categories/category-iv-habitatspecies-management-area]
synonym: "ecosystem management" EXACT []
is_a: ENVO:02500000 ! environmental system process
relationship: RO:0002211 ENVO:02500000 ! environmental system process

[Term]
id: ENVO:01001436
name: planned environmental usage process
def: "A planned process during which humans access and obtain resources, benefits, or services from a natural or anthropised ecosystem." []
is_a: ENVO:02500000 ! environmental system process
relationship: BFO:0000051 ENVO:01001170 ! active ecosystem management process
created_by: https://orcid.org/0000-0002-4366-3088

[Term]
id: ENVO:02500000
name: environmental system process
def: "A process in which includes the components of an environmental system as participants." []
is_a: BFO:0000015 ! process

[Term]
id: elmo:3620020
name: mechanical ecosystem management process
def: "An active ecosystem management process during which a human employs machines or tools to directly impact an ecosystem and realize some ecosystem management goal." []
is_a: ENVO:01001170 ! active ecosystem management process
property_value: dcterms:contributor https://orcid.org/0000-0002-4366-3088
property_value: dcterms:contributor https://orcid.org/0000-0003-4817-0423
created_by: https://orcid.org/0000-0002-1296-2528

[Term]
id: elmo:3620021
name: mechanical vegetation removal process
def: "A mechanical ecosystem management process during which vegetation is removed." []
is_a: elmo:3620020 ! mechanical ecosystem management process
property_value: dcterms:contributor https://orcid.org/0000-0002-4366-3088
property_value: dcterms:contributor https://orcid.org/0000-0003-4817-0423
created_by: https://orcid.org/0000-0002-1296-2528

[Term]
id: elmo:3620022
name: root wrench removal process
def: "A mechanical vegetation removal process in which a human employs a tool comprising a lever and gripping portion (root wrench)." []
is_a: elmo:3620021 ! mechanical vegetation removal process
property_value: dcterms:contributor https://orcid.org/0000-0002-4366-3088
property_value: dcterms:contributor https://orcid.org/0000-0003-4817-0423
created_by: https://orcid.org/0000-0002-1296-2528

[Term]
id: elmo:3620023
name: cut and cover removal process
def: "A mechanical vegetation removal process during which plants at ground level are cut and residual stumps are covered with a sun-blocking material (e.g. silage tarp)." []
is_a: elmo:3620021 ! mechanical vegetation removal process
property_value: dcterms:contributor https://orcid.org/0000-0002-4366-3088
property_value: dcterms:contributor https://orcid.org/0000-0003-4817-0423
created_by: https://orcid.org/0000-0002-1296-2528

[Term]
id: elmo:3620024
name: cutting removal process
def: "A mechanical vegetation removal process in which a human cuts and removes plant material." []
is_a: elmo:3620021 ! mechanical vegetation removal process
property_value: dcterms:contributor https://orcid.org/0000-0002-4366-3088
property_value: dcterms:contributor https://orcid.org/0000-0003-4817-0423
created_by: https://orcid.org/0000-0002-1296-2528

[Term]
id: elmo:3620025
name: spading removal process
def: "A mechanical vegetation removal process in which a human severs subsoil roots using a spade and pries the plant out of the ground." [https://www.ontarioinvasiveplants.ca/wp-content/uploads/2018/05/OPWG-Spading-Postcard-1.pdf]
is_a: elmo:3620021 ! mechanical vegetation removal process
property_value: dcterms:contributor https://orcid.org/0000-0002-4366-3088
property_value: dcterms:contributor https://orcid.org/0000-0003-4817-0423
created_by: https://orcid.org/0000-0002-1296-2528

[Term]
id: elmo:3620026
name: canopy thinning process
def: "A mechanical vegetation removal process in which a human removes trees from a given area with the goal of reducing overall canopy cover thereby increasing light availability for understorey plants." [doi:10.1111/rec.13043]
is_a: elmo:3620021 ! mechanical vegetation removal process
property_value: dcterms:contributor https://orcid.org/0000-0002-4366-3088
property_value: dcterms:contributor https://orcid.org/0000-0003-4817-0423
created_by: https://orcid.org/0000-0002-1296-2528

[Term]
id: elmo:3620027
name: leaf litter removal process
def: "A mechanical vegetation removal process in which a human removes leaf litter from the ground thereby increasing the light availability for soil." []
is_a: elmo:3620021 ! mechanical vegetation removal process
property_value: dcterms:contributor https://orcid.org/0000-0002-4366-3088
property_value: dcterms:contributor https://orcid.org/0000-0003-4817-0423
created_by: https://orcid.org/0000-0002-1296-2528

[Term]
id: elmo:3620028
name: mechanical fauna control process
def: "A mechanical ecosystem management process in which a human controls fauna populations." []
is_a: elmo:3620020 ! mechanical ecosystem management process
property_value: dcterms:contributor https://orcid.org/0000-0002-4366-3088
property_value: dcterms:contributor https://orcid.org/0000-0003-4817-0423
created_by: https://orcid.org/0000-0002-1296-2528

[Term]
id: elmo:3620029
name: mammal trapping process
def: "A mechanical fauna control process in which a human uses traps to control fauna." [https://en.wikipedia.org/wiki/Trapping]
is_a: elmo:3620028 ! mechanical fauna control process
property_value: dcterms:contributor https://orcid.org/0000-0002-4366-3088
property_value: dcterms:contributor https://orcid.org/0000-0003-4817-0423
created_by: https://orcid.org/0000-0002-1296-2528

[Term]
id: elmo:3620030
name: predator control process
def: "A mechanical fauna control process in which a human targets predators for removal from the ecosystem." [https://agrilife.org/txwildlifeservices/files/2011/07/PredatorControlforWildlifeMgt.pdf]
is_a: elmo:3620028 ! mechanical fauna control process
property_value: dcterms:contributor https://orcid.org/0000-0002-4366-3088
property_value: dcterms:contributor https://orcid.org/0000-0003-4817-0423
created_by: https://orcid.org/0000-0002-1296-2528

[Term]
id: elmo:3620031
name: fencing process
def: "A mechanical fauna control process in which a human installs fencing to restrict either immigration or emmigration of fauna from a particular area." [doi:10.1016/j.biocon.2017.08.001]
is_a: elmo:3620067 ! fauna exclusion process
property_value: dcterms:contributor https://orcid.org/0000-0002-4366-3088
property_value: dcterms:contributor https://orcid.org/0000-0003-4817-0423
created_by: https://orcid.org/0000-0002-1296-2528

[Term]
id: elmo:3620032
name: mechanical species deterrent process
def: "A mechanical fauna control process in which a human installs an electronic device to deter species from a particular area." [doi:10.1111/jfb.13769]
is_a: elmo:3620028 ! mechanical fauna control process
property_value: dcterms:contributor https://orcid.org/0000-0002-4366-3088
property_value: dcterms:contributor https://orcid.org/0000-0003-4817-0423
created_by: https://orcid.org/0000-0002-1296-2528

[Term]
id: elmo:3620033
name: mechanical hydrological alteration process
def: "A mechanical ecosystem management process during which a human deliberately alters the hydrologic cycle in an area." [https://en.wikipedia.org/wiki/Water_cycle]
is_a: elmo:3620020 ! mechanical ecosystem management process
property_value: dcterms:contributor https://orcid.org/0000-0002-4366-3088
property_value: dcterms:contributor https://orcid.org/0000-0003-4817-0423
created_by: https://orcid.org/0000-0002-1296-2528

[Term]
id: elmo:3620034
name: dam construction process
def: "A mechanical hydrological alteration process in which a human constructs some dam to restore a meander sequence to a river or stream." [doi:10.1093/biosci/biu036]
synonym: "beaver dam analogue" EXACT []
is_a: elmo:3620033 ! mechanical hydrological alteration process
property_value: dcterms:contributor https://orcid.org/0000-0002-4366-3088
property_value: dcterms:contributor https://orcid.org/0000-0003-4817-0423
created_by: https://orcid.org/0000-0002-1296-2528

[Term]
id: elmo:3620035
name: dam removal process
def: "A mechanical hydrological alteration process in which a human removes some dam with the goal of altering the hydroperiod of surrounding lands and reconnecting rivers." [doi:10.12952/journal.elementa.000108]
is_a: elmo:3620033 ! mechanical hydrological alteration process
property_value: dcterms:contributor https://orcid.org/0000-0002-4366-3088
property_value: dcterms:contributor https://orcid.org/0000-0003-4817-0423
created_by: https://orcid.org/0000-0002-1296-2528

[Term]
id: elmo:3620036
name: tile drain crushing process
def: "A mechanical hydrological alteration process in which a human uncovers and collapses subterranean tile drains in situ to reduce drainage on the landscape and restore wetland hydroperiod." []
is_a: elmo:3620033 ! mechanical hydrological alteration process
property_value: dcterms:contributor https://orcid.org/0000-0002-4366-3088
property_value: dcterms:contributor https://orcid.org/0000-0003-4817-0423
property_value: IAO:0000116 "This technique is actively practiced by the Nature Conservancy of Canada, but has not been documented in the literature yet." xsd:string
created_by: https://orcid.org/0000-0002-1296-2528

[Term]
id: elmo:3620037
name: tile drain removal process
def: "A mechanical hydrological alteration process in which a human uncovers and removes subterranean tile drains to reduce drainage on the landscape and restore wetland hydroperiod." []
is_a: elmo:3620033 ! mechanical hydrological alteration process
property_value: dcterms:contributor https://orcid.org/0000-0002-4366-3088
property_value: dcterms:contributor https://orcid.org/0000-0003-4817-0423
created_by: https://orcid.org/0000-0002-1296-2528

[Term]
id: elmo:3620038
name: nest site creation process
def: "A mechanical ecosystem management process in which a human creates sites for fauna to breed, feed and shelter." [doi:10.1186/S41610-021-00192-Z]
is_a: elmo:3620020 ! mechanical ecosystem management process
property_value: dcterms:contributor https://orcid.org/0000-0002-4366-3088
property_value: dcterms:contributor https://orcid.org/0000-0003-4817-0423
created_by: https://orcid.org/0000-0002-1296-2528

[Term]
id: elmo:3620039
name: perch creation process
def: "A mechanical ecosystem management process in which a human creates places for birds to perch." [doi:10.1007/s11258-016-0619-4]
is_a: elmo:3620020 ! mechanical ecosystem management process
property_value: dcterms:contributor https://orcid.org/0000-0002-4366-3088
property_value: dcterms:contributor https://orcid.org/0000-0003-4817-0423
created_by: https://orcid.org/0000-0002-1296-2528

[Term]
id: elmo:3620040
name: buffer strip creation process
def: "A mechanical ecosystem management process in which a human cultivates strips of flora between landscape features using earthworks and planting processes." [doi:10.2134/jeq2018.03.0120]
is_a: elmo:3620020 ! mechanical ecosystem management process
property_value: dcterms:contributor https://orcid.org/0000-0002-4366-3088
property_value: dcterms:contributor https://orcid.org/0000-0003-4817-0423
created_by: https://orcid.org/0000-0002-1296-2528

[Term]
id: elmo:3620041
name: riparian buffer strip creation process
def: "A mechanical ecosystem management process in which a human cultivates strips of flora in the riparian areas of rivers." [doi:10.1890/08-2064.1]
is_a: elmo:3620040 ! buffer strip creation process
property_value: dcterms:contributor https://orcid.org/0000-0002-4366-3088
property_value: dcterms:contributor https://orcid.org/0000-0003-4817-0423
created_by: https://orcid.org/0000-0002-1296-2528

[Term]
id: elmo:3620042
name: buffer strip retention process
def: "A mechanical ecosystem management process in which a human leaves strips of flora untouched when clearing the land for other purposes." [doi:10.2134/jeq2018.03.0120]
is_a: elmo:3620020 ! mechanical ecosystem management process
property_value: dcterms:contributor https://orcid.org/0000-0002-4366-3088
property_value: dcterms:contributor https://orcid.org/0000-0003-4817-0423
created_by: https://orcid.org/0000-0002-1296-2528

[Term]
id: elmo:3620043
name: earthworks process
def: "A mechanical ecosystem management process during which the topology of some area is deliberately changed at least at the micro scale (e.g. 1m2)." []
is_a: elmo:3620020 ! mechanical ecosystem management process
property_value: dcterms:contributor https://orcid.org/0000-0002-4366-3088
property_value: dcterms:contributor https://orcid.org/0000-0003-4817-0423
property_value: IAO:0000116 "Difficult to suggest a firm border for scale. I doubt digging out a small hole would be called earthworks but settled on at least 1 m2 of earth moved. See Landscape Microscale Size and its associated scale properties for more nuance: ENVO:03620005; ENVO:03620006; ENVO:03620007; ENVO:03620008" xsd:string
created_by: https://orcid.org/0000-0002-1296-2528

[Term]
id: elmo:3620044
name: berm creation process
def: "An earthworks process in which earthen barriers (berms) are constructed with the goal of obstructing or slowing floodwaters." [doi:10.1007/s11273-013-9285-7]
is_a: elmo:3620043 ! earthworks process
property_value: dcterms:contributor https://orcid.org/0000-0002-4366-3088
property_value: dcterms:contributor https://orcid.org/0000-0003-4817-0423
created_by: https://orcid.org/0000-0002-1296-2528

[Term]
id: elmo:3620046
name: pond creation process
def: "An earthworks process in which a human creates a pond." [doi:10.1007/s10531-021-02312-6]
is_a: elmo:3620043 ! earthworks process
property_value: dcterms:contributor https://orcid.org/0000-0002-4366-3088
property_value: dcterms:contributor https://orcid.org/0000-0003-4817-0423
created_by: https://orcid.org/0000-0002-1296-2528

[Term]
id: elmo:3620047
name: pond reprofiling process
def: "An earthworks process in which a human reshapes the banks or basin of a pond." [doi:10.1016/j.jenvman.2024.120992]
is_a: elmo:3620043 ! earthworks process
property_value: dcterms:contributor https://orcid.org/0000-0002-4366-3088
property_value: dcterms:contributor https://orcid.org/0000-0003-4817-0423
created_by: https://orcid.org/0000-0002-1296-2528

[Term]
id: elmo:3620048
name: soil decompaction process
def: "An earthworks process in which a human alleviates the compaction of soil." [doi:10.1111/j.1526-100X.2008.00477.x]
is_a: elmo:3620043 ! earthworks process
property_value: dcterms:contributor https://orcid.org/0000-0002-4366-3088
property_value: dcterms:contributor https://orcid.org/0000-0003-4817-0423
created_by: https://orcid.org/0000-0002-1296-2528

[Term]
id: elmo:3620049
name: tilling process
def: "An earthworks process in which a human breaks up the soil, and sometimes adds organic matter." [doi:10.1111/j.1526-100X.1995.tb00096.x]
synonym: "soil ripping process" NARROW []
is_a: elmo:3620048 ! soil decompaction process
property_value: dcterms:contributor https://orcid.org/0000-0002-4366-3088
property_value: dcterms:contributor https://orcid.org/0000-0003-4817-0423
created_by: https://orcid.org/0000-0002-1296-2528

[Term]
id: elmo:3620050
name: ploughing process
def: "An earthworks process in which a human deeply breaks up and overturns soil and vegetation." [doi:10.1007/s12224-024-09448-7]
is_a: elmo:3620048 ! soil decompaction process
property_value: dcterms:contributor https://orcid.org/0000-0002-4366-3088
property_value: dcterms:contributor https://orcid.org/0000-0003-4817-0423
created_by: https://orcid.org/0000-0002-1296-2528

[Term]
id: elmo:3620052
name: grading process
def: "An earthworks process in which a human creates a specific slope." [https://en.wikipedia.org/wiki/Grading_(earthworks)]
is_a: elmo:3620043 ! earthworks process
property_value: dcterms:contributor https://orcid.org/0000-0002-4366-3088
property_value: dcterms:contributor https://orcid.org/0000-0003-4817-0423
created_by: https://orcid.org/0000-0002-1296-2528

[Term]
id: elmo:3620053
name: slope stabilization process
def: "An earthworks process in which a human installs inorganic material, usually a mesh, to stabilize a slope." [https://en.wikipedia.org/wiki/Cellular_confinement]
is_a: elmo:3620043 ! earthworks process
property_value: dcterms:contributor https://orcid.org/0000-0002-4366-3088
property_value: dcterms:contributor https://orcid.org/0000-0003-4817-0423
created_by: https://orcid.org/0000-0002-1296-2528

[Term]
id: elmo:3620054
name: shoreline reinforcement process
def: "An earthworks process in which a human installs inorganic material, usually in a mesh, to stabilize a slope on the bank of a body of water." [https://en.wikipedia.org/wiki/Cellular_confinement]
is_a: elmo:3620043 ! earthworks process
property_value: dcterms:contributor https://orcid.org/0000-0002-4366-3088
property_value: dcterms:contributor https://orcid.org/0000-0003-4817-0423
created_by: https://orcid.org/0000-0002-1296-2528

[Term]
id: elmo:3620055
name: pit and mound excavation process
def: "An earthworks process in which a human digs pits and creates mounds to reproduce a natural disturbance regime." [doi:10.1016/j.foreco.2017.02.048]
is_a: elmo:3620043 ! earthworks process
property_value: dcterms:contributor https://orcid.org/0000-0002-4366-3088
property_value: dcterms:contributor https://orcid.org/0000-0003-4817-0423
created_by: https://orcid.org/0000-0002-1296-2528

[Term]
id: elmo:3620056
name: channel realignment process
def: "An earthworks process in which a human realigns the channel of a stream by digging out replacement pathways and filling existing ones." [https://streamhandbook.org/project/stream-channel-realignment/]
is_a: elmo:3620043 ! earthworks process
property_value: dcterms:contributor https://orcid.org/0000-0002-4366-3088
property_value: dcterms:contributor https://orcid.org/0000-0003-4817-0423
created_by: https://orcid.org/0000-0002-1296-2528

[Term]
id: elmo:3620057
name: natural channel realignment process
def: "An earthworks process in which a human realigns the channel of a stream by digging out replacement pathways and filling existing ones with the goal of recreating a natural pool-riffle-pool meander sequence." [https://streamhandbook.org/project/stream-channel-realignment/]
is_a: elmo:3620056 ! channel realignment process
property_value: dcterms:contributor https://orcid.org/0000-0002-4366-3088
property_value: dcterms:contributor https://orcid.org/0000-0003-4817-0423
created_by: https://orcid.org/0000-0002-1296-2528

[Term]
id: elmo:3620058
name: dredging process
def: "An earthworks process in which a human removes the sediment layer of a water body." [https://en.wikipedia.org/wiki/Dredging]
is_a: elmo:3620043 ! earthworks process
property_value: dcterms:contributor https://orcid.org/0000-0002-4366-3088
property_value: dcterms:contributor https://orcid.org/0000-0003-4817-0423
created_by: https://orcid.org/0000-0002-1296-2528

[Term]
id: elmo:3620059
name: fauna passage creation process
def: "A mechanical ecosystem management process in which a human creates a crossing (bridge or underpass) to help fauna pass through a barrier such as a road, fence or property." [https://en.wikipedia.org/wiki/Wildlife_crossing]
is_a: elmo:3620020 ! mechanical ecosystem management process
property_value: dcterms:contributor https://orcid.org/0000-0002-4366-3088
property_value: dcterms:contributor https://orcid.org/0000-0003-4817-0423
created_by: https://orcid.org/0000-0002-1296-2528

[Term]
id: elmo:3620060
name: topsoil removal process
def: "A mechanical ecosystem management process in which a human removes the topsoil layer." [doi:10.1111/avsc.12063]
is_a: elmo:3620020 ! mechanical ecosystem management process
property_value: dcterms:contributor https://orcid.org/0000-0002-4366-3088
property_value: dcterms:contributor https://orcid.org/0000-0003-4817-0423
created_by: https://orcid.org/0000-0002-1296-2528

[Term]
id: elmo:3620061
name: erosion control process
def: "A mechanical ecosystem management process in which a human installs some material to reduce erosion." [https://en.wikipedia.org/wiki/Erosion_control]
is_a: elmo:3620043 ! earthworks process
property_value: dcterms:contributor https://orcid.org/0000-0002-4366-3088
property_value: dcterms:contributor https://orcid.org/0000-0003-4817-0423
created_by: https://orcid.org/0000-0002-1296-2528

[Term]
id: elmo:3620062
name: erosion blanket process
def: "An erosion control process in which a human installs a textile." []
is_a: elmo:3620061 ! erosion control process
property_value: dcterms:contributor https://orcid.org/0000-0002-4366-3088
property_value: dcterms:contributor https://orcid.org/0000-0003-4817-0423
created_by: https://orcid.org/0000-0002-1296-2528

[Term]
id: elmo:3620063
name: erosion fencing process
def: "An erosion control process in which a human installs a fence with a geotextile to restrict sediment transport." [https://en.wikipedia.org/wiki/Silt_fence]
is_a: elmo:3620061 ! erosion control process
property_value: dcterms:contributor https://orcid.org/0000-0002-4366-3088
property_value: dcterms:contributor https://orcid.org/0000-0003-4817-0423
created_by: https://orcid.org/0000-0002-1296-2528

[Term]
id: elmo:3620064
name: wattle fencing process
def: "An erosion control process in which a human interleaves live materials to make short fencing along a slope." [https://hatchetnseed.ca/soil-bio-engineering-for-erosion-control/]
is_a: elmo:3620061 ! erosion control process
property_value: dcterms:contributor https://orcid.org/0000-0002-4366-3088
property_value: dcterms:contributor https://orcid.org/0000-0003-4817-0423
created_by: https://orcid.org/0000-0002-1296-2528

[Term]
id: elmo:3620065
name: irrigation process
def: "A mechanical ecosystem management process in which a human installs semi-permanent lines to supply a controlled amount of water to plants." [https://en.wikipedia.org/wiki/Irrigation]
is_a: elmo:3620020 ! mechanical ecosystem management process
property_value: dcterms:contributor https://orcid.org/0000-0002-4366-3088
property_value: dcterms:contributor https://orcid.org/0000-0003-4817-0423
created_by: https://orcid.org/0000-0002-1296-2528

[Term]
id: elmo:3620066
name: deterrence-focused predator control process
def: "A predator control process in which a human installs a mechanical device designed to deter predators from a given area." []
is_a: elmo:3620030 ! predator control process
property_value: dcterms:contributor https://orcid.org/0000-0002-4366-3088
property_value: dcterms:contributor https://orcid.org/0000-0003-4817-0423
created_by: https://orcid.org/0000-0002-1296-2528

[Term]
id: elmo:3620067
name: fauna exclusion process
def: "A mechanical fauna control process in which a human excludes fauna from a specific area." []
is_a: elmo:3620028 ! mechanical fauna control process
property_value: dcterms:contributor https://orcid.org/0000-0002-4366-3088
property_value: dcterms:contributor https://orcid.org/0000-0003-4817-0423
created_by: https://orcid.org/0000-0002-1296-2528

[Term]
id: elmo:3620068
name: mechanical fauna deterrent process
def: "A mechanical fauna control process in which a human deters fauna from a specific area." []
is_a: elmo:3620028 ! mechanical fauna control process
property_value: dcterms:contributor https://orcid.org/0000-0002-4366-3088
property_value: dcterms:contributor https://orcid.org/0000-0003-4817-0423
created_by: https://orcid.org/0000-0002-1296-2528

[Term]
id: elmo:3620069
name: fauna capture for conservation
def: "A mechanical fauna control process in which a human captures fauna for the purposes of protecting existing organisms from some threat." []
is_a: elmo:3620028 ! mechanical fauna control process
property_value: dcterms:contributor https://orcid.org/0000-0002-4366-3088
property_value: dcterms:contributor https://orcid.org/0000-0003-4817-0423
created_by: https://orcid.org/0000-0002-1296-2528

[Term]
id: elmo:3620070
name: fish bypass installation process
def: "A mechanical ecosystem management process in which a human installs some means of bypassing hazards (e.g. dams) for fish." []
is_a: elmo:3620020 ! mechanical ecosystem management process
property_value: dcterms:contributor https://orcid.org/0000-0002-4366-3088
property_value: dcterms:contributor https://orcid.org/0000-0003-4817-0423
created_by: https://orcid.org/0000-0002-1296-2528

[Term]
id: elmo:3620071
name: fish ladder installation process
def: "A fish bypass installation process in which a human installs a chute consisting of a series of stepped pools to allow fish to move past a dam." [https://oceanservice.noaa.gov/facts/fish-ladder.html]
is_a: elmo:3620070 ! fish bypass installation process
property_value: dcterms:contributor https://orcid.org/0000-0002-4366-3088
property_value: dcterms:contributor https://orcid.org/0000-0003-4817-0423
created_by: https://orcid.org/0000-0002-1296-2528

[Term]
id: elmo:3620072
name: ditch plugging process
def: "An earthworks process in which a human fills in a drainage ditch to restore the hydroperiod to a given area." [https://www.ducks.ca/stories/biodiversity/years-in-the-making-for-record-breaking-conservation-project/]
is_a: elmo:3620043 ! earthworks process
property_value: dcterms:contributor https://orcid.org/0000-0002-4366-3088
property_value: dcterms:contributor https://orcid.org/0000-0003-4817-0423
created_by: https://orcid.org/0000-0002-1296-2528

[Term]
id: elmo:3620073
name: sediment addition process
def: "An earthworks process in which a human adds sediment to a water body in order to modify the substrate composition." []
is_a: elmo:3620043 ! earthworks process
property_value: dcterms:contributor https://orcid.org/0000-0002-4366-3088
property_value: dcterms:contributor https://orcid.org/0000-0003-4817-0423
created_by: https://orcid.org/0000-0002-1296-2528

[Term]
id: elmo:3620074
name: new plant protection process
def: "A mechanical ecosystem management process in which a human installs a barrier to protect newly planted flora from herbivory." []
is_a: elmo:3620020 ! mechanical ecosystem management process
property_value: dcterms:contributor https://orcid.org/0000-0002-4366-3088
property_value: dcterms:contributor https://orcid.org/0000-0003-4817-0423
created_by: https://orcid.org/0000-0002-1296-2528

[Term]
id: elmo:3620500
name: chemical ecosystem management process
def: "An active ecosystem management process in which a human applys or releases a chemical substance to realize some ecological management goal." [doi:10.1016/j.scitotenv.2021.148631]
is_a: ENVO:01001170 ! active ecosystem management process
property_value: dcterms:contributor https://orcid.org/0000-0002-4366-3088
property_value: dcterms:contributor https://orcid.org/0000-0003-4817-0423
created_by: https://orcid.org/0000-0002-1296-2528

[Term]
id: elmo:3620501
name: chemical application process
def: "A chemical ecosystem management process in which a human applies some chemical to an ecosystem." [doi:10.1016/j.scitotenv.2021.148631]
is_a: elmo:3620500 ! chemical ecosystem management process
property_value: dcterms:contributor https://orcid.org/0000-0002-4366-3088
property_value: dcterms:contributor https://orcid.org/0000-0003-4817-0423
created_by: https://orcid.org/0000-0002-1296-2528

[Term]
id: elmo:3620502
name: fertilizer application process
def: "A chemical application process in which a human applies chemical fertilizer to a given area with the goal of increasing the available carbon, nitrogen or phosphorous." [wd:Q1213511]
is_a: elmo:3620501 ! chemical application process
property_value: dcterms:contributor https://orcid.org/0000-0002-4366-3088
property_value: dcterms:contributor https://orcid.org/0000-0003-4817-0423
created_by: https://orcid.org/0000-0002-1296-2528

[Term]
id: elmo:3620503
name: lime application process
def: "A chemical application process in which a human adds lime to soil or water in order to reduce the pH." [doi:10.1046/j.1365-2427.2001.00788.x]
is_a: elmo:3620501 ! chemical application process
property_value: dcterms:contributor https://orcid.org/0000-0002-4366-3088
property_value: dcterms:contributor https://orcid.org/0000-0003-4817-0423
created_by: https://orcid.org/0000-0002-1296-2528

[Term]
id: elmo:3620504
name: herbicide application process
def: "A chemical application process in which a human applies herbicide to plants or soil in a given area." [doi:10.1111/avsc.12183]
is_a: elmo:3620501 ! chemical application process
property_value: dcterms:contributor https://orcid.org/0000-0002-4366-3088
property_value: dcterms:contributor https://orcid.org/0000-0003-4817-0423
created_by: https://orcid.org/0000-0002-1296-2528

[Term]
id: elmo:3620505
name: glyphosate application process
def: "A herbicide application process in which a human applies the herbicide glyphosate to plants in some area." [doi:10.1111/avsc.12183]
is_a: elmo:3620501 ! chemical application process
property_value: dcterms:contributor https://orcid.org/0000-0002-4366-3088
property_value: dcterms:contributor https://orcid.org/0000-0003-4817-0423
created_by: https://orcid.org/0000-0002-1296-2528

[Term]
id: elmo:3620506
name: insecticide application process
def: "A chemical application process in which a human introduces an insecticide to some area with the goal of managing an insect population." [doi:10.1016/j.biocontrol.2018.07.012]
is_a: elmo:3620501 ! chemical application process
property_value: dcterms:contributor https://orcid.org/0000-0002-4366-3088
property_value: dcterms:contributor https://orcid.org/0000-0003-4817-0423
created_by: https://orcid.org/0000-0002-1296-2528

[Term]
id: elmo:3620600
name: biological ecosystem management process
def: "An active ecosystem management process in which a human adds or removes biological material from an area to realize some ecological management goal." []
is_a: ENVO:01001170 ! active ecosystem management process
property_value: dcterms:contributor https://orcid.org/0000-0002-4366-3088
property_value: dcterms:contributor https://orcid.org/0000-0003-4817-0423
created_by: https://orcid.org/0000-0002-1296-2528

[Term]
id: elmo:3620601
name: planting process
def: "A biological ecosystem management process in which a human plants flora (defined as at least having sprouted true leaves) in the soil of a given area." []
is_a: elmo:3620600 ! biological ecosystem management process
property_value: dcterms:contributor https://orcid.org/0000-0002-4366-3088
property_value: dcterms:contributor https://orcid.org/0000-0003-4817-0423
created_by: https://orcid.org/0000-0002-1296-2528

[Term]
id: elmo:3620602
name: plug planting process
def: "A planting process in which a human plants flora grown in a plug tray." [doi:10.1111/j.1526-100X.2007.00350.x]
is_a: elmo:3620601 ! planting process
property_value: dcterms:contributor https://orcid.org/0000-0002-4366-3088
property_value: dcterms:contributor https://orcid.org/0000-0003-4817-0423
created_by: https://orcid.org/0000-0002-1296-2528

[Term]
id: elmo:3620603
name: shrub planting process
def: "A planting process in which a human plants shrubs." []
is_a: elmo:3620601 ! planting process
property_value: dcterms:contributor https://orcid.org/0000-0002-4366-3088
property_value: dcterms:contributor https://orcid.org/0000-0003-4817-0423
created_by: https://orcid.org/0000-0002-1296-2528

[Term]
id: elmo:3620604
name: tree planting process
def: "A planting process in which a human plants trees." []
is_a: elmo:3620601 ! planting process
property_value: dcterms:contributor https://orcid.org/0000-0002-4366-3088
property_value: dcterms:contributor https://orcid.org/0000-0003-4817-0423
created_by: https://orcid.org/0000-0002-1296-2528

[Term]
id: elmo:3620605
name: seedling planting process
def: "A planting process in which a human plants trees that have been grown in plug trays." []
is_a: elmo:3620604 ! tree planting process
property_value: dcterms:contributor https://orcid.org/0000-0002-4366-3088
property_value: dcterms:contributor https://orcid.org/0000-0003-4817-0423
created_by: https://orcid.org/0000-0002-1296-2528

[Term]
id: elmo:3620606
name: caliper tree planting process
def: "A planting process in which a human plants trees that have grown to a diameter greater than 5 cm." []
is_a: elmo:3620604 ! tree planting process
property_value: dcterms:contributor https://orcid.org/0000-0002-4366-3088
property_value: dcterms:contributor https://orcid.org/0000-0003-4817-0423
created_by: https://orcid.org/0000-0002-1296-2528

[Term]
id: elmo:3620607
name: live staking process
def: "A planting process in which a human inserts cut branches of a flora into soil such that that flora will take root and grow." []
is_a: elmo:3620601 ! planting process
property_value: dcterms:contributor https://orcid.org/0000-0002-4366-3088
property_value: dcterms:contributor https://orcid.org/0000-0003-4817-0423
created_by: https://orcid.org/0000-0002-1296-2528

[Term]
id: elmo:3620608
name: nurse plant process
def: "A planting process in which a human plants flora with the goal of assisting the growth of other flora." [doi:10.1890/03-5084]
is_a: elmo:3620601 ! planting process
property_value: dcterms:contributor https://orcid.org/0000-0002-4366-3088
property_value: dcterms:contributor https://orcid.org/0000-0003-4817-0423
created_by: https://orcid.org/0000-0002-1296-2528

[Term]
id: elmo:3620609
name: seeding process
def: "A biological ecosystem management process in which a human sows seeds in a particular area." []
is_a: elmo:3620600 ! biological ecosystem management process
property_value: dcterms:contributor https://orcid.org/0000-0002-4366-3088
property_value: dcterms:contributor https://orcid.org/0000-0003-4817-0423
created_by: https://orcid.org/0000-0002-1296-2528

[Term]
id: elmo:3620610
name: tree seeding process
def: "A seeding process in which a human sows tree seeds." []
is_a: elmo:3620609 ! seeding process
property_value: dcterms:contributor https://orcid.org/0000-0002-4366-3088
property_value: dcterms:contributor https://orcid.org/0000-0003-4817-0423
created_by: https://orcid.org/0000-0002-1296-2528

[Term]
id: elmo:3620611
name: line seeding process
def: "A seeding process in which a human sows seeds in lines along a landscape." []
is_a: elmo:3620609 ! seeding process
property_value: dcterms:contributor https://orcid.org/0000-0002-4366-3088
property_value: dcterms:contributor https://orcid.org/0000-0003-4817-0423
created_by: https://orcid.org/0000-0002-1296-2528

[Term]
id: elmo:3620612
name: drill seeding process
def: "A seeding process in which a human uses a drill seeder to sow seeds." [doi:10.3375/043.038.0504]
is_a: elmo:3620609 ! seeding process
property_value: dcterms:contributor https://orcid.org/0000-0002-4366-3088
property_value: dcterms:contributor https://orcid.org/0000-0003-4817-0423
created_by: https://orcid.org/0000-0002-1296-2528

[Term]
id: elmo:3620613
name: broadcast seeding process
def: "A seeding process in which a human sows seeds by scattering them through the air." [doi:10.3375/043.038.0504]
is_a: elmo:3620609 ! seeding process
property_value: dcterms:contributor https://orcid.org/0000-0002-4366-3088
property_value: dcterms:contributor https://orcid.org/0000-0003-4817-0423
created_by: https://orcid.org/0000-0002-1296-2528

[Term]
id: elmo:3620614
name: hand broadcast seeding process
def: "A seeding process in which a human scatters seeds by hand." [doi:10.1111/j.1526-100X.2007.00350.x]
is_a: elmo:3620613 ! broadcast seeding process
property_value: dcterms:contributor https://orcid.org/0000-0002-4366-3088
property_value: dcterms:contributor https://orcid.org/0000-0003-4817-0423
created_by: https://orcid.org/0000-0002-1296-2528

[Term]
id: elmo:3620615
name: hydroseeding process
def: "A seeding process in which a human applies seed in a slurry of nutrients and fixatives." [doi:10.3375/043.038.0504]
is_a: elmo:3620609 ! seeding process
property_value: dcterms:contributor https://orcid.org/0000-0002-4366-3088
property_value: dcterms:contributor https://orcid.org/0000-0003-4817-0423
created_by: https://orcid.org/0000-0002-1296-2528

[Term]
id: elmo:3620616
name: seed treatment process
def: "A biological ecosystem management process in which a human applies a treatment to seed prior to sowing it." [doi:10.1111/rec.13210]
is_a: elmo:3620600 ! biological ecosystem management process
property_value: dcterms:contributor https://orcid.org/0000-0002-4366-3088
property_value: dcterms:contributor https://orcid.org/0000-0003-4817-0423
created_by: https://orcid.org/0000-0002-1296-2528

[Term]
id: elmo:3620617
name: seed scarification process
def: "A seed treatment process in which a human damages the coating of the seed, usually using sandpaper, to enhance germination." [doi:10.1111/rec.13210]
is_a: elmo:3620616 ! seed treatment process
property_value: dcterms:contributor https://orcid.org/0000-0002-4366-3088
property_value: dcterms:contributor https://orcid.org/0000-0003-4817-0423
created_by: https://orcid.org/0000-0002-1296-2528

[Term]
id: elmo:3620618
name: heat seed treatment process
def: "A seed treatment process in which a human applies heat to some seed in order to enhance germination." [doi:10.1111/rec.13210]
is_a: elmo:3620616 ! seed treatment process
property_value: dcterms:contributor https://orcid.org/0000-0002-4366-3088
property_value: dcterms:contributor https://orcid.org/0000-0003-4817-0423
created_by: https://orcid.org/0000-0002-1296-2528

[Term]
id: elmo:3620619
name: chill seed treatment process
def: "A seed treatment process in which a human applies cold to some seed in order to enhance germination, such as in cold stratification." [doi:10.1111/rec.13210]
is_a: elmo:3620616 ! seed treatment process
property_value: dcterms:contributor https://orcid.org/0000-0002-4366-3088
property_value: dcterms:contributor https://orcid.org/0000-0003-4817-0423
created_by: https://orcid.org/0000-0002-1296-2528

[Term]
id: elmo:3620620
name: soak seed treatment process
def: "A seed treatment process in which a human soaks seeds in order to enhance germination." [doi:10.1111/rec.13210]
is_a: elmo:3620616 ! seed treatment process
property_value: dcterms:contributor https://orcid.org/0000-0002-4366-3088
property_value: dcterms:contributor https://orcid.org/0000-0003-4817-0423
created_by: https://orcid.org/0000-0002-1296-2528

[Term]
id: elmo:3620621
name: light seed treatment process
def: "A seed treatment process in which light is applied to seeds in order to enhance germination." [doi:10.1111/rec.13210]
is_a: elmo:3620616 ! seed treatment process
property_value: dcterms:contributor https://orcid.org/0000-0002-4366-3088
property_value: dcterms:contributor https://orcid.org/0000-0003-4817-0423
created_by: https://orcid.org/0000-0002-1296-2528

[Term]
id: elmo:3620622
name: chemical seed treatment process
def: "A seed treatment process in which some chemical is applied to some seed in order to enhance germination." [doi:10.1111/rec.13210]
is_a: elmo:3620616 ! seed treatment process
property_value: dcterms:contributor https://orcid.org/0000-0002-4366-3088
property_value: dcterms:contributor https://orcid.org/0000-0003-4817-0423
created_by: https://orcid.org/0000-0002-1296-2528

[Term]
id: elmo:3620623
name: biological fauna control process
def: "A biological ecosystem management process in which a human uses biological means to reduce or increase a population of fauna." []
is_a: elmo:3620600 ! biological ecosystem management process
property_value: dcterms:contributor https://orcid.org/0000-0002-4366-3088
property_value: dcterms:contributor https://orcid.org/0000-0003-4817-0423
created_by: https://orcid.org/0000-0002-1296-2528

[Term]
id: elmo:3620624
name: captive breeding and release process
def: "A biological ecosystem management process in which a human facilitates the breeding of fauna, rears the young for a period of time and releases them in some environment." [doi:10.1111/j.1523-1739.2008.00967.x]
is_a: elmo:3620600 ! biological ecosystem management process
property_value: dcterms:contributor https://orcid.org/0000-0002-4366-3088
property_value: dcterms:contributor https://orcid.org/0000-0003-4817-0423
created_by: https://orcid.org/0000-0002-1296-2528

[Term]
id: elmo:3620625
name: egg relocation and release process
def: "A captive breeding and release process in which a human collects eggs and relocates them to a safe environment, whereupon they are allowed to hatch." []
is_a: elmo:3620624 ! captive breeding and release process
property_value: dcterms:contributor https://orcid.org/0000-0002-4366-3088
property_value: dcterms:contributor https://orcid.org/0000-0003-4817-0423
created_by: https://orcid.org/0000-0002-1296-2528

[Term]
id: elmo:3620626
name: egg incubation and release process
def: "An egg relocation and release process in which a human collects eggs and relocates them into an incubator, whereupon they are allowed to hatch and released into some environment." []
is_a: elmo:3620625 ! egg relocation and release process
property_value: dcterms:contributor https://orcid.org/0000-0002-4366-3088
property_value: dcterms:contributor https://orcid.org/0000-0003-4817-0423
created_by: https://orcid.org/0000-0002-1296-2528

[Term]
id: elmo:3620627
name: young capture, rearing and release
def: "A captive breeding and release process in which a human captures young fauna, rears them into adulthood and releases them into some environment." []
is_a: elmo:3620624 ! captive breeding and release process
property_value: dcterms:contributor https://orcid.org/0000-0002-4366-3088
property_value: dcterms:contributor https://orcid.org/0000-0003-4817-0423
created_by: https://orcid.org/0000-0002-1296-2528

[Term]
id: elmo:3620628
name: supplemental water process
def: "A biological ecosystem management process in which a human provides supplemental water to flora or fauna." []
is_a: elmo:3620600 ! biological ecosystem management process
property_value: dcterms:contributor https://orcid.org/0000-0002-4366-3088
property_value: dcterms:contributor https://orcid.org/0000-0003-4817-0423
created_by: https://orcid.org/0000-0002-1296-2528

[Term]
id: elmo:3620629
name: supplemental feeding process
def: "A biological ecosystem management process in which a human provides supplemental food to fauna." []
is_a: elmo:3620600 ! biological ecosystem management process
property_value: dcterms:contributor https://orcid.org/0000-0002-4366-3088
property_value: dcterms:contributor https://orcid.org/0000-0003-4817-0423
created_by: https://orcid.org/0000-0002-1296-2528

[Term]
id: elmo:3620630
name: plant material transfer process
def: "A biological ecosystem management process in which a human transfers plant material from some area to another." []
is_a: elmo:3620600 ! biological ecosystem management process
property_value: dcterms:contributor https://orcid.org/0000-0002-4366-3088
property_value: dcterms:contributor https://orcid.org/0000-0003-4817-0423
created_by: https://orcid.org/0000-0002-1296-2528

[Term]
id: elmo:3620631
name: moss layer transfer process
def: "A plant material transfer process in which a human restores the hydroperiod of a peatland by blocking drainage ditches or other means and subsequently moves material from the moss layer (top 10 cm) of another peatland onto the one being restored." [doi:10.1016/j.ecoleng.2014.03.051]
is_a: elmo:3620630 ! plant material transfer process
property_value: dcterms:contributor https://orcid.org/0000-0002-4366-3088
property_value: dcterms:contributor https://orcid.org/0000-0003-4817-0423
created_by: https://orcid.org/0000-0002-1296-2528

[Term]
id: elmo:3620632
name: soil transfer process
def: "A biological ecosystem management process in which a human transfers soil from one area to another." []
is_a: elmo:3620600 ! biological ecosystem management process
property_value: dcterms:contributor https://orcid.org/0000-0002-4366-3088
property_value: dcterms:contributor https://orcid.org/0000-0003-4817-0423
created_by: https://orcid.org/0000-0002-1296-2528

[Term]
id: elmo:3620633
name: fauna sterilization process
def: "A biological fauna control process in which a human renders some fauna sterile in order to reduce their population." []
is_a: elmo:3620623 ! biological fauna control process
property_value: dcterms:contributor https://orcid.org/0000-0002-4366-3088
property_value: dcterms:contributor https://orcid.org/0000-0003-4817-0423
created_by: https://orcid.org/0000-0002-1296-2528

[Term]
id: elmo:3620634
name: egg destruction process
def: "A biological fauna control process in which a human destroys the eggs of some fauna (e.g. oiling goose eggs)." []
is_a: elmo:3620623 ! biological fauna control process
property_value: dcterms:contributor https://orcid.org/0000-0002-4366-3088
property_value: dcterms:contributor https://orcid.org/0000-0003-4817-0423
created_by: https://orcid.org/0000-0002-1296-2528

[Term]
id: elmo:3620635
name: nest establishment deterrence process
def: "A biological ecosystem management process in which a human implements measures to deter fauna from establishing nest sites in a given area." []
is_a: elmo:3620623 ! biological fauna control process
property_value: dcterms:contributor https://orcid.org/0000-0002-4366-3088
property_value: dcterms:contributor https://orcid.org/0000-0003-4817-0423
created_by: https://orcid.org/0000-0002-1296-2528

[Term]
id: elmo:3620636
name: seabed amendment process
def: "A biological ecosystem management process in which a human adds material to a seabed to facilitate nesting." []
is_a: elmo:3620600 ! biological ecosystem management process
property_value: dcterms:contributor https://orcid.org/0000-0002-4366-3088
property_value: dcterms:contributor https://orcid.org/0000-0003-4817-0423
created_by: https://orcid.org/0000-0002-1296-2528

[Term]
id: elmo:3620637
name: soil amendment process
def: "A biological ecosystem management process in which a human adds some material to soil." [doi:10.2134/jeq2015.01.0009]
is_a: elmo:3620600 ! biological ecosystem management process
property_value: dcterms:contributor https://orcid.org/0000-0002-4366-3088
property_value: dcterms:contributor https://orcid.org/0000-0003-4817-0423
created_by: https://orcid.org/0000-0002-1296-2528

[Term]
id: elmo:3620638
name: mulch addition process
def: "A soil amendment process in which a human adds mulch (i.e. woody debris)." []
is_a: elmo:3620637 ! soil amendment process
property_value: dcterms:contributor https://orcid.org/0000-0002-4366-3088
property_value: dcterms:contributor https://orcid.org/0000-0003-4817-0423
created_by: https://orcid.org/0000-0002-1296-2528

[Term]
id: elmo:3620639
name: peat addition process
def: "A soil amendment process in which a human adds peat." []
is_a: elmo:3620637 ! soil amendment process
property_value: dcterms:contributor https://orcid.org/0000-0002-4366-3088
property_value: dcterms:contributor https://orcid.org/0000-0003-4817-0423
created_by: https://orcid.org/0000-0002-1296-2528

[Term]
id: elmo:3620640
name: topsoil addition process
def: "A soil amendment process in which a human adds topsoil." []
is_a: elmo:3620637 ! soil amendment process
property_value: dcterms:contributor https://orcid.org/0000-0002-4366-3088
property_value: dcterms:contributor https://orcid.org/0000-0003-4817-0423
created_by: https://orcid.org/0000-0002-1296-2528

[Term]
id: elmo:3620641
name: compost addition process
def: "A soil amendment process in which a human adds some composted organic material." [doi:10.2134/jeq2015.01.0009]
is_a: elmo:3620637 ! soil amendment process
property_value: dcterms:contributor https://orcid.org/0000-0002-4366-3088
property_value: dcterms:contributor https://orcid.org/0000-0003-4817-0423
created_by: https://orcid.org/0000-0002-1296-2528

[Term]
id: elmo:3620642
name: manure addition process
def: "A soil amendment process in which a human adds some manure." [doi:10.2134/jeq2015.01.0009]
is_a: elmo:3620637 ! soil amendment process
property_value: dcterms:contributor https://orcid.org/0000-0002-4366-3088
property_value: dcterms:contributor https://orcid.org/0000-0003-4817-0423
created_by: https://orcid.org/0000-0002-1296-2528

[Term]
id: elmo:3620643
name: artificial reef creation process
def: "A biological ecosystem management process in which a human creates an artificial reef out of materials with the goal of attracting coral." [doi:10.1111/1365-2664.13748]
is_a: elmo:3620600 ! biological ecosystem management process
property_value: dcterms:contributor https://orcid.org/0000-0002-4366-3088
property_value: dcterms:contributor https://orcid.org/0000-0003-4817-0423
created_by: https://orcid.org/0000-0002-1296-2528

[Term]
id: elmo:3620644
name: intentional grazing
def: "A biological ecosystem management process in which a human introduces grazing animals to an area with the goal of recreating a disturbance regime." [doi:10.1111/j.1526-100X.2009.00567.x]
is_a: elmo:3620600 ! biological ecosystem management process
property_value: dcterms:contributor https://orcid.org/0000-0002-4366-3088
property_value: dcterms:contributor https://orcid.org/0000-0003-4817-0423
created_by: https://orcid.org/0000-0002-1296-2528

[Term]
id: elmo:3620645
name: mycorrhizae addition process
def: "A biological ecosystem management process in which a human adds mycorrhizae spores to some environment." [doi:10.3389/fmicb.2016.01095]
is_a: elmo:3620600 ! biological ecosystem management process
property_value: dcterms:contributor https://orcid.org/0000-0002-4366-3088
property_value: dcterms:contributor https://orcid.org/0000-0003-4817-0423
created_by: https://orcid.org/0000-0002-1296-2528

[Term]
id: elmo:3620646
name: peatland rewetting process
def: "A biological ecosystem management process in which a human alters the hydroperiod of a peatland such that more water is available." [doi:10.1007/s11027-023-10046-9]
is_a: elmo:3620600 ! biological ecosystem management process
property_value: dcterms:contributor https://orcid.org/0000-0002-4366-3088
property_value: dcterms:contributor https://orcid.org/0000-0003-4817-0423
created_by: https://orcid.org/0000-0002-1296-2528

[Term]
id: elmo:3620647
name: fauna rescue, rehabilitation and release process
def: "A biological fauna control process in which a human captures injured fauna from some environment, rehabilitates and releases them." [doi:10.1371/journal.pone.0265514]
is_a: elmo:3620623 ! biological fauna control process
property_value: dcterms:contributor https://orcid.org/0000-0002-4366-3088
property_value: dcterms:contributor https://orcid.org/0000-0003-4817-0423
created_by: https://orcid.org/0000-0002-1296-2528

[Term]
id: elmo:3620648
name: fauna reintroduction process
def: "A biological fauna control process in which a human reintroduces fauna into some environment where the fauna once existed." []
is_a: elmo:3620623 ! biological fauna control process
property_value: dcterms:contributor https://orcid.org/0000-0002-4366-3088
property_value: dcterms:contributor https://orcid.org/0000-0003-4817-0423
created_by: https://orcid.org/0000-0002-1296-2528

[Term]
id: elmo:3620649
name: fauna medical care process
def: "A biological fauna control process in which a human provides medical care to some fauna." []
is_a: elmo:3620623 ! biological fauna control process
property_value: dcterms:contributor https://orcid.org/0000-0002-4366-3088
property_value: dcterms:contributor https://orcid.org/0000-0003-4817-0423
created_by: https://orcid.org/0000-0002-1296-2528

[Term]
id: elmo:3620650
name: translocation process
def: "A biological ecosystem management process in which a human translocates some flora or fauna from one area to another." []
is_a: elmo:3620600 ! biological ecosystem management process
property_value: dcterms:contributor https://orcid.org/0000-0002-4366-3088
property_value: dcterms:contributor https://orcid.org/0000-0003-4817-0423
created_by: https://orcid.org/0000-0002-1296-2528

[Term]
id: elmo:3620651
name: fauna translocation process
def: "A translocation process in which a human translocates some fauna from one area to another." []
is_a: elmo:3620650 ! translocation process
property_value: dcterms:contributor https://orcid.org/0000-0002-4366-3088
property_value: dcterms:contributor https://orcid.org/0000-0003-4817-0423
created_by: https://orcid.org/0000-0002-1296-2528

[Term]
id: elmo:3620652
name: coral translocation process
def: "A translocation process in which a human translocates coral from one area to another." [doi:10.3389/fmars.2019.00540]
is_a: elmo:3620650 ! translocation process
property_value: dcterms:contributor https://orcid.org/0000-0002-4366-3088
property_value: dcterms:contributor https://orcid.org/0000-0003-4817-0423
created_by: https://orcid.org/0000-0002-1296-2528

[Term]
id: elmo:3620800
name: ecosystem-oriented social process
def: "An environmental system process in which a human employs social means to realize some ecosystem management goal." []
is_a: ENVO:02500000 ! environmental system process
property_value: dcterms:contributor https://orcid.org/0000-0002-4366-3088
property_value: dcterms:contributor https://orcid.org/0000-0003-4817-0423
created_by: https://orcid.org/0000-0002-1296-2528

[Term]
id: elmo:3620801
name: legislation process
def: "A ecosystem-oriented social process in which a humans collectively implement legislation with pro-environmental goals." []
is_a: elmo:3620800 ! ecosystem-oriented social process
property_value: dcterms:contributor https://orcid.org/0000-0002-4366-3088
property_value: dcterms:contributor https://orcid.org/0000-0003-4817-0423
created_by: https://orcid.org/0000-0002-1296-2528

[Term]
id: elmo:3620802
name: legal protection process
def: "A legislation process in which the legislation explicitly protects something from degradation." []
is_a: elmo:3620801 ! legislation process
property_value: dcterms:contributor https://orcid.org/0000-0002-4366-3088
property_value: dcterms:contributor https://orcid.org/0000-0003-4817-0423
created_by: https://orcid.org/0000-0002-1296-2528

[Term]
id: elmo:3620803
name: legal habitat protection process
def: "A legal protection process in which the legal protection applies to a specific habitat." []
is_a: elmo:3620802 ! legal protection process
property_value: dcterms:contributor https://orcid.org/0000-0002-4366-3088
property_value: dcterms:contributor https://orcid.org/0000-0003-4817-0423
created_by: https://orcid.org/0000-0002-1296-2528

[Term]
id: elmo:3620804
name: legal landscape protection process
def: "A legal protection process in which the legal protection applies to a specific landscape." []
is_a: elmo:3620802 ! legal protection process
property_value: dcterms:contributor https://orcid.org/0000-0002-4366-3088
property_value: dcterms:contributor https://orcid.org/0000-0003-4817-0423
created_by: https://orcid.org/0000-0002-1296-2528

[Term]
id: elmo:3620805
name: legal species protection process
def: "A legal protection process in which the legal protection applies to some taxa." []
is_a: elmo:3620802 ! legal protection process
property_value: dcterms:contributor https://orcid.org/0000-0002-4366-3088
property_value: dcterms:contributor https://orcid.org/0000-0003-4817-0423
created_by: https://orcid.org/0000-0002-1296-2528

[Term]
id: elmo:3620806
name: legal marine area protection process
def: "A legal protection process in which the legal protection applies to some marine area." []
is_a: elmo:3620802 ! legal protection process
property_value: dcterms:contributor https://orcid.org/0000-0002-4366-3088
property_value: dcterms:contributor https://orcid.org/0000-0003-4817-0423
created_by: https://orcid.org/0000-0002-1296-2528

[Term]
id: elmo:3620807
name: private land protection process
def: "A legal protection process in which the legal protection applies to some privately held land." []
is_a: elmo:3620802 ! legal protection process
property_value: dcterms:contributor https://orcid.org/0000-0002-4366-3088
property_value: dcterms:contributor https://orcid.org/0000-0003-4817-0423
created_by: https://orcid.org/0000-0002-1296-2528

[Term]
id: elmo:3620808
name: conservation easement process
def: "A private land protection process in which a landowner agrees to conserve a portion of their land in perpetuity." []
is_a: elmo:3620807 ! private land protection process
property_value: dcterms:contributor https://orcid.org/0000-0002-4366-3088
property_value: dcterms:contributor https://orcid.org/0000-0003-4817-0423
created_by: https://orcid.org/0000-0002-1296-2528

[Term]
id: elmo:3620809
name: area policy process
def: "A legislation process in which some legislation applies to some area." []
is_a: elmo:3620801 ! legislation process
property_value: dcterms:contributor https://orcid.org/0000-0002-4366-3088
property_value: dcterms:contributor https://orcid.org/0000-0003-4817-0423
created_by: https://orcid.org/0000-0002-1296-2528

[Term]
id: elmo:3620810
name: local bylaw process
def: "An area policy process in which some pro-conservation bylaw is established by a local authority." []
is_a: elmo:3620809 ! area policy process
property_value: dcterms:contributor https://orcid.org/0000-0002-4366-3088
property_value: dcterms:contributor https://orcid.org/0000-0003-4817-0423
created_by: https://orcid.org/0000-0002-1296-2528

[Term]
id: elmo:3620811
name: provincial or state legislation process
def: "A legislation process in which some group passes pro-conservation legislation at the state or province level." []
is_a: elmo:3620801 ! legislation process
property_value: dcterms:contributor https://orcid.org/0000-0002-4366-3088
property_value: dcterms:contributor https://orcid.org/0000-0003-4817-0423
created_by: https://orcid.org/0000-0002-1296-2528

[Term]
id: elmo:3620812
name: national legislation process
def: "A legislation process in which some group passes pro-conservation legislation at the national level." []
is_a: elmo:3620801 ! legislation process
property_value: dcterms:contributor https://orcid.org/0000-0002-4366-3088
property_value: dcterms:contributor https://orcid.org/0000-0003-4817-0423
created_by: https://orcid.org/0000-0002-1296-2528

[Term]
id: elmo:3620813
name: international agreement process
def: "A ecosystem-oriented social process in which a humans collectively agree to measures that protect, conserve and restore biodiversity." []
is_a: elmo:3620800 ! ecosystem-oriented social process
property_value: dcterms:contributor https://orcid.org/0000-0002-4366-3088
property_value: dcterms:contributor https://orcid.org/0000-0003-4817-0423
created_by: https://orcid.org/0000-0002-1296-2528

[Term]
id: elmo:3620814
name: active enforcement process
def: "A ecosystem-oriented social process in which a human actively enforces the pro-conservation legislation or policies governing a specific area." []
is_a: elmo:3620800 ! ecosystem-oriented social process
property_value: dcterms:contributor https://orcid.org/0000-0002-4366-3088
property_value: dcterms:contributor https://orcid.org/0000-0003-4817-0423
created_by: https://orcid.org/0000-0002-1296-2528

[Term]
id: elmo:3620815
name: human-wildlife conflict reduction process
def: "A ecosystem-oriented social process in which a human implements measures to reduce conflict between fauna and humans." []
is_a: elmo:3620800 ! ecosystem-oriented social process
property_value: dcterms:contributor https://orcid.org/0000-0002-4366-3088
property_value: dcterms:contributor https://orcid.org/0000-0003-4817-0423
created_by: https://orcid.org/0000-0002-1296-2528

[Term]
id: elmo:3620816
name: human-assisted road crossing process
def: "A ecosystem-oriented social process in which a human assists a species in crossing a road." []
is_a: elmo:3620800 ! ecosystem-oriented social process
property_value: dcterms:contributor https://orcid.org/0000-0002-4366-3088
property_value: dcterms:contributor https://orcid.org/0000-0003-4817-0423
created_by: https://orcid.org/0000-0002-1296-2528

[Term]
id: elmo:3620817
name: awareness-raising process
def: "A ecosystem-oriented social process in which a human undertakes a process in order to make others more aware of threats to biodiversity." []
is_a: elmo:3620800 ! ecosystem-oriented social process
property_value: dcterms:contributor https://orcid.org/0000-0002-4366-3088
property_value: dcterms:contributor https://orcid.org/0000-0003-4817-0423
created_by: https://orcid.org/0000-0002-1296-2528

[Term]
id: elmo:3620818
name: social media campaign process
def: "An awareness-raising process in which a human uses social media to spread messages about threats to biodiversity." []
is_a: elmo:3620817 ! awareness-raising process
property_value: dcterms:contributor https://orcid.org/0000-0002-4366-3088
property_value: dcterms:contributor https://orcid.org/0000-0003-4817-0423
created_by: https://orcid.org/0000-0002-1296-2528

[Term]
id: elmo:3620819
name: community event creation process
def: "An awareness-raising process in which a human hosts an event for the community in a given area." []
is_a: elmo:3620817 ! awareness-raising process
property_value: dcterms:contributor https://orcid.org/0000-0002-4366-3088
property_value: dcterms:contributor https://orcid.org/0000-0003-4817-0423
created_by: https://orcid.org/0000-0002-1296-2528

[Term]
id: elmo:3620820
name: education process
def: "An awareness-raising process in which a human endeavours to improve the knowledge of others vis-a-vis restoration or conservation of biodiversity." []
is_a: elmo:3620817 ! awareness-raising process
property_value: dcterms:contributor https://orcid.org/0000-0002-4366-3088
property_value: dcterms:contributor https://orcid.org/0000-0003-4817-0423
created_by: https://orcid.org/0000-0002-1296-2528

[Term]
id: elmo:3620821
name: citizen science process
def: "An awareness-raising process in which a humans gather measurements of some ecosystem elements." []
is_a: elmo:3620817 ! awareness-raising process
property_value: dcterms:contributor https://orcid.org/0000-0002-4366-3088
property_value: dcterms:contributor https://orcid.org/0000-0003-4817-0423
created_by: https://orcid.org/0000-0002-1296-2528

[Term]
id: elmo:3620822
name: community engagement process
def: "An awareness-raising process in which a humans are gathered in a given area and engaged in the restoration and conservation of biodiversity." []
is_a: elmo:3620817 ! awareness-raising process
property_value: dcterms:contributor https://orcid.org/0000-0002-4366-3088
property_value: dcterms:contributor https://orcid.org/0000-0003-4817-0423
created_by: https://orcid.org/0000-0002-1296-2528

[Term]
id: elmo:3620823
name: pro-environmental behaviour change process
def: "A ecosystem-oriented social process in which a human endeavours to alter the behaviour of others vis-a-vis the degradation of ecosystems." [doi:10.1038/s41562-022-01473-w]
is_a: elmo:3620800 ! ecosystem-oriented social process
property_value: dcterms:contributor https://orcid.org/0000-0002-4366-3088
property_value: dcterms:contributor https://orcid.org/0000-0003-4817-0423
created_by: https://orcid.org/0000-0002-1296-2528

[Term]
id: elmo:3620824
name: signage installation process
def: "A pro-environmental behaviour change process in which signage is installed to encourage or deter activities in an area." []
is_a: elmo:3620823 ! pro-environmental behaviour change process
property_value: dcterms:contributor https://orcid.org/0000-0002-4366-3088
property_value: dcterms:contributor https://orcid.org/0000-0003-4817-0423
created_by: https://orcid.org/0000-0002-1296-2528

[Term]
id: elmo:3620825
name: individual outreach process
def: "A pro-environmental behaviour change process in which a human reaches out to people directly to encourage or deter activities in an area." []
is_a: elmo:3620823 ! pro-environmental behaviour change process
property_value: dcterms:contributor https://orcid.org/0000-0002-4366-3088
property_value: dcterms:contributor https://orcid.org/0000-0003-4817-0423
created_by: https://orcid.org/0000-0002-1296-2528

[Term]
id: elmo:3620826
name: landowner outreach process
def: "A pro-environmental behaviour change process in which a human reaches out to a landowner to encourage or deter activities in an area." []
is_a: elmo:3620823 ! pro-environmental behaviour change process
property_value: dcterms:contributor https://orcid.org/0000-0002-4366-3088
property_value: dcterms:contributor https://orcid.org/0000-0003-4817-0423
created_by: https://orcid.org/0000-0002-1296-2528

[Term]
id: elmo:3620827
name: sensitive features marking process
def: "A pro-environmental behaviour change process in which a human marks environmentally sensitive features to deter degradation or interference." []
is_a: elmo:3620823 ! pro-environmental behaviour change process
property_value: dcterms:contributor https://orcid.org/0000-0002-4366-3088
property_value: dcterms:contributor https://orcid.org/0000-0003-4817-0423
created_by: https://orcid.org/0000-0002-1296-2528

[Term]
id: elmo:3620828
name: fundraising process
def: "A ecosystem-oriented social process in which a human raises funds to support the restoration and conservation of a specific area." []
is_a: elmo:3620800 ! ecosystem-oriented social process
property_value: dcterms:contributor https://orcid.org/0000-0002-4366-3088
property_value: dcterms:contributor https://orcid.org/0000-0003-4817-0423
created_by: https://orcid.org/0000-0002-1296-2528

[Term]
id: elmo:3620829
name: financial incentive process
def: "A ecosystem-oriented social process in which financial incentives are offered to a humans in order to take pro-environmental measures." []
is_a: elmo:3620800 ! ecosystem-oriented social process
property_value: dcterms:contributor https://orcid.org/0000-0002-4366-3088
property_value: dcterms:contributor https://orcid.org/0000-0003-4817-0423
created_by: https://orcid.org/0000-0002-1296-2528

[Term]
id: elmo:3620830
name: environmental usage regulation process
def: "A ecosystem-oriented social process in which some authority regulates the usage of environments." []
is_a: elmo:3620800 ! ecosystem-oriented social process
property_value: dcterms:contributor https://orcid.org/0000-0002-4366-3088
property_value: dcterms:contributor https://orcid.org/0000-0003-4817-0423
created_by: https://orcid.org/0000-0002-1296-2528

[Term]
id: elmo:3620831
name: regulate grazing
def: "An environmental usage regulation process in which some authority regulates grazing in a given area." []
is_a: elmo:3620830 ! environmental usage regulation process
property_value: dcterms:contributor https://orcid.org/0000-0002-4366-3088
property_value: dcterms:contributor https://orcid.org/0000-0003-4817-0423
created_by: https://orcid.org/0000-0002-1296-2528

[Term]
id: elmo:3620832
name: prohibit grazing
def: "An environmental usage regulation process in which some authority prohibits grazing in a given area." []
is_a: elmo:3620831 ! regulate grazing
property_value: dcterms:contributor https://orcid.org/0000-0002-4366-3088
property_value: dcterms:contributor https://orcid.org/0000-0003-4817-0423
created_by: https://orcid.org/0000-0002-1296-2528

[Term]
id: elmo:3620833
name: regulate fishing
def: "An environmental usage regulation process in which some authority regulates fishing in a given area." []
is_a: elmo:3620830 ! environmental usage regulation process
property_value: dcterms:contributor https://orcid.org/0000-0002-4366-3088
property_value: dcterms:contributor https://orcid.org/0000-0003-4817-0423
created_by: https://orcid.org/0000-0002-1296-2528

[Term]
id: elmo:3620834
name: prohibit fishing
def: "An environmental usage regulation process in which some authority prohibits fishing in a given area." []
is_a: elmo:3620833 ! regulate fishing
property_value: dcterms:contributor https://orcid.org/0000-0002-4366-3088
property_value: dcterms:contributor https://orcid.org/0000-0003-4817-0423
created_by: https://orcid.org/0000-0002-1296-2528

[Term]
id: elmo:3620835
name: regulate chemical usage
def: "An environmental usage regulation process in which some authority regulates chemical usage in a given area." []
is_a: elmo:3620830 ! environmental usage regulation process
property_value: dcterms:contributor https://orcid.org/0000-0002-4366-3088
property_value: dcterms:contributor https://orcid.org/0000-0003-4817-0423
created_by: https://orcid.org/0000-0002-1296-2528

[Term]
id: elmo:3620836
name: prohibit chemical usage
def: "An environmental usage regulation process in which some authority prohibits chemical usage in a given area." []
is_a: elmo:3620835 ! regulate chemical usage
property_value: dcterms:contributor https://orcid.org/0000-0002-4366-3088
property_value: dcterms:contributor https://orcid.org/0000-0003-4817-0423
created_by: https://orcid.org/0000-0002-1296-2528

[Term]
id: elmo:3620837
name: regulate hunting
def: "An environmental usage regulation process in which some authority regulates hunting in a given area." []
is_a: elmo:3620830 ! environmental usage regulation process
property_value: dcterms:contributor https://orcid.org/0000-0002-4366-3088
property_value: dcterms:contributor https://orcid.org/0000-0003-4817-0423
created_by: https://orcid.org/0000-0002-1296-2528

[Term]
id: elmo:3620838
name: prohibit hunting
def: "An environmental usage regulation process in which some authority prohibits hunting in a given area." []
is_a: elmo:3620837 ! regulate hunting
property_value: dcterms:contributor https://orcid.org/0000-0002-4366-3088
property_value: dcterms:contributor https://orcid.org/0000-0003-4817-0423
created_by: https://orcid.org/0000-0002-1296-2528

[Term]
id: elmo:3620839
name: regulate recreational activities
def: "An environmental usage regulation process in which some authority regulates recreational activities in a given area." []
is_a: elmo:3620830 ! environmental usage regulation process
property_value: dcterms:contributor https://orcid.org/0000-0002-4366-3088
property_value: dcterms:contributor https://orcid.org/0000-0003-4817-0423
created_by: https://orcid.org/0000-0002-1296-2528

[Term]
id: elmo:3620840
name: prohibit recreational activities
def: "An environmental usage regulation process in which some authority prohibits recreational activities in a given area." []
is_a: elmo:3620839 ! regulate recreational activities
property_value: dcterms:contributor https://orcid.org/0000-0002-4366-3088
property_value: dcterms:contributor https://orcid.org/0000-0003-4817-0423
created_by: https://orcid.org/0000-0002-1296-2528

[Term]
id: elmo:3620841
name: limit public access
def: "An environmental usage regulation process in which some authority limits public access to a given area." []
is_a: elmo:3620830 ! environmental usage regulation process
property_value: dcterms:contributor https://orcid.org/0000-0002-4366-3088
property_value: dcterms:contributor https://orcid.org/0000-0003-4817-0423
created_by: https://orcid.org/0000-0002-1296-2528

[Term]
id: elmo:3620842
name: prohibit public access
def: "An environmental usage regulation process in which some authority prohibits public access to a given area." []
is_a: elmo:3620841 ! limit public access
property_value: dcterms:contributor https://orcid.org/0000-0002-4366-3088
property_value: dcterms:contributor https://orcid.org/0000-0003-4817-0423
created_by: https://orcid.org/0000-0002-1296-2528

[Term]
id: elmo:3620843
name: regulate dredging
def: "An environmental usage regulation process in which some authority regulates dredging in a given area." []
is_a: elmo:3620830 ! environmental usage regulation process
property_value: dcterms:contributor https://orcid.org/0000-0002-4366-3088
property_value: dcterms:contributor https://orcid.org/0000-0003-4817-0423
created_by: https://orcid.org/0000-0002-1296-2528

[Term]
id: elmo:3620844
name: prohibit dredging
def: "An environmental usage regulation process in which some authority prohibits dredging in a given area." []
is_a: elmo:3620843 ! regulate dredging
property_value: dcterms:contributor https://orcid.org/0000-0002-4366-3088
property_value: dcterms:contributor https://orcid.org/0000-0003-4817-0423
created_by: https://orcid.org/0000-0002-1296-2528

[Term]
id: elmo:3620845
name: regulate aquaculture
def: "An environmental usage regulation process in which some authority regulates aquaculture in a given area." []
is_a: elmo:3620830 ! environmental usage regulation process
property_value: dcterms:contributor https://orcid.org/0000-0002-4366-3088
property_value: dcterms:contributor https://orcid.org/0000-0003-4817-0423
created_by: https://orcid.org/0000-0002-1296-2528

[Term]
id: elmo:3620846
name: prohibit aquaculture
def: "An environmental usage regulation process in which some authority prohibits aquaculture in a given area." []
is_a: elmo:3620845 ! regulate aquaculture
property_value: dcterms:contributor https://orcid.org/0000-0002-4366-3088
property_value: dcterms:contributor https://orcid.org/0000-0003-4817-0423
created_by: https://orcid.org/0000-0002-1296-2528

[Term]
id: elmo:3620847
name: cultural ecosystem management process
def: "A ecosystem-oriented social process in which a humans undertake shared practices passed down through generations to manage the ecosystem in which they live." []
is_a: elmo:3620800 ! ecosystem-oriented social process
property_value: dcterms:contributor https://orcid.org/0000-0002-4366-3088
property_value: dcterms:contributor https://orcid.org/0000-0003-4817-0423
created_by: https://orcid.org/0000-0002-1296-2528

[Term]
id: elmo:3620848
name: cultural ecosystem usage process
def: "A ecosystem-oriented social process in which a humans harvest resources from the environment for shared practices that are passed down through generations." []
is_a: elmo:3620800 ! ecosystem-oriented social process
property_value: dcterms:contributor https://orcid.org/0000-0002-4366-3088
property_value: dcterms:contributor https://orcid.org/0000-0003-4817-0423
created_by: https://orcid.org/0000-0002-1296-2528

[Term]
id: elmo:3620849
name: plan specification change process
def: "A ecosystem-oriented social process in which a human alters the way in which some planned process is undertaken." []
is_a: elmo:3620800 ! ecosystem-oriented social process
property_value: dcterms:contributor https://orcid.org/0000-0002-4366-3088
property_value: dcterms:contributor https://orcid.org/0000-0003-4817-0423
created_by: https://orcid.org/0000-0002-1296-2528

[Term]
id: elmo:3620850
name: alter mowing timing
def: "A change to the mowing regime in which a human alters the timing of regular mowing with the goal of protecting specific taxa." []
is_a: elmo:3620851 ! alter mowing regime
property_value: dcterms:contributor https://orcid.org/0000-0002-4366-3088
property_value: dcterms:contributor https://orcid.org/0000-0003-4817-0423
created_by: https://orcid.org/0000-0002-1296-2528

[Term]
id: elmo:3620851
name: alter mowing regime
def: "A plan specification change process in which a human alters the mowing regime (i.e. frequency, height, timing)" []
is_a: elmo:3620849 ! plan specification change process
property_value: dcterms:contributor https://orcid.org/0000-0002-4366-3088
property_value: dcterms:contributor https://orcid.org/0000-0003-4817-0423
created_by: https://orcid.org/0000-0002-1296-2528

[Term]
id: elmo:3620852
name: alter mowing height
def: "A change to the mowing regime in which a human alters the height of a mower with the goal of protecting specific taxa." []
is_a: elmo:3620851 ! alter mowing regime
property_value: dcterms:contributor https://orcid.org/0000-0002-4366-3088
property_value: dcterms:contributor https://orcid.org/0000-0003-4817-0423
created_by: https://orcid.org/0000-0002-1296-2528

[Term]
id: elmo:3620853
name: alter tilling regime
def: "A change to the tilling regime in which a human alters the frequency, timing or severity of a regular tilling process." []
is_a: elmo:3620849 ! plan specification change process
property_value: dcterms:contributor https://orcid.org/0000-0002-4366-3088
property_value: dcterms:contributor https://orcid.org/0000-0003-4817-0423
created_by: https://orcid.org/0000-0002-1296-2528

[Term]
id: elmo:3620854
name: alter chemical regime
def: "A change to the chemical regime in which a human alters the frequency, timing or severity of a regular chemical application process." []
is_a: elmo:3620849 ! plan specification change process
property_value: dcterms:contributor https://orcid.org/0000-0002-4366-3088
property_value: dcterms:contributor https://orcid.org/0000-0003-4817-0423
created_by: https://orcid.org/0000-0002-1296-2528

[Term]
id: elmo:3620855
name: alter insecticide regime
def: "A change to the insecticide regime in which a human alters the frequency, timing or severity of a regular insecticide application process." []
is_a: elmo:3620854 ! alter chemical regime
property_value: dcterms:contributor https://orcid.org/0000-0002-4366-3088
property_value: dcterms:contributor https://orcid.org/0000-0003-4817-0423
created_by: https://orcid.org/0000-0002-1296-2528

[Term]
id: elmo:3620856
name: alter fertilizer regime
def: "A change to the fertilizer regime in which a human alters the frequency, timing or severity of a regular fertilizer application process." []
is_a: elmo:3620849 ! plan specification change process
property_value: dcterms:contributor https://orcid.org/0000-0002-4366-3088
property_value: dcterms:contributor https://orcid.org/0000-0003-4817-0423
created_by: https://orcid.org/0000-0002-1296-2528

[Term]
id: elmo:3620857
name: alter lighting regime
def: "A change to the lighting regime in which a human alters the frequency, timing or intensity of lighting." []
is_a: elmo:3620849 ! plan specification change process
property_value: dcterms:contributor https://orcid.org/0000-0002-4366-3088
property_value: dcterms:contributor https://orcid.org/0000-0003-4817-0423
created_by: https://orcid.org/0000-0002-1296-2528

[Term]
id: elmo:3620858
name: alter grazing regime
def: "A change to the grazing regime in which a human alters the frequency, timing or intensity of grazing." []
is_a: elmo:3620849 ! plan specification change process
property_value: dcterms:contributor https://orcid.org/0000-0002-4366-3088
property_value: dcterms:contributor https://orcid.org/0000-0003-4817-0423
created_by: https://orcid.org/0000-0002-1296-2528

[Term]
id: elmo:3620859
name: alter dam regime
def: "A change to the dam regime in which a human alters the frequency, timing or intensity of water released by a dam." []
is_a: elmo:3620849 ! plan specification change process
property_value: dcterms:contributor https://orcid.org/0000-0002-4366-3088
property_value: dcterms:contributor https://orcid.org/0000-0003-4817-0423
created_by: https://orcid.org/0000-0002-1296-2528

[Term]
id: elmo:3620860
name: alter herbicide regime
def: "A change to the herbicide regime in which a human alters the frequency, timing or severity of a regular herbicide application process." []
is_a: elmo:3620854 ! alter chemical regime
property_value: dcterms:contributor https://orcid.org/0000-0002-4366-3088
property_value: dcterms:contributor https://orcid.org/0000-0003-4817-0423
created_by: https://orcid.org/0000-0002-1296-2528

[Term]
id: elmo:3620861
name: cease herbicide usage
def: "A change to the herbicide regime in which a human ceases some herbicide application process." []
is_a: elmo:3620860 ! alter herbicide regime
property_value: dcterms:contributor https://orcid.org/0000-0002-4366-3088
property_value: dcterms:contributor https://orcid.org/0000-0003-4817-0423
created_by: https://orcid.org/0000-0002-1296-2528

[Term]
id: elmo:3621000
name: fishing with equipment modified for conservation
def: "A planned environmental usage process in which fishing equipment is modified for conservation (e.g. bycatch deterrent devices are installed)" []
is_a: ENVO:01001436 ! planned environmental usage process
property_value: dcterms:contributor https://orcid.org/0000-0002-1296-2528

[Term]
id: elmo:3621001
name: fishing with net modified for conservation
def: "A fishing process in which a human uses a net that has been modified to reduce bycatch or accomplish some other conservation-oriented goal." []
is_a: elmo:3621000 ! fishing with equipment modified for conservation
property_value: dcterms:contributor https://orcid.org/0000-0002-1296-2528

[Term]
id: elmo:3621002
name: fishing with hook modified for conservation
def: "A fishing process in which a human uses a hook that has been modified for conservation." []
is_a: elmo:3621000 ! fishing with equipment modified for conservation
property_value: dcterms:contributor https://orcid.org/0000-0002-1296-2528

[Term]
id: elmo:3621003
name: fishing with added acoustic devices for conservation
def: "A fishing process in which a human adds acoustic devices to fishing gear to deter bycatch." []
is_a: elmo:3621000 ! fishing with equipment modified for conservation
property_value: dcterms:contributor https://orcid.org/0000-0002-1296-2528

[Term]
id: elmo:3621004
name: fishing with modified traps
def: "A fishing process in which a human uses traps modified to deter bycatch." []
is_a: elmo:3621000 ! fishing with equipment modified for conservation
property_value: dcterms:contributor https://orcid.org/0000-0002-1296-2528

[Term]
id: elmo:3621005
name: fishing with modified line-setting procedure
def: "A fishing process in which a human attaches bait to lines in a way that deters seabird scavenging (i.e. underwater)" []
is_a: elmo:3621000 ! fishing with equipment modified for conservation
property_value: dcterms:contributor https://orcid.org/0000-0002-1296-2528

[Term]
id: elmo:3621006
name: aquaculture process modified for conservation
def: "A planned environmental usage process in which a human engages in aquaculture with modifications for conservation (e.g. disease control measures)" []
is_a: ENVO:01001436 ! planned environmental usage process
property_value: dcterms:contributor https://orcid.org/0000-0002-1296-2528

[Term]
id: elmo:3621007
name: underwater turbine modified for conservation
def: "A planned environmental usage process in which a human installs an underwater turbine modified for conservation." []
is_a: ENVO:01001436 ! planned environmental usage process
property_value: dcterms:contributor https://orcid.org/0000-0002-1296-2528

[Term]
id: elmo:3621008
name: farming process modified for conservation
def: "A planned environmental usage process in which a human engages in farming with modifications for the conservation of biodiversity." []
is_a: ENVO:01001436 ! planned environmental usage process
property_value: dcterms:contributor https://orcid.org/0000-0002-1296-2528

[Term]
id: elmo:3621009
name: farming with intercropping
def: "A farming process modified for conservation in which a human grows two or more crop varities in close proximity to one another." [ISBN:9781933395210]
is_a: elmo:3621008 ! farming process modified for conservation
property_value: dcterms:contributor https://orcid.org/0000-0002-1296-2528

[Term]
id: elmo:3621010
name: agroforestry process
def: "A farming process modified for conservation in which a human integrates trees and crops or pasture." [wd:Q397350]
is_a: elmo:3621008 ! farming process modified for conservation
property_value: dcterms:contributor https://orcid.org/0000-0002-1296-2528

[Term]
id: elmo:3621011
name: alley cropping farming process
def: "An agroforestry process in which crops are grown in between rows of trees and shrubs." [ISBN:9781933395210]
is_a: elmo:3621010 ! agroforestry process
property_value: dcterms:contributor https://orcid.org/0000-0002-1296-2528

[Term]
id: elmo:3621012
name: no-till farming
def: "A farming process modified for conservation in which a human does not disturb the soil in between crop plantings." [wd:Q1227672]
is_a: elmo:3621008 ! farming process modified for conservation
property_value: dcterms:contributor https://orcid.org/0000-0002-1296-2528

[Term]
id: elmo:3621013
name: organic farming regime
def: "A farming process modified for conservation in which a human avoids synthetic or chemical inputs in the farming process. The definition of organic is often the subject of government regulation." [https://en.wikipedia.org/wiki/Organic_farming]
is_a: elmo:3621008 ! farming process modified for conservation
property_value: dcterms:contributor https://orcid.org/0000-0002-1296-2528

[Term]
id: elmo:3621014
name: crop rotation
def: "A farming process modified for conservation in which the crop type is rotated year over year." [ISBN:9781933395210]
is_a: elmo:3621008 ! farming process modified for conservation
property_value: dcterms:contributor https://orcid.org/0000-0002-1296-2528

[Term]
id: elmo:3621015
name: set aside farmland for conservation
def: "A farming process modified for conservation in which a human agrees not to farm some portion of a landscape." [https://en.wikipedia.org/wiki/Set-aside]
is_a: elmo:3621008 ! farming process modified for conservation
property_value: dcterms:contributor https://orcid.org/0000-0002-1296-2528

[Term]
id: elmo:3621016
name: forestry process modified for conservation
def: "A planned environmental usage process in which a human harvests trees in a manner that attempts to ameliorate the impact on the landscape." []
is_a: ENVO:01001436 ! planned environmental usage process
property_value: dcterms:contributor https://orcid.org/0000-0002-1296-2528

[Term]
id: elmo:3621017
name: coppice process
def: "A forestry process in which a human cuts trees down to the stump, allowing the trees to regenerate from the stump." [https://en.wikipedia.org/wiki/Coppicing]
is_a: elmo:3621016 ! forestry process modified for conservation
property_value: dcterms:contributor https://orcid.org/0000-0002-1296-2528

[Term]
id: elmo:3621018
name: selective harvesting process
def: "A forestry process in which a human harvests trees according to their age with the goal of preserving some overall age for a forest stand." [https://en.wikipedia.org/wiki/Selection_cutting]
is_a: elmo:3621016 ! forestry process modified for conservation
property_value: dcterms:contributor https://orcid.org/0000-0002-1296-2528

[Term]
id: elmo:3621019
name: woody debris removal process
def: "A forestry process in which a human removes coarse woody debris after harvesting trees, thereby reducing the risk and intensity of forest fire." [https://en.wikipedia.org/wiki/Coarse_woody_debris]
is_a: elmo:3621016 ! forestry process modified for conservation
property_value: dcterms:contributor https://orcid.org/0000-0002-1296-2528

[Term]
id: elmo:3621020
name: leave woody debris
def: "A forestry process in which a human leaves coarse woody debris after harvesting, thereby increasing available resources." [https://en.wikipedia.org/wiki/Coarse_woody_debris]
is_a: elmo:3621016 ! forestry process modified for conservation
property_value: dcterms:contributor https://orcid.org/0000-0002-1296-2528

[Term]
id: elmo:3621021
name: shelterwood cutting process
def: "A forestry process in which a human primarily harvests large trees in order to increase light availability for seedling species." [https://en.wikipedia.org/wiki/Shelterwood_cutting]
is_a: elmo:3621016 ! forestry process modified for conservation
property_value: dcterms:contributor https://orcid.org/0000-0002-1296-2528

[Term]
id: elmo:3621022
name: regulate wind turbine speed
def: "A planned environmental usage process in which a human modifies the level of wind speed required to spin turbines, thereby preventing avifauna fatalities." [doi:10.1002/2688-8319.12371]
synonym: "curtailment" EXACT []
synonym: "doi:10.1002/2688-8319.12371" BROAD []
is_a: ENVO:01001436 ! planned environmental usage process
property_value: dcterms:contributor https://orcid.org/0000-0002-1296-2528

[Typedef]
id: ENVO:01001307
name: partially_surrounded_by
def: "x partially_surrounded_by y if and only if (1) x is adjacent to y and for the region r that is adjacent to x, r partially overlaps y (2) the shared boundary between x and y occupies  a non-trivial proportion of the outermost boundary of x" []

[Typedef]
id: ENVO:01003004
name: derives from part of
def: "A relation between two distinct material entities, the new entity and the old entity, in which the new entity begins to exist through the separation or transformation of a part of the old entity, and the new entity inherits a significant portion of the matter belonging to that part of the old entity." []

[Typedef]
id: ENVO:02000200
name: has increased levels of
def: "A has part relationship between a whole and a part, where the number of parts present in the whole is higher than in comparable entities." []
is_a: RO:0002180

