<?xml version="1.0"?>
<rdf:RDF xmlns="https://w3id.org/elmo/elmo/elmo-full.owl#"
     xml:base="https://w3id.org/elmo/elmo/elmo-full.owl"
     xmlns:dce="http://purl.org/dc/elements/1.1/"
     xmlns:obo="http://purl.obolibrary.org/obo/"
     xmlns:owl="http://www.w3.org/2002/07/owl#"
     xmlns:rdf="http://www.w3.org/1999/02/22-rdf-syntax-ns#"
     xmlns:xml="http://www.w3.org/XML/1998/namespace"
     xmlns:xsd="http://www.w3.org/2001/XMLSchema#"
     xmlns:doap="http://usefulinc.com/ns/doap#"
     xmlns:foaf="http://xmlns.com/foaf/0.1/"
     xmlns:rdfs="http://www.w3.org/2000/01/rdf-schema#"
     xmlns:dcterms="http://purl.org/dc/terms/"
     xmlns:oboInOwl="http://www.geneontology.org/formats/oboInOwl#">
    <owl:Ontology rdf:about="https://w3id.org/elmo/elmo/elmo-full.owl">
        <owl:versionIRI rdf:resource="https://w3id.org/elmo/elmo/releases/2025-04-22/elmo-full.owl"/>
        <dcterms:description>None</dcterms:description>
        <dcterms:license rdf:resource="https://creativecommons.org/public-domain/"/>
        <dcterms:title>Ecolink Model Ontology (ELMO)</dcterms:title>
        <owl:versionInfo>2025-04-22</owl:versionInfo>
    </owl:Ontology>
    


    <!-- 
    ///////////////////////////////////////////////////////////////////////////////////////
    //
    // Annotation properties
    //
    ///////////////////////////////////////////////////////////////////////////////////////
     -->

    


    <!-- http://purl.obolibrary.org/obo/IAO_0000114 -->

    <owl:AnnotationProperty rdf:about="http://purl.obolibrary.org/obo/IAO_0000114"/>
    


    <!-- http://purl.obolibrary.org/obo/IAO_0000115 -->

    <owl:AnnotationProperty rdf:about="http://purl.obolibrary.org/obo/IAO_0000115">
        <rdfs:label>definition</rdfs:label>
    </owl:AnnotationProperty>
    


    <!-- http://purl.obolibrary.org/obo/IAO_0000116 -->

    <owl:AnnotationProperty rdf:about="http://purl.obolibrary.org/obo/IAO_0000116">
        <rdfs:label xml:lang="en">editor note</rdfs:label>
    </owl:AnnotationProperty>
    


    <!-- http://purl.obolibrary.org/obo/IAO_0000119 -->

    <owl:AnnotationProperty rdf:about="http://purl.obolibrary.org/obo/IAO_0000119"/>
    


    <!-- http://purl.org/dc/elements/1.1/contributor -->

    <owl:AnnotationProperty rdf:about="http://purl.org/dc/elements/1.1/contributor"/>
    


    <!-- http://purl.org/dc/elements/1.1/creator -->

    <owl:AnnotationProperty rdf:about="http://purl.org/dc/elements/1.1/creator"/>
    


    <!-- http://purl.org/dc/elements/1.1/description -->

    <owl:AnnotationProperty rdf:about="http://purl.org/dc/elements/1.1/description"/>
    


    <!-- http://purl.org/dc/elements/1.1/source -->

    <owl:AnnotationProperty rdf:about="http://purl.org/dc/elements/1.1/source"/>
    


    <!-- http://purl.org/dc/elements/1.1/title -->

    <owl:AnnotationProperty rdf:about="http://purl.org/dc/elements/1.1/title"/>
    


    <!-- http://purl.org/dc/elements/1.1/type -->

    <owl:AnnotationProperty rdf:about="http://purl.org/dc/elements/1.1/type"/>
    


    <!-- http://purl.org/dc/terms/contributor -->

    <owl:AnnotationProperty rdf:about="http://purl.org/dc/terms/contributor"/>
    


    <!-- http://purl.org/dc/terms/creator -->

    <owl:AnnotationProperty rdf:about="http://purl.org/dc/terms/creator"/>
    


    <!-- http://purl.org/dc/terms/description -->

    <owl:AnnotationProperty rdf:about="http://purl.org/dc/terms/description">
        <rdfs:label>description</rdfs:label>
    </owl:AnnotationProperty>
    


    <!-- http://purl.org/dc/terms/license -->

    <owl:AnnotationProperty rdf:about="http://purl.org/dc/terms/license">
        <rdfs:label>license</rdfs:label>
    </owl:AnnotationProperty>
    


    <!-- http://purl.org/dc/terms/source -->

    <owl:AnnotationProperty rdf:about="http://purl.org/dc/terms/source"/>
    


    <!-- http://purl.org/dc/terms/title -->

    <owl:AnnotationProperty rdf:about="http://purl.org/dc/terms/title">
        <rdfs:label>title</rdfs:label>
    </owl:AnnotationProperty>
    


    <!-- http://usefulinc.com/ns/doap#GitRepository -->

    <owl:AnnotationProperty rdf:about="http://usefulinc.com/ns/doap#GitRepository"/>
    


    <!-- http://usefulinc.com/ns/doap#bug-database -->

    <owl:AnnotationProperty rdf:about="http://usefulinc.com/ns/doap#bug-database"/>
    


    <!-- http://www.geneontology.org/formats/oboInOwl#created_by -->

    <owl:AnnotationProperty rdf:about="http://www.geneontology.org/formats/oboInOwl#created_by"/>
    


    <!-- http://www.geneontology.org/formats/oboInOwl#default-namespace -->

    <owl:AnnotationProperty rdf:about="http://www.geneontology.org/formats/oboInOwl#default-namespace"/>
    


    <!-- http://www.geneontology.org/formats/oboInOwl#hasBroadSynonym -->

    <owl:AnnotationProperty rdf:about="http://www.geneontology.org/formats/oboInOwl#hasBroadSynonym"/>
    


    <!-- http://www.geneontology.org/formats/oboInOwl#hasDbXref -->

    <owl:AnnotationProperty rdf:about="http://www.geneontology.org/formats/oboInOwl#hasDbXref"/>
    


    <!-- http://www.geneontology.org/formats/oboInOwl#hasExactSynonym -->

    <owl:AnnotationProperty rdf:about="http://www.geneontology.org/formats/oboInOwl#hasExactSynonym"/>
    


    <!-- http://www.geneontology.org/formats/oboInOwl#hasNarrowSynonym -->

    <owl:AnnotationProperty rdf:about="http://www.geneontology.org/formats/oboInOwl#hasNarrowSynonym"/>
    


    <!-- http://xmlns.com/foaf/0.1/homepage -->

    <owl:AnnotationProperty rdf:about="http://xmlns.com/foaf/0.1/homepage"/>
    


    <!-- 
    ///////////////////////////////////////////////////////////////////////////////////////
    //
    // Object Properties
    //
    ///////////////////////////////////////////////////////////////////////////////////////
     -->

    


    <!-- http://purl.obolibrary.org/obo/BFO_0000050 -->

    <owl:ObjectProperty rdf:about="http://purl.obolibrary.org/obo/BFO_0000050"/>
    


    <!-- http://purl.obolibrary.org/obo/BFO_0000051 -->

    <owl:ObjectProperty rdf:about="http://purl.obolibrary.org/obo/BFO_0000051"/>
    


    <!-- http://purl.obolibrary.org/obo/BFO_0000066 -->

    <owl:ObjectProperty rdf:about="http://purl.obolibrary.org/obo/BFO_0000066"/>
    


    <!-- http://purl.obolibrary.org/obo/BFO_0000067 -->

    <owl:ObjectProperty rdf:about="http://purl.obolibrary.org/obo/BFO_0000067"/>
    


    <!-- http://purl.obolibrary.org/obo/ENVO_01001307 -->

    <owl:ObjectProperty rdf:about="http://purl.obolibrary.org/obo/ENVO_01001307">
        <obo:IAO_0000115>x partially_surrounded_by y if and only if (1) x is adjacent to y and for the region r that is adjacent to x, r partially overlaps y (2) the shared boundary between x and y occupies  a non-trivial proportion of the outermost boundary of x</obo:IAO_0000115>
        <rdfs:label>partially_surrounded_by</rdfs:label>
    </owl:ObjectProperty>
    


    <!-- http://purl.obolibrary.org/obo/ENVO_01003004 -->

    <owl:ObjectProperty rdf:about="http://purl.obolibrary.org/obo/ENVO_01003004">
        <obo:IAO_0000115 xml:lang="en">A relation between two distinct material entities, the new entity and the old entity, in which the new entity begins to exist through the separation or transformation of a part of the old entity, and the new entity inherits a significant portion of the matter belonging to that part of the old entity.</obo:IAO_0000115>
        <rdfs:label xml:lang="en">derives from part of</rdfs:label>
    </owl:ObjectProperty>
    


    <!-- http://purl.obolibrary.org/obo/ENVO_02000200 -->

    <owl:ObjectProperty rdf:about="http://purl.obolibrary.org/obo/ENVO_02000200">
        <rdfs:subPropertyOf rdf:resource="http://purl.obolibrary.org/obo/RO_0002180"/>
        <obo:IAO_0000115>A has part relationship between a whole and a part, where the number of parts present in the whole is higher than in comparable entities.</obo:IAO_0000115>
        <rdfs:label>has increased levels of</rdfs:label>
    </owl:ObjectProperty>
    


    <!-- http://purl.obolibrary.org/obo/RO_0000052 -->

    <owl:ObjectProperty rdf:about="http://purl.obolibrary.org/obo/RO_0000052"/>
    


    <!-- http://purl.obolibrary.org/obo/RO_0000053 -->

    <owl:ObjectProperty rdf:about="http://purl.obolibrary.org/obo/RO_0000053"/>
    


    <!-- http://purl.obolibrary.org/obo/RO_0000056 -->

    <owl:ObjectProperty rdf:about="http://purl.obolibrary.org/obo/RO_0000056"/>
    


    <!-- http://purl.obolibrary.org/obo/RO_0000057 -->

    <owl:ObjectProperty rdf:about="http://purl.obolibrary.org/obo/RO_0000057"/>
    


    <!-- http://purl.obolibrary.org/obo/RO_0000086 -->

    <owl:ObjectProperty rdf:about="http://purl.obolibrary.org/obo/RO_0000086"/>
    


    <!-- http://purl.obolibrary.org/obo/RO_0000087 -->

    <owl:ObjectProperty rdf:about="http://purl.obolibrary.org/obo/RO_0000087"/>
    


    <!-- http://purl.obolibrary.org/obo/RO_0000091 -->

    <owl:ObjectProperty rdf:about="http://purl.obolibrary.org/obo/RO_0000091"/>
    


    <!-- http://purl.obolibrary.org/obo/RO_0001000 -->

    <owl:ObjectProperty rdf:about="http://purl.obolibrary.org/obo/RO_0001000"/>
    


    <!-- http://purl.obolibrary.org/obo/RO_0001025 -->

    <owl:ObjectProperty rdf:about="http://purl.obolibrary.org/obo/RO_0001025"/>
    


    <!-- http://purl.obolibrary.org/obo/RO_0002007 -->

    <owl:ObjectProperty rdf:about="http://purl.obolibrary.org/obo/RO_0002007"/>
    


    <!-- http://purl.obolibrary.org/obo/RO_0002084 -->

    <owl:ObjectProperty rdf:about="http://purl.obolibrary.org/obo/RO_0002084"/>
    


    <!-- http://purl.obolibrary.org/obo/RO_0002131 -->

    <owl:ObjectProperty rdf:about="http://purl.obolibrary.org/obo/RO_0002131"/>
    


    <!-- http://purl.obolibrary.org/obo/RO_0002170 -->

    <owl:ObjectProperty rdf:about="http://purl.obolibrary.org/obo/RO_0002170"/>
    


    <!-- http://purl.obolibrary.org/obo/RO_0002180 -->

    <owl:ObjectProperty rdf:about="http://purl.obolibrary.org/obo/RO_0002180"/>
    


    <!-- http://purl.obolibrary.org/obo/RO_0002211 -->

    <owl:ObjectProperty rdf:about="http://purl.obolibrary.org/obo/RO_0002211"/>
    


    <!-- http://purl.obolibrary.org/obo/RO_0002219 -->

    <owl:ObjectProperty rdf:about="http://purl.obolibrary.org/obo/RO_0002219"/>
    


    <!-- http://purl.obolibrary.org/obo/RO_0002220 -->

    <owl:ObjectProperty rdf:about="http://purl.obolibrary.org/obo/RO_0002220"/>
    


    <!-- http://purl.obolibrary.org/obo/RO_0002229 -->

    <owl:ObjectProperty rdf:about="http://purl.obolibrary.org/obo/RO_0002229"/>
    


    <!-- http://purl.obolibrary.org/obo/RO_0002233 -->

    <owl:ObjectProperty rdf:about="http://purl.obolibrary.org/obo/RO_0002233"/>
    


    <!-- http://purl.obolibrary.org/obo/RO_0002234 -->

    <owl:ObjectProperty rdf:about="http://purl.obolibrary.org/obo/RO_0002234"/>
    


    <!-- http://purl.obolibrary.org/obo/RO_0002297 -->

    <owl:ObjectProperty rdf:about="http://purl.obolibrary.org/obo/RO_0002297"/>
    


    <!-- http://purl.obolibrary.org/obo/RO_0002351 -->

    <owl:ObjectProperty rdf:about="http://purl.obolibrary.org/obo/RO_0002351"/>
    


    <!-- http://purl.obolibrary.org/obo/RO_0002353 -->

    <owl:ObjectProperty rdf:about="http://purl.obolibrary.org/obo/RO_0002353"/>
    


    <!-- http://purl.obolibrary.org/obo/RO_0002354 -->

    <owl:ObjectProperty rdf:about="http://purl.obolibrary.org/obo/RO_0002354"/>
    


    <!-- http://purl.obolibrary.org/obo/RO_0002473 -->

    <owl:ObjectProperty rdf:about="http://purl.obolibrary.org/obo/RO_0002473"/>
    


    <!-- http://purl.obolibrary.org/obo/RO_0002500 -->

    <owl:ObjectProperty rdf:about="http://purl.obolibrary.org/obo/RO_0002500"/>
    


    <!-- http://purl.obolibrary.org/obo/RO_0002507 -->

    <owl:ObjectProperty rdf:about="http://purl.obolibrary.org/obo/RO_0002507"/>
    


    <!-- http://purl.obolibrary.org/obo/RO_0002509 -->

    <owl:ObjectProperty rdf:about="http://purl.obolibrary.org/obo/RO_0002509"/>
    


    <!-- http://purl.obolibrary.org/obo/RO_0002608 -->

    <owl:ObjectProperty rdf:about="http://purl.obolibrary.org/obo/RO_0002608"/>
    


    <!-- 
    ///////////////////////////////////////////////////////////////////////////////////////
    //
    // Classes
    //
    ///////////////////////////////////////////////////////////////////////////////////////
     -->

    


    <!-- http://purl.obolibrary.org/obo/BFO_0000015 -->

    <owl:Class rdf:about="http://purl.obolibrary.org/obo/BFO_0000015">
        <rdfs:label xml:lang="en">process</rdfs:label>
    </owl:Class>
    


    <!-- http://purl.obolibrary.org/obo/ENVO_01001170 -->

    <owl:Class rdf:about="http://purl.obolibrary.org/obo/ENVO_01001170">
        <rdfs:subClassOf rdf:resource="http://purl.obolibrary.org/obo/ENVO_02500000"/>
        <rdfs:subClassOf>
            <owl:Restriction>
                <owl:onProperty rdf:resource="http://purl.obolibrary.org/obo/RO_0002211"/>
                <owl:someValuesFrom rdf:resource="http://purl.obolibrary.org/obo/ENVO_02500000"/>
            </owl:Restriction>
        </rdfs:subClassOf>
        <obo:IAO_0000115>A process during which an ecosystem, its parts, or the processes it participates in are modified by human intervention to accomplish an objective.</obo:IAO_0000115>
        <oboInOwl:hasExactSynonym>ecosystem management</oboInOwl:hasExactSynonym>
        <rdfs:label xml:lang="en">active ecosystem management process</rdfs:label>
    </owl:Class>
    <owl:Axiom>
        <owl:annotatedSource rdf:resource="http://purl.obolibrary.org/obo/ENVO_01001170"/>
        <owl:annotatedProperty rdf:resource="http://purl.obolibrary.org/obo/IAO_0000115"/>
        <owl:annotatedTarget>A process during which an ecosystem, its parts, or the processes it participates in are modified by human intervention to accomplish an objective.</owl:annotatedTarget>
        <oboInOwl:hasDbXref>https://www.iucn.org/theme/protected-areas/about/protected-areas-categories/category-iv-habitatspecies-management-area</oboInOwl:hasDbXref>
    </owl:Axiom>
    


    <!-- http://purl.obolibrary.org/obo/ENVO_01001436 -->

    <owl:Class rdf:about="http://purl.obolibrary.org/obo/ENVO_01001436">
        <rdfs:subClassOf rdf:resource="http://purl.obolibrary.org/obo/ENVO_02500000"/>
        <rdfs:subClassOf>
            <owl:Restriction>
                <owl:onProperty rdf:resource="http://purl.obolibrary.org/obo/BFO_0000051"/>
                <owl:someValuesFrom rdf:resource="http://purl.obolibrary.org/obo/ENVO_01001170"/>
            </owl:Restriction>
        </rdfs:subClassOf>
        <obo:IAO_0000115>A planned process during which humans access and obtain resources, benefits, or services from a natural or anthropised ecosystem.</obo:IAO_0000115>
        <oboInOwl:created_by rdf:resource="https://orcid.org/0000-0002-4366-3088"/>
        <rdfs:label xml:lang="en">planned environmental usage process</rdfs:label>
    </owl:Class>
    


    <!-- http://purl.obolibrary.org/obo/ENVO_02500000 -->

    <owl:Class rdf:about="http://purl.obolibrary.org/obo/ENVO_02500000">
        <rdfs:subClassOf rdf:resource="http://purl.obolibrary.org/obo/BFO_0000015"/>
        <obo:IAO_0000115>A process in which includes the components of an environmental system as participants.</obo:IAO_0000115>
        <rdfs:label xml:lang="en">environmental system process</rdfs:label>
    </owl:Class>
    


    <!-- https://w3id.org/elmo/ELMO_0000000 -->

    <owl:Class rdf:about="https://w3id.org/elmo/ELMO_0000000">
        <rdfs:label xml:lang="en">root node</rdfs:label>
    </owl:Class>
    


    <!-- https://w3id.org/elmo/elmo_3620020 -->

    <owl:Class rdf:about="https://w3id.org/elmo/elmo_3620020">
        <rdfs:subClassOf rdf:resource="http://purl.obolibrary.org/obo/ENVO_01001170"/>
        <obo:IAO_0000115 xml:lang="en">An active ecosystem management process during which a human employs machines or tools to directly impact an ecosystem and realize some ecosystem management goal.</obo:IAO_0000115>
        <dcterms:contributor rdf:resource="https://orcid.org/0000-0002-4366-3088"/>
        <dcterms:contributor rdf:resource="https://orcid.org/0000-0003-4817-0423"/>
        <oboInOwl:created_by rdf:resource="https://orcid.org/0000-0002-1296-2528"/>
        <rdfs:label xml:lang="en">mechanical ecosystem management process</rdfs:label>
    </owl:Class>
    


    <!-- https://w3id.org/elmo/elmo_3620021 -->

    <owl:Class rdf:about="https://w3id.org/elmo/elmo_3620021">
        <rdfs:subClassOf rdf:resource="https://w3id.org/elmo/elmo_3620020"/>
        <obo:IAO_0000115 xml:lang="en">A mechanical ecosystem management process during which vegetation is removed.</obo:IAO_0000115>
        <dcterms:contributor rdf:resource="https://orcid.org/0000-0002-4366-3088"/>
        <dcterms:contributor rdf:resource="https://orcid.org/0000-0003-4817-0423"/>
        <oboInOwl:created_by rdf:resource="https://orcid.org/0000-0002-1296-2528"/>
        <rdfs:label xml:lang="en">mechanical vegetation removal process</rdfs:label>
    </owl:Class>
    


    <!-- https://w3id.org/elmo/elmo_3620022 -->

    <owl:Class rdf:about="https://w3id.org/elmo/elmo_3620022">
        <rdfs:subClassOf rdf:resource="https://w3id.org/elmo/elmo_3620021"/>
        <obo:IAO_0000115 xml:lang="en">A mechanical vegetation removal process in which a human employs a tool comprising a lever and gripping portion (root wrench).</obo:IAO_0000115>
        <dcterms:contributor rdf:resource="https://orcid.org/0000-0002-4366-3088"/>
        <dcterms:contributor rdf:resource="https://orcid.org/0000-0003-4817-0423"/>
        <oboInOwl:created_by rdf:resource="https://orcid.org/0000-0002-1296-2528"/>
        <rdfs:label xml:lang="en">root wrench removal process</rdfs:label>
    </owl:Class>
    


    <!-- https://w3id.org/elmo/elmo_3620023 -->

    <owl:Class rdf:about="https://w3id.org/elmo/elmo_3620023">
        <rdfs:subClassOf rdf:resource="https://w3id.org/elmo/elmo_3620021"/>
        <obo:IAO_0000115 xml:lang="en">A mechanical vegetation removal process during which plants at ground level are cut and residual stumps are covered with a sun-blocking material (e.g. silage tarp).</obo:IAO_0000115>
        <dcterms:contributor rdf:resource="https://orcid.org/0000-0002-4366-3088"/>
        <dcterms:contributor rdf:resource="https://orcid.org/0000-0003-4817-0423"/>
        <oboInOwl:created_by rdf:resource="https://orcid.org/0000-0002-1296-2528"/>
        <rdfs:label xml:lang="en">cut and cover removal process</rdfs:label>
    </owl:Class>
    


    <!-- https://w3id.org/elmo/elmo_3620024 -->

    <owl:Class rdf:about="https://w3id.org/elmo/elmo_3620024">
        <rdfs:subClassOf rdf:resource="https://w3id.org/elmo/elmo_3620021"/>
        <obo:IAO_0000115 xml:lang="en">A mechanical vegetation removal process in which a human cuts and removes plant material.</obo:IAO_0000115>
        <dcterms:contributor rdf:resource="https://orcid.org/0000-0002-4366-3088"/>
        <dcterms:contributor rdf:resource="https://orcid.org/0000-0003-4817-0423"/>
        <oboInOwl:created_by rdf:resource="https://orcid.org/0000-0002-1296-2528"/>
        <rdfs:label xml:lang="en">cutting removal process</rdfs:label>
    </owl:Class>
    


    <!-- https://w3id.org/elmo/elmo_3620025 -->

    <owl:Class rdf:about="https://w3id.org/elmo/elmo_3620025">
        <rdfs:subClassOf rdf:resource="https://w3id.org/elmo/elmo_3620021"/>
        <obo:IAO_0000115 xml:lang="en">A mechanical vegetation removal process in which a human severs subsoil roots using a spade and pries the plant out of the ground.</obo:IAO_0000115>
        <dcterms:contributor rdf:resource="https://orcid.org/0000-0002-4366-3088"/>
        <dcterms:contributor rdf:resource="https://orcid.org/0000-0003-4817-0423"/>
        <oboInOwl:created_by rdf:resource="https://orcid.org/0000-0002-1296-2528"/>
        <rdfs:label xml:lang="en">spading removal process</rdfs:label>
    </owl:Class>
    <owl:Axiom>
        <owl:annotatedSource rdf:resource="https://w3id.org/elmo/elmo_3620025"/>
        <owl:annotatedProperty rdf:resource="http://purl.obolibrary.org/obo/IAO_0000115"/>
        <owl:annotatedTarget xml:lang="en">A mechanical vegetation removal process in which a human severs subsoil roots using a spade and pries the plant out of the ground.</owl:annotatedTarget>
        <oboInOwl:hasDbXref rdf:resource="https://www.ontarioinvasiveplants.ca/wp-content/uploads/2018/05/OPWG-Spading-Postcard-1.pdf"/>
    </owl:Axiom>
    


    <!-- https://w3id.org/elmo/elmo_3620026 -->

    <owl:Class rdf:about="https://w3id.org/elmo/elmo_3620026">
        <rdfs:subClassOf rdf:resource="https://w3id.org/elmo/elmo_3620021"/>
        <obo:IAO_0000115 xml:lang="en">A mechanical vegetation removal process in which a human removes trees from a given area with the goal of reducing overall canopy cover thereby increasing light availability for understorey plants.</obo:IAO_0000115>
        <dcterms:contributor rdf:resource="https://orcid.org/0000-0002-4366-3088"/>
        <dcterms:contributor rdf:resource="https://orcid.org/0000-0003-4817-0423"/>
        <oboInOwl:created_by rdf:resource="https://orcid.org/0000-0002-1296-2528"/>
        <rdfs:label xml:lang="en">canopy thinning process</rdfs:label>
    </owl:Class>
    <owl:Axiom>
        <owl:annotatedSource rdf:resource="https://w3id.org/elmo/elmo_3620026"/>
        <owl:annotatedProperty rdf:resource="http://purl.obolibrary.org/obo/IAO_0000115"/>
        <owl:annotatedTarget xml:lang="en">A mechanical vegetation removal process in which a human removes trees from a given area with the goal of reducing overall canopy cover thereby increasing light availability for understorey plants.</owl:annotatedTarget>
        <oboInOwl:hasDbXref rdf:resource="doi:10.1111/rec.13043"/>
    </owl:Axiom>
    


    <!-- https://w3id.org/elmo/elmo_3620027 -->

    <owl:Class rdf:about="https://w3id.org/elmo/elmo_3620027">
        <rdfs:subClassOf rdf:resource="https://w3id.org/elmo/elmo_3620021"/>
        <obo:IAO_0000115 xml:lang="en">A mechanical vegetation removal process in which a human removes leaf litter from the ground thereby increasing the light availability for soil.</obo:IAO_0000115>
        <dcterms:contributor rdf:resource="https://orcid.org/0000-0002-4366-3088"/>
        <dcterms:contributor rdf:resource="https://orcid.org/0000-0003-4817-0423"/>
        <oboInOwl:created_by rdf:resource="https://orcid.org/0000-0002-1296-2528"/>
        <rdfs:label xml:lang="en">leaf litter removal process</rdfs:label>
    </owl:Class>
    


    <!-- https://w3id.org/elmo/elmo_3620028 -->

    <owl:Class rdf:about="https://w3id.org/elmo/elmo_3620028">
        <rdfs:subClassOf rdf:resource="https://w3id.org/elmo/elmo_3620020"/>
        <obo:IAO_0000115 xml:lang="en">A mechanical ecosystem management process in which a human controls fauna populations.</obo:IAO_0000115>
        <dcterms:contributor rdf:resource="https://orcid.org/0000-0002-4366-3088"/>
        <dcterms:contributor rdf:resource="https://orcid.org/0000-0003-4817-0423"/>
        <oboInOwl:created_by rdf:resource="https://orcid.org/0000-0002-1296-2528"/>
        <rdfs:label xml:lang="en">mechanical fauna control process</rdfs:label>
    </owl:Class>
    


    <!-- https://w3id.org/elmo/elmo_3620029 -->

    <owl:Class rdf:about="https://w3id.org/elmo/elmo_3620029">
        <rdfs:subClassOf rdf:resource="https://w3id.org/elmo/elmo_3620028"/>
        <obo:IAO_0000115 xml:lang="en">A mechanical fauna control process in which a human uses traps to control fauna.</obo:IAO_0000115>
        <dcterms:contributor rdf:resource="https://orcid.org/0000-0002-4366-3088"/>
        <dcterms:contributor rdf:resource="https://orcid.org/0000-0003-4817-0423"/>
        <oboInOwl:created_by rdf:resource="https://orcid.org/0000-0002-1296-2528"/>
        <rdfs:label xml:lang="en">mammal trapping process</rdfs:label>
    </owl:Class>
    <owl:Axiom>
        <owl:annotatedSource rdf:resource="https://w3id.org/elmo/elmo_3620029"/>
        <owl:annotatedProperty rdf:resource="http://purl.obolibrary.org/obo/IAO_0000115"/>
        <owl:annotatedTarget xml:lang="en">A mechanical fauna control process in which a human uses traps to control fauna.</owl:annotatedTarget>
        <oboInOwl:hasDbXref rdf:resource="https://en.wikipedia.org/wiki/Trapping"/>
    </owl:Axiom>
    


    <!-- https://w3id.org/elmo/elmo_3620030 -->

    <owl:Class rdf:about="https://w3id.org/elmo/elmo_3620030">
        <rdfs:subClassOf rdf:resource="https://w3id.org/elmo/elmo_3620028"/>
        <obo:IAO_0000115 xml:lang="en">A mechanical fauna control process in which a human targets predators for removal from the ecosystem.</obo:IAO_0000115>
        <dcterms:contributor rdf:resource="https://orcid.org/0000-0002-4366-3088"/>
        <dcterms:contributor rdf:resource="https://orcid.org/0000-0003-4817-0423"/>
        <oboInOwl:created_by rdf:resource="https://orcid.org/0000-0002-1296-2528"/>
        <rdfs:label xml:lang="en">predator control process</rdfs:label>
    </owl:Class>
    <owl:Axiom>
        <owl:annotatedSource rdf:resource="https://w3id.org/elmo/elmo_3620030"/>
        <owl:annotatedProperty rdf:resource="http://purl.obolibrary.org/obo/IAO_0000115"/>
        <owl:annotatedTarget xml:lang="en">A mechanical fauna control process in which a human targets predators for removal from the ecosystem.</owl:annotatedTarget>
        <oboInOwl:hasDbXref rdf:resource="https://agrilife.org/txwildlifeservices/files/2011/07/PredatorControlforWildlifeMgt.pdf"/>
    </owl:Axiom>
    


    <!-- https://w3id.org/elmo/elmo_3620031 -->

    <owl:Class rdf:about="https://w3id.org/elmo/elmo_3620031">
        <rdfs:subClassOf rdf:resource="https://w3id.org/elmo/elmo_3620067"/>
        <obo:IAO_0000115 xml:lang="en">A mechanical fauna control process in which a human installs fencing to restrict either immigration or emmigration of fauna from a particular area.</obo:IAO_0000115>
        <dcterms:contributor rdf:resource="https://orcid.org/0000-0002-4366-3088"/>
        <dcterms:contributor rdf:resource="https://orcid.org/0000-0003-4817-0423"/>
        <oboInOwl:created_by rdf:resource="https://orcid.org/0000-0002-1296-2528"/>
        <rdfs:label xml:lang="en">fencing process</rdfs:label>
    </owl:Class>
    <owl:Axiom>
        <owl:annotatedSource rdf:resource="https://w3id.org/elmo/elmo_3620031"/>
        <owl:annotatedProperty rdf:resource="http://purl.obolibrary.org/obo/IAO_0000115"/>
        <owl:annotatedTarget xml:lang="en">A mechanical fauna control process in which a human installs fencing to restrict either immigration or emmigration of fauna from a particular area.</owl:annotatedTarget>
        <oboInOwl:hasDbXref rdf:resource="doi:10.1016/j.biocon.2017.08.001"/>
    </owl:Axiom>
    


    <!-- https://w3id.org/elmo/elmo_3620032 -->

    <owl:Class rdf:about="https://w3id.org/elmo/elmo_3620032">
        <rdfs:subClassOf rdf:resource="https://w3id.org/elmo/elmo_3620028"/>
        <obo:IAO_0000115 xml:lang="en">A mechanical fauna control process in which a human installs an electronic device to deter species from a particular area.</obo:IAO_0000115>
        <dcterms:contributor rdf:resource="https://orcid.org/0000-0002-4366-3088"/>
        <dcterms:contributor rdf:resource="https://orcid.org/0000-0003-4817-0423"/>
        <oboInOwl:created_by rdf:resource="https://orcid.org/0000-0002-1296-2528"/>
        <rdfs:label xml:lang="en">mechanical species deterrent process</rdfs:label>
    </owl:Class>
    <owl:Axiom>
        <owl:annotatedSource rdf:resource="https://w3id.org/elmo/elmo_3620032"/>
        <owl:annotatedProperty rdf:resource="http://purl.obolibrary.org/obo/IAO_0000115"/>
        <owl:annotatedTarget xml:lang="en">A mechanical fauna control process in which a human installs an electronic device to deter species from a particular area.</owl:annotatedTarget>
        <oboInOwl:hasDbXref rdf:resource="doi:10.1111/jfb.13769"/>
    </owl:Axiom>
    


    <!-- https://w3id.org/elmo/elmo_3620033 -->

    <owl:Class rdf:about="https://w3id.org/elmo/elmo_3620033">
        <rdfs:subClassOf rdf:resource="https://w3id.org/elmo/elmo_3620020"/>
        <obo:IAO_0000115 xml:lang="en">A mechanical ecosystem management process during which a human deliberately alters the hydrologic cycle in an area.</obo:IAO_0000115>
        <dcterms:contributor rdf:resource="https://orcid.org/0000-0002-4366-3088"/>
        <dcterms:contributor rdf:resource="https://orcid.org/0000-0003-4817-0423"/>
        <oboInOwl:created_by rdf:resource="https://orcid.org/0000-0002-1296-2528"/>
        <rdfs:label xml:lang="en">mechanical hydrological alteration process</rdfs:label>
    </owl:Class>
    <owl:Axiom>
        <owl:annotatedSource rdf:resource="https://w3id.org/elmo/elmo_3620033"/>
        <owl:annotatedProperty rdf:resource="http://purl.obolibrary.org/obo/IAO_0000115"/>
        <owl:annotatedTarget xml:lang="en">A mechanical ecosystem management process during which a human deliberately alters the hydrologic cycle in an area.</owl:annotatedTarget>
        <oboInOwl:hasDbXref rdf:resource="https://en.wikipedia.org/wiki/Water_cycle"/>
    </owl:Axiom>
    


    <!-- https://w3id.org/elmo/elmo_3620034 -->

    <owl:Class rdf:about="https://w3id.org/elmo/elmo_3620034">
        <rdfs:subClassOf rdf:resource="https://w3id.org/elmo/elmo_3620033"/>
        <obo:IAO_0000115 xml:lang="en">A mechanical hydrological alteration process in which a human constructs some dam to restore a meander sequence to a river or stream.</obo:IAO_0000115>
        <dcterms:contributor rdf:resource="https://orcid.org/0000-0002-4366-3088"/>
        <dcterms:contributor rdf:resource="https://orcid.org/0000-0003-4817-0423"/>
        <oboInOwl:created_by rdf:resource="https://orcid.org/0000-0002-1296-2528"/>
        <oboInOwl:hasExactSynonym xml:lang="en">beaver dam analogue</oboInOwl:hasExactSynonym>
        <rdfs:label xml:lang="en">dam construction process</rdfs:label>
    </owl:Class>
    <owl:Axiom>
        <owl:annotatedSource rdf:resource="https://w3id.org/elmo/elmo_3620034"/>
        <owl:annotatedProperty rdf:resource="http://purl.obolibrary.org/obo/IAO_0000115"/>
        <owl:annotatedTarget xml:lang="en">A mechanical hydrological alteration process in which a human constructs some dam to restore a meander sequence to a river or stream.</owl:annotatedTarget>
        <oboInOwl:hasDbXref rdf:resource="doi:10.1093/biosci/biu036"/>
    </owl:Axiom>
    


    <!-- https://w3id.org/elmo/elmo_3620035 -->

    <owl:Class rdf:about="https://w3id.org/elmo/elmo_3620035">
        <rdfs:subClassOf rdf:resource="https://w3id.org/elmo/elmo_3620033"/>
        <obo:IAO_0000115 xml:lang="en">A mechanical hydrological alteration process in which a human removes some dam with the goal of altering the hydroperiod of surrounding lands and reconnecting rivers.</obo:IAO_0000115>
        <dcterms:contributor rdf:resource="https://orcid.org/0000-0002-4366-3088"/>
        <dcterms:contributor rdf:resource="https://orcid.org/0000-0003-4817-0423"/>
        <oboInOwl:created_by rdf:resource="https://orcid.org/0000-0002-1296-2528"/>
        <rdfs:label xml:lang="en">dam removal process</rdfs:label>
    </owl:Class>
    <owl:Axiom>
        <owl:annotatedSource rdf:resource="https://w3id.org/elmo/elmo_3620035"/>
        <owl:annotatedProperty rdf:resource="http://purl.obolibrary.org/obo/IAO_0000115"/>
        <owl:annotatedTarget xml:lang="en">A mechanical hydrological alteration process in which a human removes some dam with the goal of altering the hydroperiod of surrounding lands and reconnecting rivers.</owl:annotatedTarget>
        <oboInOwl:hasDbXref rdf:resource="doi:10.12952/journal.elementa.000108"/>
    </owl:Axiom>
    


    <!-- https://w3id.org/elmo/elmo_3620036 -->

    <owl:Class rdf:about="https://w3id.org/elmo/elmo_3620036">
        <rdfs:subClassOf rdf:resource="https://w3id.org/elmo/elmo_3620033"/>
        <obo:IAO_0000115 xml:lang="en">A mechanical hydrological alteration process in which a human uncovers and collapses subterranean tile drains in situ to reduce drainage on the landscape and restore wetland hydroperiod.</obo:IAO_0000115>
        <obo:IAO_0000116 xml:lang="en">This technique is actively practiced by the Nature Conservancy of Canada, but has not been documented in the literature yet.</obo:IAO_0000116>
        <dcterms:contributor rdf:resource="https://orcid.org/0000-0002-4366-3088"/>
        <dcterms:contributor rdf:resource="https://orcid.org/0000-0003-4817-0423"/>
        <oboInOwl:created_by rdf:resource="https://orcid.org/0000-0002-1296-2528"/>
        <rdfs:label xml:lang="en">tile drain crushing process</rdfs:label>
    </owl:Class>
    


    <!-- https://w3id.org/elmo/elmo_3620037 -->

    <owl:Class rdf:about="https://w3id.org/elmo/elmo_3620037">
        <rdfs:subClassOf rdf:resource="https://w3id.org/elmo/elmo_3620033"/>
        <obo:IAO_0000115 xml:lang="en">A mechanical hydrological alteration process in which a human uncovers and removes subterranean tile drains to reduce drainage on the landscape and restore wetland hydroperiod.</obo:IAO_0000115>
        <dcterms:contributor rdf:resource="https://orcid.org/0000-0002-4366-3088"/>
        <dcterms:contributor rdf:resource="https://orcid.org/0000-0003-4817-0423"/>
        <oboInOwl:created_by rdf:resource="https://orcid.org/0000-0002-1296-2528"/>
        <rdfs:label xml:lang="en">tile drain removal process</rdfs:label>
    </owl:Class>
    


    <!-- https://w3id.org/elmo/elmo_3620038 -->

    <owl:Class rdf:about="https://w3id.org/elmo/elmo_3620038">
        <rdfs:subClassOf rdf:resource="https://w3id.org/elmo/elmo_3620020"/>
        <obo:IAO_0000115 xml:lang="en">A mechanical ecosystem management process in which a human creates sites for fauna to breed, feed and shelter.</obo:IAO_0000115>
        <dcterms:contributor rdf:resource="https://orcid.org/0000-0002-4366-3088"/>
        <dcterms:contributor rdf:resource="https://orcid.org/0000-0003-4817-0423"/>
        <oboInOwl:created_by rdf:resource="https://orcid.org/0000-0002-1296-2528"/>
        <rdfs:label xml:lang="en">nest site creation process</rdfs:label>
    </owl:Class>
    <owl:Axiom>
        <owl:annotatedSource rdf:resource="https://w3id.org/elmo/elmo_3620038"/>
        <owl:annotatedProperty rdf:resource="http://purl.obolibrary.org/obo/IAO_0000115"/>
        <owl:annotatedTarget xml:lang="en">A mechanical ecosystem management process in which a human creates sites for fauna to breed, feed and shelter.</owl:annotatedTarget>
        <oboInOwl:hasDbXref rdf:resource="doi:10.1186/S41610-021-00192-Z"/>
    </owl:Axiom>
    


    <!-- https://w3id.org/elmo/elmo_3620039 -->

    <owl:Class rdf:about="https://w3id.org/elmo/elmo_3620039">
        <rdfs:subClassOf rdf:resource="https://w3id.org/elmo/elmo_3620020"/>
        <obo:IAO_0000115 xml:lang="en">A mechanical ecosystem management process in which a human creates places for birds to perch.</obo:IAO_0000115>
        <dcterms:contributor rdf:resource="https://orcid.org/0000-0002-4366-3088"/>
        <dcterms:contributor rdf:resource="https://orcid.org/0000-0003-4817-0423"/>
        <oboInOwl:created_by rdf:resource="https://orcid.org/0000-0002-1296-2528"/>
        <rdfs:label xml:lang="en">perch creation process</rdfs:label>
    </owl:Class>
    <owl:Axiom>
        <owl:annotatedSource rdf:resource="https://w3id.org/elmo/elmo_3620039"/>
        <owl:annotatedProperty rdf:resource="http://purl.obolibrary.org/obo/IAO_0000115"/>
        <owl:annotatedTarget xml:lang="en">A mechanical ecosystem management process in which a human creates places for birds to perch.</owl:annotatedTarget>
        <oboInOwl:hasDbXref rdf:resource="doi:10.1007/s11258-016-0619-4"/>
    </owl:Axiom>
    


    <!-- https://w3id.org/elmo/elmo_3620040 -->

    <owl:Class rdf:about="https://w3id.org/elmo/elmo_3620040">
        <rdfs:subClassOf rdf:resource="https://w3id.org/elmo/elmo_3620020"/>
        <obo:IAO_0000115 xml:lang="en">A mechanical ecosystem management process in which a human cultivates strips of flora between landscape features using earthworks and planting processes.</obo:IAO_0000115>
        <dcterms:contributor rdf:resource="https://orcid.org/0000-0002-4366-3088"/>
        <dcterms:contributor rdf:resource="https://orcid.org/0000-0003-4817-0423"/>
        <oboInOwl:created_by rdf:resource="https://orcid.org/0000-0002-1296-2528"/>
        <rdfs:label xml:lang="en">buffer strip creation process</rdfs:label>
    </owl:Class>
    <owl:Axiom>
        <owl:annotatedSource rdf:resource="https://w3id.org/elmo/elmo_3620040"/>
        <owl:annotatedProperty rdf:resource="http://purl.obolibrary.org/obo/IAO_0000115"/>
        <owl:annotatedTarget xml:lang="en">A mechanical ecosystem management process in which a human cultivates strips of flora between landscape features using earthworks and planting processes.</owl:annotatedTarget>
        <oboInOwl:hasDbXref rdf:resource="doi:10.2134/jeq2018.03.0120"/>
    </owl:Axiom>
    


    <!-- https://w3id.org/elmo/elmo_3620041 -->

    <owl:Class rdf:about="https://w3id.org/elmo/elmo_3620041">
        <rdfs:subClassOf rdf:resource="https://w3id.org/elmo/elmo_3620040"/>
        <obo:IAO_0000115 xml:lang="en">A mechanical ecosystem management process in which a human cultivates strips of flora in the riparian areas of rivers.</obo:IAO_0000115>
        <dcterms:contributor rdf:resource="https://orcid.org/0000-0002-4366-3088"/>
        <dcterms:contributor rdf:resource="https://orcid.org/0000-0003-4817-0423"/>
        <oboInOwl:created_by rdf:resource="https://orcid.org/0000-0002-1296-2528"/>
        <rdfs:label xml:lang="en">riparian buffer strip creation process</rdfs:label>
    </owl:Class>
    <owl:Axiom>
        <owl:annotatedSource rdf:resource="https://w3id.org/elmo/elmo_3620041"/>
        <owl:annotatedProperty rdf:resource="http://purl.obolibrary.org/obo/IAO_0000115"/>
        <owl:annotatedTarget xml:lang="en">A mechanical ecosystem management process in which a human cultivates strips of flora in the riparian areas of rivers.</owl:annotatedTarget>
        <oboInOwl:hasDbXref rdf:resource="doi:10.1890/08-2064.1"/>
    </owl:Axiom>
    


    <!-- https://w3id.org/elmo/elmo_3620042 -->

    <owl:Class rdf:about="https://w3id.org/elmo/elmo_3620042">
        <rdfs:subClassOf rdf:resource="https://w3id.org/elmo/elmo_3620020"/>
        <obo:IAO_0000115 xml:lang="en">A mechanical ecosystem management process in which a human leaves strips of flora untouched when clearing the land for other purposes.</obo:IAO_0000115>
        <dcterms:contributor rdf:resource="https://orcid.org/0000-0002-4366-3088"/>
        <dcterms:contributor rdf:resource="https://orcid.org/0000-0003-4817-0423"/>
        <oboInOwl:created_by rdf:resource="https://orcid.org/0000-0002-1296-2528"/>
        <rdfs:label xml:lang="en">buffer strip retention process</rdfs:label>
    </owl:Class>
    <owl:Axiom>
        <owl:annotatedSource rdf:resource="https://w3id.org/elmo/elmo_3620042"/>
        <owl:annotatedProperty rdf:resource="http://purl.obolibrary.org/obo/IAO_0000115"/>
        <owl:annotatedTarget xml:lang="en">A mechanical ecosystem management process in which a human leaves strips of flora untouched when clearing the land for other purposes.</owl:annotatedTarget>
        <oboInOwl:hasDbXref rdf:resource="doi:10.2134/jeq2018.03.0120"/>
    </owl:Axiom>
    


    <!-- https://w3id.org/elmo/elmo_3620043 -->

    <owl:Class rdf:about="https://w3id.org/elmo/elmo_3620043">
        <rdfs:subClassOf rdf:resource="https://w3id.org/elmo/elmo_3620020"/>
        <obo:IAO_0000115 xml:lang="en">A mechanical ecosystem management process during which the topology of some area is deliberately changed at least at the micro scale (e.g. 1m2).</obo:IAO_0000115>
        <obo:IAO_0000116 xml:lang="en">Difficult to suggest a firm border for scale. I doubt digging out a small hole would be called earthworks but settled on at least 1 m2 of earth moved. See Landscape Microscale Size and its associated scale properties for more nuance: ENVO:03620005; ENVO:03620006; ENVO:03620007; ENVO:03620008</obo:IAO_0000116>
        <dcterms:contributor rdf:resource="https://orcid.org/0000-0002-4366-3088"/>
        <dcterms:contributor rdf:resource="https://orcid.org/0000-0003-4817-0423"/>
        <oboInOwl:created_by rdf:resource="https://orcid.org/0000-0002-1296-2528"/>
        <rdfs:label xml:lang="en">earthworks process</rdfs:label>
    </owl:Class>
    


    <!-- https://w3id.org/elmo/elmo_3620044 -->

    <owl:Class rdf:about="https://w3id.org/elmo/elmo_3620044">
        <rdfs:subClassOf rdf:resource="https://w3id.org/elmo/elmo_3620043"/>
        <obo:IAO_0000115 xml:lang="en">An earthworks process in which earthen barriers (berms) are constructed with the goal of obstructing or slowing floodwaters.</obo:IAO_0000115>
        <dcterms:contributor rdf:resource="https://orcid.org/0000-0002-4366-3088"/>
        <dcterms:contributor rdf:resource="https://orcid.org/0000-0003-4817-0423"/>
        <oboInOwl:created_by rdf:resource="https://orcid.org/0000-0002-1296-2528"/>
        <rdfs:label xml:lang="en">berm creation process</rdfs:label>
    </owl:Class>
    <owl:Axiom>
        <owl:annotatedSource rdf:resource="https://w3id.org/elmo/elmo_3620044"/>
        <owl:annotatedProperty rdf:resource="http://purl.obolibrary.org/obo/IAO_0000115"/>
        <owl:annotatedTarget xml:lang="en">An earthworks process in which earthen barriers (berms) are constructed with the goal of obstructing or slowing floodwaters.</owl:annotatedTarget>
        <oboInOwl:hasDbXref rdf:resource="doi:10.1007/s11273-013-9285-7"/>
    </owl:Axiom>
    


    <!-- https://w3id.org/elmo/elmo_3620046 -->

    <owl:Class rdf:about="https://w3id.org/elmo/elmo_3620046">
        <rdfs:subClassOf rdf:resource="https://w3id.org/elmo/elmo_3620043"/>
        <obo:IAO_0000115 xml:lang="en">An earthworks process in which a human creates a pond.</obo:IAO_0000115>
        <dcterms:contributor rdf:resource="https://orcid.org/0000-0002-4366-3088"/>
        <dcterms:contributor rdf:resource="https://orcid.org/0000-0003-4817-0423"/>
        <oboInOwl:created_by rdf:resource="https://orcid.org/0000-0002-1296-2528"/>
        <rdfs:label xml:lang="en">pond creation process</rdfs:label>
    </owl:Class>
    <owl:Axiom>
        <owl:annotatedSource rdf:resource="https://w3id.org/elmo/elmo_3620046"/>
        <owl:annotatedProperty rdf:resource="http://purl.obolibrary.org/obo/IAO_0000115"/>
        <owl:annotatedTarget xml:lang="en">An earthworks process in which a human creates a pond.</owl:annotatedTarget>
        <oboInOwl:hasDbXref rdf:resource="doi:10.1007/s10531-021-02312-6"/>
    </owl:Axiom>
    


    <!-- https://w3id.org/elmo/elmo_3620047 -->

    <owl:Class rdf:about="https://w3id.org/elmo/elmo_3620047">
        <rdfs:subClassOf rdf:resource="https://w3id.org/elmo/elmo_3620043"/>
        <obo:IAO_0000115 xml:lang="en">An earthworks process in which a human reshapes the banks or basin of a pond.</obo:IAO_0000115>
        <dcterms:contributor rdf:resource="https://orcid.org/0000-0002-4366-3088"/>
        <dcterms:contributor rdf:resource="https://orcid.org/0000-0003-4817-0423"/>
        <oboInOwl:created_by rdf:resource="https://orcid.org/0000-0002-1296-2528"/>
        <rdfs:label xml:lang="en">pond reprofiling process</rdfs:label>
    </owl:Class>
    <owl:Axiom>
        <owl:annotatedSource rdf:resource="https://w3id.org/elmo/elmo_3620047"/>
        <owl:annotatedProperty rdf:resource="http://purl.obolibrary.org/obo/IAO_0000115"/>
        <owl:annotatedTarget xml:lang="en">An earthworks process in which a human reshapes the banks or basin of a pond.</owl:annotatedTarget>
        <oboInOwl:hasDbXref rdf:resource="doi:10.1016/j.jenvman.2024.120992"/>
    </owl:Axiom>
    


    <!-- https://w3id.org/elmo/elmo_3620048 -->

    <owl:Class rdf:about="https://w3id.org/elmo/elmo_3620048">
        <rdfs:subClassOf rdf:resource="https://w3id.org/elmo/elmo_3620043"/>
        <obo:IAO_0000115 xml:lang="en">An earthworks process in which a human alleviates the compaction of soil.</obo:IAO_0000115>
        <dcterms:contributor rdf:resource="https://orcid.org/0000-0002-4366-3088"/>
        <dcterms:contributor rdf:resource="https://orcid.org/0000-0003-4817-0423"/>
        <oboInOwl:created_by rdf:resource="https://orcid.org/0000-0002-1296-2528"/>
        <rdfs:label xml:lang="en">soil decompaction process</rdfs:label>
    </owl:Class>
    <owl:Axiom>
        <owl:annotatedSource rdf:resource="https://w3id.org/elmo/elmo_3620048"/>
        <owl:annotatedProperty rdf:resource="http://purl.obolibrary.org/obo/IAO_0000115"/>
        <owl:annotatedTarget xml:lang="en">An earthworks process in which a human alleviates the compaction of soil.</owl:annotatedTarget>
        <oboInOwl:hasDbXref rdf:resource="doi:10.1111/j.1526-100X.2008.00477.x"/>
    </owl:Axiom>
    


    <!-- https://w3id.org/elmo/elmo_3620049 -->

    <owl:Class rdf:about="https://w3id.org/elmo/elmo_3620049">
        <rdfs:subClassOf rdf:resource="https://w3id.org/elmo/elmo_3620048"/>
        <obo:IAO_0000115 xml:lang="en">An earthworks process in which a human breaks up the soil, and sometimes adds organic matter.</obo:IAO_0000115>
        <dcterms:contributor rdf:resource="https://orcid.org/0000-0002-4366-3088"/>
        <dcterms:contributor rdf:resource="https://orcid.org/0000-0003-4817-0423"/>
        <oboInOwl:created_by rdf:resource="https://orcid.org/0000-0002-1296-2528"/>
        <oboInOwl:hasNarrowSynonym xml:lang="en">soil ripping process</oboInOwl:hasNarrowSynonym>
        <rdfs:label xml:lang="en">tilling process</rdfs:label>
    </owl:Class>
    <owl:Axiom>
        <owl:annotatedSource rdf:resource="https://w3id.org/elmo/elmo_3620049"/>
        <owl:annotatedProperty rdf:resource="http://purl.obolibrary.org/obo/IAO_0000115"/>
        <owl:annotatedTarget xml:lang="en">An earthworks process in which a human breaks up the soil, and sometimes adds organic matter.</owl:annotatedTarget>
        <oboInOwl:hasDbXref rdf:resource="doi:10.1111/j.1526-100X.1995.tb00096.x"/>
    </owl:Axiom>
    


    <!-- https://w3id.org/elmo/elmo_3620050 -->

    <owl:Class rdf:about="https://w3id.org/elmo/elmo_3620050">
        <rdfs:subClassOf rdf:resource="https://w3id.org/elmo/elmo_3620048"/>
        <obo:IAO_0000115 xml:lang="en">An earthworks process in which a human deeply breaks up and overturns soil and vegetation.</obo:IAO_0000115>
        <dcterms:contributor rdf:resource="https://orcid.org/0000-0002-4366-3088"/>
        <dcterms:contributor rdf:resource="https://orcid.org/0000-0003-4817-0423"/>
        <oboInOwl:created_by rdf:resource="https://orcid.org/0000-0002-1296-2528"/>
        <rdfs:label xml:lang="en">ploughing process</rdfs:label>
    </owl:Class>
    <owl:Axiom>
        <owl:annotatedSource rdf:resource="https://w3id.org/elmo/elmo_3620050"/>
        <owl:annotatedProperty rdf:resource="http://purl.obolibrary.org/obo/IAO_0000115"/>
        <owl:annotatedTarget xml:lang="en">An earthworks process in which a human deeply breaks up and overturns soil and vegetation.</owl:annotatedTarget>
        <oboInOwl:hasDbXref rdf:resource="doi:10.1007/s12224-024-09448-7"/>
    </owl:Axiom>
    


    <!-- https://w3id.org/elmo/elmo_3620052 -->

    <owl:Class rdf:about="https://w3id.org/elmo/elmo_3620052">
        <rdfs:subClassOf rdf:resource="https://w3id.org/elmo/elmo_3620043"/>
        <obo:IAO_0000115 xml:lang="en">An earthworks process in which a human creates a specific slope.</obo:IAO_0000115>
        <dcterms:contributor rdf:resource="https://orcid.org/0000-0002-4366-3088"/>
        <dcterms:contributor rdf:resource="https://orcid.org/0000-0003-4817-0423"/>
        <oboInOwl:created_by rdf:resource="https://orcid.org/0000-0002-1296-2528"/>
        <rdfs:label xml:lang="en">grading process</rdfs:label>
    </owl:Class>
    <owl:Axiom>
        <owl:annotatedSource rdf:resource="https://w3id.org/elmo/elmo_3620052"/>
        <owl:annotatedProperty rdf:resource="http://purl.obolibrary.org/obo/IAO_0000115"/>
        <owl:annotatedTarget xml:lang="en">An earthworks process in which a human creates a specific slope.</owl:annotatedTarget>
        <oboInOwl:hasDbXref rdf:resource="https://en.wikipedia.org/wiki/Grading_(earthworks)"/>
    </owl:Axiom>
    


    <!-- https://w3id.org/elmo/elmo_3620053 -->

    <owl:Class rdf:about="https://w3id.org/elmo/elmo_3620053">
        <rdfs:subClassOf rdf:resource="https://w3id.org/elmo/elmo_3620043"/>
        <obo:IAO_0000115 xml:lang="en">An earthworks process in which a human installs inorganic material, usually a mesh, to stabilize a slope.</obo:IAO_0000115>
        <dcterms:contributor rdf:resource="https://orcid.org/0000-0002-4366-3088"/>
        <dcterms:contributor rdf:resource="https://orcid.org/0000-0003-4817-0423"/>
        <oboInOwl:created_by rdf:resource="https://orcid.org/0000-0002-1296-2528"/>
        <rdfs:label xml:lang="en">slope stabilization process</rdfs:label>
    </owl:Class>
    <owl:Axiom>
        <owl:annotatedSource rdf:resource="https://w3id.org/elmo/elmo_3620053"/>
        <owl:annotatedProperty rdf:resource="http://purl.obolibrary.org/obo/IAO_0000115"/>
        <owl:annotatedTarget xml:lang="en">An earthworks process in which a human installs inorganic material, usually a mesh, to stabilize a slope.</owl:annotatedTarget>
        <oboInOwl:hasDbXref rdf:resource="https://en.wikipedia.org/wiki/Cellular_confinement"/>
    </owl:Axiom>
    


    <!-- https://w3id.org/elmo/elmo_3620054 -->

    <owl:Class rdf:about="https://w3id.org/elmo/elmo_3620054">
        <rdfs:subClassOf rdf:resource="https://w3id.org/elmo/elmo_3620043"/>
        <obo:IAO_0000115 xml:lang="en">An earthworks process in which a human installs inorganic material, usually in a mesh, to stabilize a slope on the bank of a body of water.</obo:IAO_0000115>
        <dcterms:contributor rdf:resource="https://orcid.org/0000-0002-4366-3088"/>
        <dcterms:contributor rdf:resource="https://orcid.org/0000-0003-4817-0423"/>
        <oboInOwl:created_by rdf:resource="https://orcid.org/0000-0002-1296-2528"/>
        <rdfs:label xml:lang="en">shoreline reinforcement process</rdfs:label>
    </owl:Class>
    <owl:Axiom>
        <owl:annotatedSource rdf:resource="https://w3id.org/elmo/elmo_3620054"/>
        <owl:annotatedProperty rdf:resource="http://purl.obolibrary.org/obo/IAO_0000115"/>
        <owl:annotatedTarget xml:lang="en">An earthworks process in which a human installs inorganic material, usually in a mesh, to stabilize a slope on the bank of a body of water.</owl:annotatedTarget>
        <oboInOwl:hasDbXref rdf:resource="https://en.wikipedia.org/wiki/Cellular_confinement"/>
    </owl:Axiom>
    


    <!-- https://w3id.org/elmo/elmo_3620055 -->

    <owl:Class rdf:about="https://w3id.org/elmo/elmo_3620055">
        <rdfs:subClassOf rdf:resource="https://w3id.org/elmo/elmo_3620043"/>
        <obo:IAO_0000115 xml:lang="en">An earthworks process in which a human digs pits and creates mounds to reproduce a natural disturbance regime.</obo:IAO_0000115>
        <dcterms:contributor rdf:resource="https://orcid.org/0000-0002-4366-3088"/>
        <dcterms:contributor rdf:resource="https://orcid.org/0000-0003-4817-0423"/>
        <oboInOwl:created_by rdf:resource="https://orcid.org/0000-0002-1296-2528"/>
        <rdfs:label xml:lang="en">pit and mound excavation process</rdfs:label>
    </owl:Class>
    <owl:Axiom>
        <owl:annotatedSource rdf:resource="https://w3id.org/elmo/elmo_3620055"/>
        <owl:annotatedProperty rdf:resource="http://purl.obolibrary.org/obo/IAO_0000115"/>
        <owl:annotatedTarget xml:lang="en">An earthworks process in which a human digs pits and creates mounds to reproduce a natural disturbance regime.</owl:annotatedTarget>
        <oboInOwl:hasDbXref rdf:resource="doi:10.1016/j.foreco.2017.02.048"/>
    </owl:Axiom>
    


    <!-- https://w3id.org/elmo/elmo_3620056 -->

    <owl:Class rdf:about="https://w3id.org/elmo/elmo_3620056">
        <rdfs:subClassOf rdf:resource="https://w3id.org/elmo/elmo_3620043"/>
        <obo:IAO_0000115 xml:lang="en">An earthworks process in which a human realigns the channel of a stream by digging out replacement pathways and filling existing ones.</obo:IAO_0000115>
        <dcterms:contributor rdf:resource="https://orcid.org/0000-0002-4366-3088"/>
        <dcterms:contributor rdf:resource="https://orcid.org/0000-0003-4817-0423"/>
        <oboInOwl:created_by rdf:resource="https://orcid.org/0000-0002-1296-2528"/>
        <rdfs:label xml:lang="en">channel realignment process</rdfs:label>
    </owl:Class>
    <owl:Axiom>
        <owl:annotatedSource rdf:resource="https://w3id.org/elmo/elmo_3620056"/>
        <owl:annotatedProperty rdf:resource="http://purl.obolibrary.org/obo/IAO_0000115"/>
        <owl:annotatedTarget xml:lang="en">An earthworks process in which a human realigns the channel of a stream by digging out replacement pathways and filling existing ones.</owl:annotatedTarget>
        <oboInOwl:hasDbXref rdf:resource="https://streamhandbook.org/project/stream-channel-realignment/"/>
    </owl:Axiom>
    


    <!-- https://w3id.org/elmo/elmo_3620057 -->

    <owl:Class rdf:about="https://w3id.org/elmo/elmo_3620057">
        <rdfs:subClassOf rdf:resource="https://w3id.org/elmo/elmo_3620056"/>
        <obo:IAO_0000115 xml:lang="en">An earthworks process in which a human realigns the channel of a stream by digging out replacement pathways and filling existing ones with the goal of recreating a natural pool-riffle-pool meander sequence.</obo:IAO_0000115>
        <dcterms:contributor rdf:resource="https://orcid.org/0000-0002-4366-3088"/>
        <dcterms:contributor rdf:resource="https://orcid.org/0000-0003-4817-0423"/>
        <oboInOwl:created_by rdf:resource="https://orcid.org/0000-0002-1296-2528"/>
        <rdfs:label xml:lang="en">natural channel realignment process</rdfs:label>
    </owl:Class>
    <owl:Axiom>
        <owl:annotatedSource rdf:resource="https://w3id.org/elmo/elmo_3620057"/>
        <owl:annotatedProperty rdf:resource="http://purl.obolibrary.org/obo/IAO_0000115"/>
        <owl:annotatedTarget xml:lang="en">An earthworks process in which a human realigns the channel of a stream by digging out replacement pathways and filling existing ones with the goal of recreating a natural pool-riffle-pool meander sequence.</owl:annotatedTarget>
        <oboInOwl:hasDbXref rdf:resource="https://streamhandbook.org/project/stream-channel-realignment/"/>
    </owl:Axiom>
    


    <!-- https://w3id.org/elmo/elmo_3620058 -->

    <owl:Class rdf:about="https://w3id.org/elmo/elmo_3620058">
        <rdfs:subClassOf rdf:resource="https://w3id.org/elmo/elmo_3620043"/>
        <obo:IAO_0000115 xml:lang="en">An earthworks process in which a human removes the sediment layer of a water body.</obo:IAO_0000115>
        <dcterms:contributor rdf:resource="https://orcid.org/0000-0002-4366-3088"/>
        <dcterms:contributor rdf:resource="https://orcid.org/0000-0003-4817-0423"/>
        <oboInOwl:created_by rdf:resource="https://orcid.org/0000-0002-1296-2528"/>
        <rdfs:label xml:lang="en">dredging process</rdfs:label>
    </owl:Class>
    <owl:Axiom>
        <owl:annotatedSource rdf:resource="https://w3id.org/elmo/elmo_3620058"/>
        <owl:annotatedProperty rdf:resource="http://purl.obolibrary.org/obo/IAO_0000115"/>
        <owl:annotatedTarget xml:lang="en">An earthworks process in which a human removes the sediment layer of a water body.</owl:annotatedTarget>
        <oboInOwl:hasDbXref rdf:resource="https://en.wikipedia.org/wiki/Dredging"/>
    </owl:Axiom>
    


    <!-- https://w3id.org/elmo/elmo_3620059 -->

    <owl:Class rdf:about="https://w3id.org/elmo/elmo_3620059">
        <rdfs:subClassOf rdf:resource="https://w3id.org/elmo/elmo_3620020"/>
        <obo:IAO_0000115 xml:lang="en">A mechanical ecosystem management process in which a human creates a crossing (bridge or underpass) to help fauna pass through a barrier such as a road, fence or property.</obo:IAO_0000115>
        <dcterms:contributor rdf:resource="https://orcid.org/0000-0002-4366-3088"/>
        <dcterms:contributor rdf:resource="https://orcid.org/0000-0003-4817-0423"/>
        <oboInOwl:created_by rdf:resource="https://orcid.org/0000-0002-1296-2528"/>
        <rdfs:label xml:lang="en">fauna passage creation process</rdfs:label>
    </owl:Class>
    <owl:Axiom>
        <owl:annotatedSource rdf:resource="https://w3id.org/elmo/elmo_3620059"/>
        <owl:annotatedProperty rdf:resource="http://purl.obolibrary.org/obo/IAO_0000115"/>
        <owl:annotatedTarget xml:lang="en">A mechanical ecosystem management process in which a human creates a crossing (bridge or underpass) to help fauna pass through a barrier such as a road, fence or property.</owl:annotatedTarget>
        <oboInOwl:hasDbXref rdf:resource="https://en.wikipedia.org/wiki/Wildlife_crossing"/>
    </owl:Axiom>
    


    <!-- https://w3id.org/elmo/elmo_3620060 -->

    <owl:Class rdf:about="https://w3id.org/elmo/elmo_3620060">
        <rdfs:subClassOf rdf:resource="https://w3id.org/elmo/elmo_3620020"/>
        <obo:IAO_0000115 xml:lang="en">A mechanical ecosystem management process in which a human removes the topsoil layer.</obo:IAO_0000115>
        <dcterms:contributor rdf:resource="https://orcid.org/0000-0002-4366-3088"/>
        <dcterms:contributor rdf:resource="https://orcid.org/0000-0003-4817-0423"/>
        <oboInOwl:created_by rdf:resource="https://orcid.org/0000-0002-1296-2528"/>
        <rdfs:label xml:lang="en">topsoil removal process</rdfs:label>
    </owl:Class>
    <owl:Axiom>
        <owl:annotatedSource rdf:resource="https://w3id.org/elmo/elmo_3620060"/>
        <owl:annotatedProperty rdf:resource="http://purl.obolibrary.org/obo/IAO_0000115"/>
        <owl:annotatedTarget xml:lang="en">A mechanical ecosystem management process in which a human removes the topsoil layer.</owl:annotatedTarget>
        <oboInOwl:hasDbXref rdf:resource="doi:10.1111/avsc.12063"/>
    </owl:Axiom>
    


    <!-- https://w3id.org/elmo/elmo_3620061 -->

    <owl:Class rdf:about="https://w3id.org/elmo/elmo_3620061">
        <rdfs:subClassOf rdf:resource="https://w3id.org/elmo/elmo_3620043"/>
        <obo:IAO_0000115 xml:lang="en">A mechanical ecosystem management process in which a human installs some material to reduce erosion.</obo:IAO_0000115>
        <dcterms:contributor rdf:resource="https://orcid.org/0000-0002-4366-3088"/>
        <dcterms:contributor rdf:resource="https://orcid.org/0000-0003-4817-0423"/>
        <oboInOwl:created_by rdf:resource="https://orcid.org/0000-0002-1296-2528"/>
        <rdfs:label xml:lang="en">erosion control process</rdfs:label>
    </owl:Class>
    <owl:Axiom>
        <owl:annotatedSource rdf:resource="https://w3id.org/elmo/elmo_3620061"/>
        <owl:annotatedProperty rdf:resource="http://purl.obolibrary.org/obo/IAO_0000115"/>
        <owl:annotatedTarget xml:lang="en">A mechanical ecosystem management process in which a human installs some material to reduce erosion.</owl:annotatedTarget>
        <oboInOwl:hasDbXref rdf:resource="https://en.wikipedia.org/wiki/Erosion_control"/>
    </owl:Axiom>
    


    <!-- https://w3id.org/elmo/elmo_3620062 -->

    <owl:Class rdf:about="https://w3id.org/elmo/elmo_3620062">
        <rdfs:subClassOf rdf:resource="https://w3id.org/elmo/elmo_3620061"/>
        <obo:IAO_0000115 xml:lang="en">An erosion control process in which a human installs a textile.</obo:IAO_0000115>
        <dcterms:contributor rdf:resource="https://orcid.org/0000-0002-4366-3088"/>
        <dcterms:contributor rdf:resource="https://orcid.org/0000-0003-4817-0423"/>
        <oboInOwl:created_by rdf:resource="https://orcid.org/0000-0002-1296-2528"/>
        <rdfs:label xml:lang="en">erosion blanket process</rdfs:label>
    </owl:Class>
    


    <!-- https://w3id.org/elmo/elmo_3620063 -->

    <owl:Class rdf:about="https://w3id.org/elmo/elmo_3620063">
        <rdfs:subClassOf rdf:resource="https://w3id.org/elmo/elmo_3620061"/>
        <obo:IAO_0000115 xml:lang="en">An erosion control process in which a human installs a fence with a geotextile to restrict sediment transport.</obo:IAO_0000115>
        <dcterms:contributor rdf:resource="https://orcid.org/0000-0002-4366-3088"/>
        <dcterms:contributor rdf:resource="https://orcid.org/0000-0003-4817-0423"/>
        <oboInOwl:created_by rdf:resource="https://orcid.org/0000-0002-1296-2528"/>
        <rdfs:label xml:lang="en">erosion fencing process</rdfs:label>
    </owl:Class>
    <owl:Axiom>
        <owl:annotatedSource rdf:resource="https://w3id.org/elmo/elmo_3620063"/>
        <owl:annotatedProperty rdf:resource="http://purl.obolibrary.org/obo/IAO_0000115"/>
        <owl:annotatedTarget xml:lang="en">An erosion control process in which a human installs a fence with a geotextile to restrict sediment transport.</owl:annotatedTarget>
        <oboInOwl:hasDbXref rdf:resource="https://en.wikipedia.org/wiki/Silt_fence"/>
    </owl:Axiom>
    


    <!-- https://w3id.org/elmo/elmo_3620064 -->

    <owl:Class rdf:about="https://w3id.org/elmo/elmo_3620064">
        <rdfs:subClassOf rdf:resource="https://w3id.org/elmo/elmo_3620061"/>
        <obo:IAO_0000115 xml:lang="en">An erosion control process in which a human interleaves live materials to make short fencing along a slope.</obo:IAO_0000115>
        <dcterms:contributor rdf:resource="https://orcid.org/0000-0002-4366-3088"/>
        <dcterms:contributor rdf:resource="https://orcid.org/0000-0003-4817-0423"/>
        <oboInOwl:created_by rdf:resource="https://orcid.org/0000-0002-1296-2528"/>
        <rdfs:label xml:lang="en">wattle fencing process</rdfs:label>
    </owl:Class>
    <owl:Axiom>
        <owl:annotatedSource rdf:resource="https://w3id.org/elmo/elmo_3620064"/>
        <owl:annotatedProperty rdf:resource="http://purl.obolibrary.org/obo/IAO_0000115"/>
        <owl:annotatedTarget xml:lang="en">An erosion control process in which a human interleaves live materials to make short fencing along a slope.</owl:annotatedTarget>
        <oboInOwl:hasDbXref rdf:resource="https://hatchetnseed.ca/soil-bio-engineering-for-erosion-control/"/>
    </owl:Axiom>
    


    <!-- https://w3id.org/elmo/elmo_3620065 -->

    <owl:Class rdf:about="https://w3id.org/elmo/elmo_3620065">
        <rdfs:subClassOf rdf:resource="https://w3id.org/elmo/elmo_3620020"/>
        <obo:IAO_0000115 xml:lang="en">A mechanical ecosystem management process in which a human installs semi-permanent lines to supply a controlled amount of water to plants.</obo:IAO_0000115>
        <dcterms:contributor rdf:resource="https://orcid.org/0000-0002-4366-3088"/>
        <dcterms:contributor rdf:resource="https://orcid.org/0000-0003-4817-0423"/>
        <oboInOwl:created_by rdf:resource="https://orcid.org/0000-0002-1296-2528"/>
        <rdfs:label xml:lang="en">irrigation process</rdfs:label>
    </owl:Class>
    <owl:Axiom>
        <owl:annotatedSource rdf:resource="https://w3id.org/elmo/elmo_3620065"/>
        <owl:annotatedProperty rdf:resource="http://purl.obolibrary.org/obo/IAO_0000115"/>
        <owl:annotatedTarget xml:lang="en">A mechanical ecosystem management process in which a human installs semi-permanent lines to supply a controlled amount of water to plants.</owl:annotatedTarget>
        <oboInOwl:hasDbXref rdf:resource="https://en.wikipedia.org/wiki/Irrigation"/>
    </owl:Axiom>
    


    <!-- https://w3id.org/elmo/elmo_3620066 -->

    <owl:Class rdf:about="https://w3id.org/elmo/elmo_3620066">
        <rdfs:subClassOf rdf:resource="https://w3id.org/elmo/elmo_3620030"/>
        <obo:IAO_0000115 xml:lang="en">A predator control process in which a human installs a mechanical device designed to deter predators from a given area.</obo:IAO_0000115>
        <dcterms:contributor rdf:resource="https://orcid.org/0000-0002-4366-3088"/>
        <dcterms:contributor rdf:resource="https://orcid.org/0000-0003-4817-0423"/>
        <oboInOwl:created_by rdf:resource="https://orcid.org/0000-0002-1296-2528"/>
        <rdfs:label xml:lang="en">deterrence-focused predator control process</rdfs:label>
    </owl:Class>
    


    <!-- https://w3id.org/elmo/elmo_3620067 -->

    <owl:Class rdf:about="https://w3id.org/elmo/elmo_3620067">
        <rdfs:subClassOf rdf:resource="https://w3id.org/elmo/elmo_3620028"/>
        <obo:IAO_0000115 xml:lang="en">A mechanical fauna control process in which a human excludes fauna from a specific area.</obo:IAO_0000115>
        <dcterms:contributor rdf:resource="https://orcid.org/0000-0002-4366-3088"/>
        <dcterms:contributor rdf:resource="https://orcid.org/0000-0003-4817-0423"/>
        <oboInOwl:created_by rdf:resource="https://orcid.org/0000-0002-1296-2528"/>
        <rdfs:label xml:lang="en">fauna exclusion process</rdfs:label>
    </owl:Class>
    


    <!-- https://w3id.org/elmo/elmo_3620068 -->

    <owl:Class rdf:about="https://w3id.org/elmo/elmo_3620068">
        <rdfs:subClassOf rdf:resource="https://w3id.org/elmo/elmo_3620028"/>
        <obo:IAO_0000115 xml:lang="en">A mechanical fauna control process in which a human deters fauna from a specific area.</obo:IAO_0000115>
        <dcterms:contributor rdf:resource="https://orcid.org/0000-0002-4366-3088"/>
        <dcterms:contributor rdf:resource="https://orcid.org/0000-0003-4817-0423"/>
        <oboInOwl:created_by rdf:resource="https://orcid.org/0000-0002-1296-2528"/>
        <rdfs:label xml:lang="en">mechanical fauna deterrent process</rdfs:label>
    </owl:Class>
    


    <!-- https://w3id.org/elmo/elmo_3620069 -->

    <owl:Class rdf:about="https://w3id.org/elmo/elmo_3620069">
        <rdfs:subClassOf rdf:resource="https://w3id.org/elmo/elmo_3620028"/>
        <obo:IAO_0000115 xml:lang="en">A mechanical fauna control process in which a human captures fauna for the purposes of protecting existing organisms from some threat.</obo:IAO_0000115>
        <dcterms:contributor rdf:resource="https://orcid.org/0000-0002-4366-3088"/>
        <dcterms:contributor rdf:resource="https://orcid.org/0000-0003-4817-0423"/>
        <oboInOwl:created_by rdf:resource="https://orcid.org/0000-0002-1296-2528"/>
        <rdfs:label xml:lang="en">fauna capture for conservation</rdfs:label>
    </owl:Class>
    


    <!-- https://w3id.org/elmo/elmo_3620070 -->

    <owl:Class rdf:about="https://w3id.org/elmo/elmo_3620070">
        <rdfs:subClassOf rdf:resource="https://w3id.org/elmo/elmo_3620020"/>
        <obo:IAO_0000115 xml:lang="en">A mechanical ecosystem management process in which a human installs some means of bypassing hazards (e.g. dams) for fish.</obo:IAO_0000115>
        <dcterms:contributor rdf:resource="https://orcid.org/0000-0002-4366-3088"/>
        <dcterms:contributor rdf:resource="https://orcid.org/0000-0003-4817-0423"/>
        <oboInOwl:created_by rdf:resource="https://orcid.org/0000-0002-1296-2528"/>
        <rdfs:label xml:lang="en">fish bypass installation process</rdfs:label>
    </owl:Class>
    


    <!-- https://w3id.org/elmo/elmo_3620071 -->

    <owl:Class rdf:about="https://w3id.org/elmo/elmo_3620071">
        <rdfs:subClassOf rdf:resource="https://w3id.org/elmo/elmo_3620070"/>
        <obo:IAO_0000115 xml:lang="en">A fish bypass installation process in which a human installs a chute consisting of a series of stepped pools to allow fish to move past a dam.</obo:IAO_0000115>
        <dcterms:contributor rdf:resource="https://orcid.org/0000-0002-4366-3088"/>
        <dcterms:contributor rdf:resource="https://orcid.org/0000-0003-4817-0423"/>
        <oboInOwl:created_by rdf:resource="https://orcid.org/0000-0002-1296-2528"/>
        <rdfs:label xml:lang="en">fish ladder installation process</rdfs:label>
    </owl:Class>
    <owl:Axiom>
        <owl:annotatedSource rdf:resource="https://w3id.org/elmo/elmo_3620071"/>
        <owl:annotatedProperty rdf:resource="http://purl.obolibrary.org/obo/IAO_0000115"/>
        <owl:annotatedTarget xml:lang="en">A fish bypass installation process in which a human installs a chute consisting of a series of stepped pools to allow fish to move past a dam.</owl:annotatedTarget>
        <oboInOwl:hasDbXref rdf:resource="https://oceanservice.noaa.gov/facts/fish-ladder.html"/>
    </owl:Axiom>
    


    <!-- https://w3id.org/elmo/elmo_3620072 -->

    <owl:Class rdf:about="https://w3id.org/elmo/elmo_3620072">
        <rdfs:subClassOf rdf:resource="https://w3id.org/elmo/elmo_3620043"/>
        <obo:IAO_0000115 xml:lang="en">An earthworks process in which a human fills in a drainage ditch to restore the hydroperiod to a given area.</obo:IAO_0000115>
        <dcterms:contributor rdf:resource="https://orcid.org/0000-0002-4366-3088"/>
        <dcterms:contributor rdf:resource="https://orcid.org/0000-0003-4817-0423"/>
        <oboInOwl:created_by rdf:resource="https://orcid.org/0000-0002-1296-2528"/>
        <rdfs:label xml:lang="en">ditch plugging process</rdfs:label>
    </owl:Class>
    <owl:Axiom>
        <owl:annotatedSource rdf:resource="https://w3id.org/elmo/elmo_3620072"/>
        <owl:annotatedProperty rdf:resource="http://purl.obolibrary.org/obo/IAO_0000115"/>
        <owl:annotatedTarget xml:lang="en">An earthworks process in which a human fills in a drainage ditch to restore the hydroperiod to a given area.</owl:annotatedTarget>
        <oboInOwl:hasDbXref rdf:resource="https://www.ducks.ca/stories/biodiversity/years-in-the-making-for-record-breaking-conservation-project/"/>
    </owl:Axiom>
    


    <!-- https://w3id.org/elmo/elmo_3620073 -->

    <owl:Class rdf:about="https://w3id.org/elmo/elmo_3620073">
        <rdfs:subClassOf rdf:resource="https://w3id.org/elmo/elmo_3620043"/>
        <obo:IAO_0000115 xml:lang="en">An earthworks process in which a human adds sediment to a water body in order to modify the substrate composition.</obo:IAO_0000115>
        <dcterms:contributor rdf:resource="https://orcid.org/0000-0002-4366-3088"/>
        <dcterms:contributor rdf:resource="https://orcid.org/0000-0003-4817-0423"/>
        <oboInOwl:created_by rdf:resource="https://orcid.org/0000-0002-1296-2528"/>
        <rdfs:label xml:lang="en">sediment addition process</rdfs:label>
    </owl:Class>
    


    <!-- https://w3id.org/elmo/elmo_3620074 -->

    <owl:Class rdf:about="https://w3id.org/elmo/elmo_3620074">
        <rdfs:subClassOf rdf:resource="https://w3id.org/elmo/elmo_3620020"/>
        <obo:IAO_0000115 xml:lang="en">A mechanical ecosystem management process in which a human installs a barrier to protect newly planted flora from herbivory.</obo:IAO_0000115>
        <dcterms:contributor rdf:resource="https://orcid.org/0000-0002-4366-3088"/>
        <dcterms:contributor rdf:resource="https://orcid.org/0000-0003-4817-0423"/>
        <oboInOwl:created_by rdf:resource="https://orcid.org/0000-0002-1296-2528"/>
        <rdfs:label xml:lang="en">new plant protection process</rdfs:label>
    </owl:Class>
    


    <!-- https://w3id.org/elmo/elmo_3620500 -->

    <owl:Class rdf:about="https://w3id.org/elmo/elmo_3620500">
        <rdfs:subClassOf rdf:resource="http://purl.obolibrary.org/obo/ENVO_01001170"/>
        <obo:IAO_0000115 xml:lang="en">An active ecosystem management process in which a human applys or releases a chemical substance to realize some ecological management goal.</obo:IAO_0000115>
        <dcterms:contributor rdf:resource="https://orcid.org/0000-0002-4366-3088"/>
        <dcterms:contributor rdf:resource="https://orcid.org/0000-0003-4817-0423"/>
        <oboInOwl:created_by rdf:resource="https://orcid.org/0000-0002-1296-2528"/>
        <rdfs:label xml:lang="en">chemical ecosystem management process</rdfs:label>
    </owl:Class>
    <owl:Axiom>
        <owl:annotatedSource rdf:resource="https://w3id.org/elmo/elmo_3620500"/>
        <owl:annotatedProperty rdf:resource="http://purl.obolibrary.org/obo/IAO_0000115"/>
        <owl:annotatedTarget xml:lang="en">An active ecosystem management process in which a human applys or releases a chemical substance to realize some ecological management goal.</owl:annotatedTarget>
        <oboInOwl:hasDbXref rdf:resource="doi:10.1016/j.scitotenv.2021.148631"/>
    </owl:Axiom>
    


    <!-- https://w3id.org/elmo/elmo_3620501 -->

    <owl:Class rdf:about="https://w3id.org/elmo/elmo_3620501">
        <rdfs:subClassOf rdf:resource="https://w3id.org/elmo/elmo_3620500"/>
        <obo:IAO_0000115 xml:lang="en">A chemical ecosystem management process in which a human applies some chemical to an ecosystem.</obo:IAO_0000115>
        <dcterms:contributor rdf:resource="https://orcid.org/0000-0002-4366-3088"/>
        <dcterms:contributor rdf:resource="https://orcid.org/0000-0003-4817-0423"/>
        <oboInOwl:created_by rdf:resource="https://orcid.org/0000-0002-1296-2528"/>
        <rdfs:label xml:lang="en">chemical application process</rdfs:label>
    </owl:Class>
    <owl:Axiom>
        <owl:annotatedSource rdf:resource="https://w3id.org/elmo/elmo_3620501"/>
        <owl:annotatedProperty rdf:resource="http://purl.obolibrary.org/obo/IAO_0000115"/>
        <owl:annotatedTarget xml:lang="en">A chemical ecosystem management process in which a human applies some chemical to an ecosystem.</owl:annotatedTarget>
        <oboInOwl:hasDbXref rdf:resource="doi:10.1016/j.scitotenv.2021.148631"/>
    </owl:Axiom>
    


    <!-- https://w3id.org/elmo/elmo_3620502 -->

    <owl:Class rdf:about="https://w3id.org/elmo/elmo_3620502">
        <rdfs:subClassOf rdf:resource="https://w3id.org/elmo/elmo_3620501"/>
        <obo:IAO_0000115 xml:lang="en">A chemical application process in which a human applies chemical fertilizer to a given area with the goal of increasing the available carbon, nitrogen or phosphorous.</obo:IAO_0000115>
        <dcterms:contributor rdf:resource="https://orcid.org/0000-0002-4366-3088"/>
        <dcterms:contributor rdf:resource="https://orcid.org/0000-0003-4817-0423"/>
        <oboInOwl:created_by rdf:resource="https://orcid.org/0000-0002-1296-2528"/>
        <rdfs:label xml:lang="en">fertilizer application process</rdfs:label>
    </owl:Class>
    <owl:Axiom>
        <owl:annotatedSource rdf:resource="https://w3id.org/elmo/elmo_3620502"/>
        <owl:annotatedProperty rdf:resource="http://purl.obolibrary.org/obo/IAO_0000115"/>
        <owl:annotatedTarget xml:lang="en">A chemical application process in which a human applies chemical fertilizer to a given area with the goal of increasing the available carbon, nitrogen or phosphorous.</owl:annotatedTarget>
        <oboInOwl:hasDbXref rdf:resource="wd:Q1213511"/>
    </owl:Axiom>
    


    <!-- https://w3id.org/elmo/elmo_3620503 -->

    <owl:Class rdf:about="https://w3id.org/elmo/elmo_3620503">
        <rdfs:subClassOf rdf:resource="https://w3id.org/elmo/elmo_3620501"/>
        <obo:IAO_0000115 xml:lang="en">A chemical application process in which a human adds lime to soil or water in order to reduce the pH.</obo:IAO_0000115>
        <dcterms:contributor rdf:resource="https://orcid.org/0000-0002-4366-3088"/>
        <dcterms:contributor rdf:resource="https://orcid.org/0000-0003-4817-0423"/>
        <oboInOwl:created_by rdf:resource="https://orcid.org/0000-0002-1296-2528"/>
        <rdfs:label xml:lang="en">lime application process</rdfs:label>
    </owl:Class>
    <owl:Axiom>
        <owl:annotatedSource rdf:resource="https://w3id.org/elmo/elmo_3620503"/>
        <owl:annotatedProperty rdf:resource="http://purl.obolibrary.org/obo/IAO_0000115"/>
        <owl:annotatedTarget xml:lang="en">A chemical application process in which a human adds lime to soil or water in order to reduce the pH.</owl:annotatedTarget>
        <oboInOwl:hasDbXref rdf:resource="doi:10.1046/j.1365-2427.2001.00788.x"/>
    </owl:Axiom>
    


    <!-- https://w3id.org/elmo/elmo_3620504 -->

    <owl:Class rdf:about="https://w3id.org/elmo/elmo_3620504">
        <rdfs:subClassOf rdf:resource="https://w3id.org/elmo/elmo_3620501"/>
        <obo:IAO_0000115 xml:lang="en">A chemical application process in which a human applies herbicide to plants or soil in a given area.</obo:IAO_0000115>
        <dcterms:contributor rdf:resource="https://orcid.org/0000-0002-4366-3088"/>
        <dcterms:contributor rdf:resource="https://orcid.org/0000-0003-4817-0423"/>
        <oboInOwl:created_by rdf:resource="https://orcid.org/0000-0002-1296-2528"/>
        <rdfs:label xml:lang="en">herbicide application process</rdfs:label>
    </owl:Class>
    <owl:Axiom>
        <owl:annotatedSource rdf:resource="https://w3id.org/elmo/elmo_3620504"/>
        <owl:annotatedProperty rdf:resource="http://purl.obolibrary.org/obo/IAO_0000115"/>
        <owl:annotatedTarget xml:lang="en">A chemical application process in which a human applies herbicide to plants or soil in a given area.</owl:annotatedTarget>
        <oboInOwl:hasDbXref rdf:resource="doi:10.1111/avsc.12183"/>
    </owl:Axiom>
    


    <!-- https://w3id.org/elmo/elmo_3620505 -->

    <owl:Class rdf:about="https://w3id.org/elmo/elmo_3620505">
        <rdfs:subClassOf rdf:resource="https://w3id.org/elmo/elmo_3620501"/>
        <obo:IAO_0000115 xml:lang="en">A herbicide application process in which a human applies the herbicide glyphosate to plants in some area.</obo:IAO_0000115>
        <dcterms:contributor rdf:resource="https://orcid.org/0000-0002-4366-3088"/>
        <dcterms:contributor rdf:resource="https://orcid.org/0000-0003-4817-0423"/>
        <oboInOwl:created_by rdf:resource="https://orcid.org/0000-0002-1296-2528"/>
        <rdfs:label xml:lang="en">glyphosate application process</rdfs:label>
    </owl:Class>
    <owl:Axiom>
        <owl:annotatedSource rdf:resource="https://w3id.org/elmo/elmo_3620505"/>
        <owl:annotatedProperty rdf:resource="http://purl.obolibrary.org/obo/IAO_0000115"/>
        <owl:annotatedTarget xml:lang="en">A herbicide application process in which a human applies the herbicide glyphosate to plants in some area.</owl:annotatedTarget>
        <oboInOwl:hasDbXref rdf:resource="doi:10.1111/avsc.12183"/>
    </owl:Axiom>
    


    <!-- https://w3id.org/elmo/elmo_3620506 -->

    <owl:Class rdf:about="https://w3id.org/elmo/elmo_3620506">
        <rdfs:subClassOf rdf:resource="https://w3id.org/elmo/elmo_3620501"/>
        <obo:IAO_0000115 xml:lang="en">A chemical application process in which a human introduces an insecticide to some area with the goal of managing an insect population.</obo:IAO_0000115>
        <dcterms:contributor rdf:resource="https://orcid.org/0000-0002-4366-3088"/>
        <dcterms:contributor rdf:resource="https://orcid.org/0000-0003-4817-0423"/>
        <oboInOwl:created_by rdf:resource="https://orcid.org/0000-0002-1296-2528"/>
        <rdfs:label xml:lang="en">insecticide application process</rdfs:label>
    </owl:Class>
    <owl:Axiom>
        <owl:annotatedSource rdf:resource="https://w3id.org/elmo/elmo_3620506"/>
        <owl:annotatedProperty rdf:resource="http://purl.obolibrary.org/obo/IAO_0000115"/>
        <owl:annotatedTarget xml:lang="en">A chemical application process in which a human introduces an insecticide to some area with the goal of managing an insect population.</owl:annotatedTarget>
        <oboInOwl:hasDbXref rdf:resource="doi:10.1016/j.biocontrol.2018.07.012"/>
    </owl:Axiom>
    


    <!-- https://w3id.org/elmo/elmo_3620600 -->

    <owl:Class rdf:about="https://w3id.org/elmo/elmo_3620600">
        <rdfs:subClassOf rdf:resource="http://purl.obolibrary.org/obo/ENVO_01001170"/>
        <obo:IAO_0000115 xml:lang="en">An active ecosystem management process in which a human adds or removes biological material from an area to realize some ecological management goal.</obo:IAO_0000115>
        <dcterms:contributor rdf:resource="https://orcid.org/0000-0002-4366-3088"/>
        <dcterms:contributor rdf:resource="https://orcid.org/0000-0003-4817-0423"/>
        <oboInOwl:created_by rdf:resource="https://orcid.org/0000-0002-1296-2528"/>
        <rdfs:label xml:lang="en">biological ecosystem management process</rdfs:label>
    </owl:Class>
    


    <!-- https://w3id.org/elmo/elmo_3620601 -->

    <owl:Class rdf:about="https://w3id.org/elmo/elmo_3620601">
        <rdfs:subClassOf rdf:resource="https://w3id.org/elmo/elmo_3620600"/>
        <obo:IAO_0000115 xml:lang="en">A biological ecosystem management process in which a human plants flora (defined as at least having sprouted true leaves) in the soil of a given area.</obo:IAO_0000115>
        <dcterms:contributor rdf:resource="https://orcid.org/0000-0002-4366-3088"/>
        <dcterms:contributor rdf:resource="https://orcid.org/0000-0003-4817-0423"/>
        <oboInOwl:created_by rdf:resource="https://orcid.org/0000-0002-1296-2528"/>
        <rdfs:label xml:lang="en">planting process</rdfs:label>
    </owl:Class>
    


    <!-- https://w3id.org/elmo/elmo_3620602 -->

    <owl:Class rdf:about="https://w3id.org/elmo/elmo_3620602">
        <rdfs:subClassOf rdf:resource="https://w3id.org/elmo/elmo_3620601"/>
        <obo:IAO_0000115 xml:lang="en">A planting process in which a human plants flora grown in a plug tray.</obo:IAO_0000115>
        <dcterms:contributor rdf:resource="https://orcid.org/0000-0002-4366-3088"/>
        <dcterms:contributor rdf:resource="https://orcid.org/0000-0003-4817-0423"/>
        <oboInOwl:created_by rdf:resource="https://orcid.org/0000-0002-1296-2528"/>
        <rdfs:label xml:lang="en">plug planting process</rdfs:label>
    </owl:Class>
    <owl:Axiom>
        <owl:annotatedSource rdf:resource="https://w3id.org/elmo/elmo_3620602"/>
        <owl:annotatedProperty rdf:resource="http://purl.obolibrary.org/obo/IAO_0000115"/>
        <owl:annotatedTarget xml:lang="en">A planting process in which a human plants flora grown in a plug tray.</owl:annotatedTarget>
        <oboInOwl:hasDbXref rdf:resource="doi:10.1111/j.1526-100X.2007.00350.x"/>
    </owl:Axiom>
    


    <!-- https://w3id.org/elmo/elmo_3620603 -->

    <owl:Class rdf:about="https://w3id.org/elmo/elmo_3620603">
        <rdfs:subClassOf rdf:resource="https://w3id.org/elmo/elmo_3620601"/>
        <obo:IAO_0000115 xml:lang="en">A planting process in which a human plants shrubs.</obo:IAO_0000115>
        <dcterms:contributor rdf:resource="https://orcid.org/0000-0002-4366-3088"/>
        <dcterms:contributor rdf:resource="https://orcid.org/0000-0003-4817-0423"/>
        <oboInOwl:created_by rdf:resource="https://orcid.org/0000-0002-1296-2528"/>
        <rdfs:label xml:lang="en">shrub planting process</rdfs:label>
    </owl:Class>
    


    <!-- https://w3id.org/elmo/elmo_3620604 -->

    <owl:Class rdf:about="https://w3id.org/elmo/elmo_3620604">
        <rdfs:subClassOf rdf:resource="https://w3id.org/elmo/elmo_3620601"/>
        <obo:IAO_0000115 xml:lang="en">A planting process in which a human plants trees.</obo:IAO_0000115>
        <dcterms:contributor rdf:resource="https://orcid.org/0000-0002-4366-3088"/>
        <dcterms:contributor rdf:resource="https://orcid.org/0000-0003-4817-0423"/>
        <oboInOwl:created_by rdf:resource="https://orcid.org/0000-0002-1296-2528"/>
        <rdfs:label xml:lang="en">tree planting process</rdfs:label>
    </owl:Class>
    


    <!-- https://w3id.org/elmo/elmo_3620605 -->

    <owl:Class rdf:about="https://w3id.org/elmo/elmo_3620605">
        <rdfs:subClassOf rdf:resource="https://w3id.org/elmo/elmo_3620604"/>
        <obo:IAO_0000115 xml:lang="en">A planting process in which a human plants trees that have been grown in plug trays.</obo:IAO_0000115>
        <dcterms:contributor rdf:resource="https://orcid.org/0000-0002-4366-3088"/>
        <dcterms:contributor rdf:resource="https://orcid.org/0000-0003-4817-0423"/>
        <oboInOwl:created_by rdf:resource="https://orcid.org/0000-0002-1296-2528"/>
        <rdfs:label xml:lang="en">seedling planting process</rdfs:label>
    </owl:Class>
    


    <!-- https://w3id.org/elmo/elmo_3620606 -->

    <owl:Class rdf:about="https://w3id.org/elmo/elmo_3620606">
        <rdfs:subClassOf rdf:resource="https://w3id.org/elmo/elmo_3620604"/>
        <obo:IAO_0000115 xml:lang="en">A planting process in which a human plants trees that have grown to a diameter greater than 5 cm.</obo:IAO_0000115>
        <dcterms:contributor rdf:resource="https://orcid.org/0000-0002-4366-3088"/>
        <dcterms:contributor rdf:resource="https://orcid.org/0000-0003-4817-0423"/>
        <oboInOwl:created_by rdf:resource="https://orcid.org/0000-0002-1296-2528"/>
        <rdfs:label xml:lang="en">caliper tree planting process</rdfs:label>
    </owl:Class>
    


    <!-- https://w3id.org/elmo/elmo_3620607 -->

    <owl:Class rdf:about="https://w3id.org/elmo/elmo_3620607">
        <rdfs:subClassOf rdf:resource="https://w3id.org/elmo/elmo_3620601"/>
        <obo:IAO_0000115 xml:lang="en">A planting process in which a human inserts cut branches of a flora into soil such that that flora will take root and grow.</obo:IAO_0000115>
        <dcterms:contributor rdf:resource="https://orcid.org/0000-0002-4366-3088"/>
        <dcterms:contributor rdf:resource="https://orcid.org/0000-0003-4817-0423"/>
        <oboInOwl:created_by rdf:resource="https://orcid.org/0000-0002-1296-2528"/>
        <rdfs:label xml:lang="en">live staking process</rdfs:label>
    </owl:Class>
    


    <!-- https://w3id.org/elmo/elmo_3620608 -->

    <owl:Class rdf:about="https://w3id.org/elmo/elmo_3620608">
        <rdfs:subClassOf rdf:resource="https://w3id.org/elmo/elmo_3620601"/>
        <obo:IAO_0000115 xml:lang="en">A planting process in which a human plants flora with the goal of assisting the growth of other flora.</obo:IAO_0000115>
        <dcterms:contributor rdf:resource="https://orcid.org/0000-0002-4366-3088"/>
        <dcterms:contributor rdf:resource="https://orcid.org/0000-0003-4817-0423"/>
        <oboInOwl:created_by rdf:resource="https://orcid.org/0000-0002-1296-2528"/>
        <rdfs:label xml:lang="en">nurse plant process</rdfs:label>
    </owl:Class>
    <owl:Axiom>
        <owl:annotatedSource rdf:resource="https://w3id.org/elmo/elmo_3620608"/>
        <owl:annotatedProperty rdf:resource="http://purl.obolibrary.org/obo/IAO_0000115"/>
        <owl:annotatedTarget xml:lang="en">A planting process in which a human plants flora with the goal of assisting the growth of other flora.</owl:annotatedTarget>
        <oboInOwl:hasDbXref rdf:resource="doi:10.1890/03-5084"/>
    </owl:Axiom>
    


    <!-- https://w3id.org/elmo/elmo_3620609 -->

    <owl:Class rdf:about="https://w3id.org/elmo/elmo_3620609">
        <rdfs:subClassOf rdf:resource="https://w3id.org/elmo/elmo_3620600"/>
        <obo:IAO_0000115 xml:lang="en">A biological ecosystem management process in which a human sows seeds in a particular area.</obo:IAO_0000115>
        <dcterms:contributor rdf:resource="https://orcid.org/0000-0002-4366-3088"/>
        <dcterms:contributor rdf:resource="https://orcid.org/0000-0003-4817-0423"/>
        <oboInOwl:created_by rdf:resource="https://orcid.org/0000-0002-1296-2528"/>
        <rdfs:label xml:lang="en">seeding process</rdfs:label>
    </owl:Class>
    


    <!-- https://w3id.org/elmo/elmo_3620610 -->

    <owl:Class rdf:about="https://w3id.org/elmo/elmo_3620610">
        <rdfs:subClassOf rdf:resource="https://w3id.org/elmo/elmo_3620609"/>
        <obo:IAO_0000115 xml:lang="en">A seeding process in which a human sows tree seeds.</obo:IAO_0000115>
        <dcterms:contributor rdf:resource="https://orcid.org/0000-0002-4366-3088"/>
        <dcterms:contributor rdf:resource="https://orcid.org/0000-0003-4817-0423"/>
        <oboInOwl:created_by rdf:resource="https://orcid.org/0000-0002-1296-2528"/>
        <rdfs:label xml:lang="en">tree seeding process</rdfs:label>
    </owl:Class>
    


    <!-- https://w3id.org/elmo/elmo_3620611 -->

    <owl:Class rdf:about="https://w3id.org/elmo/elmo_3620611">
        <rdfs:subClassOf rdf:resource="https://w3id.org/elmo/elmo_3620609"/>
        <obo:IAO_0000115 xml:lang="en">A seeding process in which a human sows seeds in lines along a landscape.</obo:IAO_0000115>
        <dcterms:contributor rdf:resource="https://orcid.org/0000-0002-4366-3088"/>
        <dcterms:contributor rdf:resource="https://orcid.org/0000-0003-4817-0423"/>
        <oboInOwl:created_by rdf:resource="https://orcid.org/0000-0002-1296-2528"/>
        <rdfs:label xml:lang="en">line seeding process</rdfs:label>
    </owl:Class>
    


    <!-- https://w3id.org/elmo/elmo_3620612 -->

    <owl:Class rdf:about="https://w3id.org/elmo/elmo_3620612">
        <rdfs:subClassOf rdf:resource="https://w3id.org/elmo/elmo_3620609"/>
        <obo:IAO_0000115 xml:lang="en">A seeding process in which a human uses a drill seeder to sow seeds.</obo:IAO_0000115>
        <dcterms:contributor rdf:resource="https://orcid.org/0000-0002-4366-3088"/>
        <dcterms:contributor rdf:resource="https://orcid.org/0000-0003-4817-0423"/>
        <oboInOwl:created_by rdf:resource="https://orcid.org/0000-0002-1296-2528"/>
        <rdfs:label xml:lang="en">drill seeding process</rdfs:label>
    </owl:Class>
    <owl:Axiom>
        <owl:annotatedSource rdf:resource="https://w3id.org/elmo/elmo_3620612"/>
        <owl:annotatedProperty rdf:resource="http://purl.obolibrary.org/obo/IAO_0000115"/>
        <owl:annotatedTarget xml:lang="en">A seeding process in which a human uses a drill seeder to sow seeds.</owl:annotatedTarget>
        <oboInOwl:hasDbXref rdf:resource="doi:10.3375/043.038.0504"/>
    </owl:Axiom>
    


    <!-- https://w3id.org/elmo/elmo_3620613 -->

    <owl:Class rdf:about="https://w3id.org/elmo/elmo_3620613">
        <rdfs:subClassOf rdf:resource="https://w3id.org/elmo/elmo_3620609"/>
        <obo:IAO_0000115 xml:lang="en">A seeding process in which a human sows seeds by scattering them through the air.</obo:IAO_0000115>
        <dcterms:contributor rdf:resource="https://orcid.org/0000-0002-4366-3088"/>
        <dcterms:contributor rdf:resource="https://orcid.org/0000-0003-4817-0423"/>
        <oboInOwl:created_by rdf:resource="https://orcid.org/0000-0002-1296-2528"/>
        <rdfs:label xml:lang="en">broadcast seeding process</rdfs:label>
    </owl:Class>
    <owl:Axiom>
        <owl:annotatedSource rdf:resource="https://w3id.org/elmo/elmo_3620613"/>
        <owl:annotatedProperty rdf:resource="http://purl.obolibrary.org/obo/IAO_0000115"/>
        <owl:annotatedTarget xml:lang="en">A seeding process in which a human sows seeds by scattering them through the air.</owl:annotatedTarget>
        <oboInOwl:hasDbXref rdf:resource="doi:10.3375/043.038.0504"/>
    </owl:Axiom>
    


    <!-- https://w3id.org/elmo/elmo_3620614 -->

    <owl:Class rdf:about="https://w3id.org/elmo/elmo_3620614">
        <rdfs:subClassOf rdf:resource="https://w3id.org/elmo/elmo_3620613"/>
        <obo:IAO_0000115 xml:lang="en">A seeding process in which a human scatters seeds by hand.</obo:IAO_0000115>
        <dcterms:contributor rdf:resource="https://orcid.org/0000-0002-4366-3088"/>
        <dcterms:contributor rdf:resource="https://orcid.org/0000-0003-4817-0423"/>
        <oboInOwl:created_by rdf:resource="https://orcid.org/0000-0002-1296-2528"/>
        <rdfs:label xml:lang="en">hand broadcast seeding process</rdfs:label>
    </owl:Class>
    <owl:Axiom>
        <owl:annotatedSource rdf:resource="https://w3id.org/elmo/elmo_3620614"/>
        <owl:annotatedProperty rdf:resource="http://purl.obolibrary.org/obo/IAO_0000115"/>
        <owl:annotatedTarget xml:lang="en">A seeding process in which a human scatters seeds by hand.</owl:annotatedTarget>
        <oboInOwl:hasDbXref rdf:resource="doi:10.1111/j.1526-100X.2007.00350.x"/>
    </owl:Axiom>
    


    <!-- https://w3id.org/elmo/elmo_3620615 -->

    <owl:Class rdf:about="https://w3id.org/elmo/elmo_3620615">
        <rdfs:subClassOf rdf:resource="https://w3id.org/elmo/elmo_3620609"/>
        <obo:IAO_0000115 xml:lang="en">A seeding process in which a human applies seed in a slurry of nutrients and fixatives.</obo:IAO_0000115>
        <dcterms:contributor rdf:resource="https://orcid.org/0000-0002-4366-3088"/>
        <dcterms:contributor rdf:resource="https://orcid.org/0000-0003-4817-0423"/>
        <oboInOwl:created_by rdf:resource="https://orcid.org/0000-0002-1296-2528"/>
        <rdfs:label xml:lang="en">hydroseeding process</rdfs:label>
    </owl:Class>
    <owl:Axiom>
        <owl:annotatedSource rdf:resource="https://w3id.org/elmo/elmo_3620615"/>
        <owl:annotatedProperty rdf:resource="http://purl.obolibrary.org/obo/IAO_0000115"/>
        <owl:annotatedTarget xml:lang="en">A seeding process in which a human applies seed in a slurry of nutrients and fixatives.</owl:annotatedTarget>
        <oboInOwl:hasDbXref rdf:resource="doi:10.3375/043.038.0504"/>
    </owl:Axiom>
    


    <!-- https://w3id.org/elmo/elmo_3620616 -->

    <owl:Class rdf:about="https://w3id.org/elmo/elmo_3620616">
        <rdfs:subClassOf rdf:resource="https://w3id.org/elmo/elmo_3620600"/>
        <obo:IAO_0000115 xml:lang="en">A biological ecosystem management process in which a human applies a treatment to seed prior to sowing it.</obo:IAO_0000115>
        <dcterms:contributor rdf:resource="https://orcid.org/0000-0002-4366-3088"/>
        <dcterms:contributor rdf:resource="https://orcid.org/0000-0003-4817-0423"/>
        <oboInOwl:created_by rdf:resource="https://orcid.org/0000-0002-1296-2528"/>
        <rdfs:label xml:lang="en">seed treatment process</rdfs:label>
    </owl:Class>
    <owl:Axiom>
        <owl:annotatedSource rdf:resource="https://w3id.org/elmo/elmo_3620616"/>
        <owl:annotatedProperty rdf:resource="http://purl.obolibrary.org/obo/IAO_0000115"/>
        <owl:annotatedTarget xml:lang="en">A biological ecosystem management process in which a human applies a treatment to seed prior to sowing it.</owl:annotatedTarget>
        <oboInOwl:hasDbXref rdf:resource="doi:10.1111/rec.13210"/>
    </owl:Axiom>
    


    <!-- https://w3id.org/elmo/elmo_3620617 -->

    <owl:Class rdf:about="https://w3id.org/elmo/elmo_3620617">
        <rdfs:subClassOf rdf:resource="https://w3id.org/elmo/elmo_3620616"/>
        <obo:IAO_0000115 xml:lang="en">A seed treatment process in which a human damages the coating of the seed, usually using sandpaper, to enhance germination.</obo:IAO_0000115>
        <dcterms:contributor rdf:resource="https://orcid.org/0000-0002-4366-3088"/>
        <dcterms:contributor rdf:resource="https://orcid.org/0000-0003-4817-0423"/>
        <oboInOwl:created_by rdf:resource="https://orcid.org/0000-0002-1296-2528"/>
        <rdfs:label xml:lang="en">seed scarification process</rdfs:label>
    </owl:Class>
    <owl:Axiom>
        <owl:annotatedSource rdf:resource="https://w3id.org/elmo/elmo_3620617"/>
        <owl:annotatedProperty rdf:resource="http://purl.obolibrary.org/obo/IAO_0000115"/>
        <owl:annotatedTarget xml:lang="en">A seed treatment process in which a human damages the coating of the seed, usually using sandpaper, to enhance germination.</owl:annotatedTarget>
        <oboInOwl:hasDbXref rdf:resource="doi:10.1111/rec.13210"/>
    </owl:Axiom>
    


    <!-- https://w3id.org/elmo/elmo_3620618 -->

    <owl:Class rdf:about="https://w3id.org/elmo/elmo_3620618">
        <rdfs:subClassOf rdf:resource="https://w3id.org/elmo/elmo_3620616"/>
        <obo:IAO_0000115 xml:lang="en">A seed treatment process in which a human applies heat to some seed in order to enhance germination.</obo:IAO_0000115>
        <dcterms:contributor rdf:resource="https://orcid.org/0000-0002-4366-3088"/>
        <dcterms:contributor rdf:resource="https://orcid.org/0000-0003-4817-0423"/>
        <oboInOwl:created_by rdf:resource="https://orcid.org/0000-0002-1296-2528"/>
        <rdfs:label xml:lang="en">heat seed treatment process</rdfs:label>
    </owl:Class>
    <owl:Axiom>
        <owl:annotatedSource rdf:resource="https://w3id.org/elmo/elmo_3620618"/>
        <owl:annotatedProperty rdf:resource="http://purl.obolibrary.org/obo/IAO_0000115"/>
        <owl:annotatedTarget xml:lang="en">A seed treatment process in which a human applies heat to some seed in order to enhance germination.</owl:annotatedTarget>
        <oboInOwl:hasDbXref rdf:resource="doi:10.1111/rec.13210"/>
    </owl:Axiom>
    


    <!-- https://w3id.org/elmo/elmo_3620619 -->

    <owl:Class rdf:about="https://w3id.org/elmo/elmo_3620619">
        <rdfs:subClassOf rdf:resource="https://w3id.org/elmo/elmo_3620616"/>
        <obo:IAO_0000115 xml:lang="en">A seed treatment process in which a human applies cold to some seed in order to enhance germination, such as in cold stratification.</obo:IAO_0000115>
        <dcterms:contributor rdf:resource="https://orcid.org/0000-0002-4366-3088"/>
        <dcterms:contributor rdf:resource="https://orcid.org/0000-0003-4817-0423"/>
        <oboInOwl:created_by rdf:resource="https://orcid.org/0000-0002-1296-2528"/>
        <rdfs:label xml:lang="en">chill seed treatment process</rdfs:label>
    </owl:Class>
    <owl:Axiom>
        <owl:annotatedSource rdf:resource="https://w3id.org/elmo/elmo_3620619"/>
        <owl:annotatedProperty rdf:resource="http://purl.obolibrary.org/obo/IAO_0000115"/>
        <owl:annotatedTarget xml:lang="en">A seed treatment process in which a human applies cold to some seed in order to enhance germination, such as in cold stratification.</owl:annotatedTarget>
        <oboInOwl:hasDbXref rdf:resource="doi:10.1111/rec.13210"/>
    </owl:Axiom>
    


    <!-- https://w3id.org/elmo/elmo_3620620 -->

    <owl:Class rdf:about="https://w3id.org/elmo/elmo_3620620">
        <rdfs:subClassOf rdf:resource="https://w3id.org/elmo/elmo_3620616"/>
        <obo:IAO_0000115 xml:lang="en">A seed treatment process in which a human soaks seeds in order to enhance germination.</obo:IAO_0000115>
        <dcterms:contributor rdf:resource="https://orcid.org/0000-0002-4366-3088"/>
        <dcterms:contributor rdf:resource="https://orcid.org/0000-0003-4817-0423"/>
        <oboInOwl:created_by rdf:resource="https://orcid.org/0000-0002-1296-2528"/>
        <rdfs:label xml:lang="en">soak seed treatment process</rdfs:label>
    </owl:Class>
    <owl:Axiom>
        <owl:annotatedSource rdf:resource="https://w3id.org/elmo/elmo_3620620"/>
        <owl:annotatedProperty rdf:resource="http://purl.obolibrary.org/obo/IAO_0000115"/>
        <owl:annotatedTarget xml:lang="en">A seed treatment process in which a human soaks seeds in order to enhance germination.</owl:annotatedTarget>
        <oboInOwl:hasDbXref rdf:resource="doi:10.1111/rec.13210"/>
    </owl:Axiom>
    


    <!-- https://w3id.org/elmo/elmo_3620621 -->

    <owl:Class rdf:about="https://w3id.org/elmo/elmo_3620621">
        <rdfs:subClassOf rdf:resource="https://w3id.org/elmo/elmo_3620616"/>
        <obo:IAO_0000115 xml:lang="en">A seed treatment process in which light is applied to seeds in order to enhance germination.</obo:IAO_0000115>
        <dcterms:contributor rdf:resource="https://orcid.org/0000-0002-4366-3088"/>
        <dcterms:contributor rdf:resource="https://orcid.org/0000-0003-4817-0423"/>
        <oboInOwl:created_by rdf:resource="https://orcid.org/0000-0002-1296-2528"/>
        <rdfs:label xml:lang="en">light seed treatment process</rdfs:label>
    </owl:Class>
    <owl:Axiom>
        <owl:annotatedSource rdf:resource="https://w3id.org/elmo/elmo_3620621"/>
        <owl:annotatedProperty rdf:resource="http://purl.obolibrary.org/obo/IAO_0000115"/>
        <owl:annotatedTarget xml:lang="en">A seed treatment process in which light is applied to seeds in order to enhance germination.</owl:annotatedTarget>
        <oboInOwl:hasDbXref rdf:resource="doi:10.1111/rec.13210"/>
    </owl:Axiom>
    


    <!-- https://w3id.org/elmo/elmo_3620622 -->

    <owl:Class rdf:about="https://w3id.org/elmo/elmo_3620622">
        <rdfs:subClassOf rdf:resource="https://w3id.org/elmo/elmo_3620616"/>
        <obo:IAO_0000115 xml:lang="en">A seed treatment process in which some chemical is applied to some seed in order to enhance germination.</obo:IAO_0000115>
        <dcterms:contributor rdf:resource="https://orcid.org/0000-0002-4366-3088"/>
        <dcterms:contributor rdf:resource="https://orcid.org/0000-0003-4817-0423"/>
        <oboInOwl:created_by rdf:resource="https://orcid.org/0000-0002-1296-2528"/>
        <rdfs:label xml:lang="en">chemical seed treatment process</rdfs:label>
    </owl:Class>
    <owl:Axiom>
        <owl:annotatedSource rdf:resource="https://w3id.org/elmo/elmo_3620622"/>
        <owl:annotatedProperty rdf:resource="http://purl.obolibrary.org/obo/IAO_0000115"/>
        <owl:annotatedTarget xml:lang="en">A seed treatment process in which some chemical is applied to some seed in order to enhance germination.</owl:annotatedTarget>
        <oboInOwl:hasDbXref rdf:resource="doi:10.1111/rec.13210"/>
    </owl:Axiom>
    


    <!-- https://w3id.org/elmo/elmo_3620623 -->

    <owl:Class rdf:about="https://w3id.org/elmo/elmo_3620623">
        <rdfs:subClassOf rdf:resource="https://w3id.org/elmo/elmo_3620600"/>
        <obo:IAO_0000115 xml:lang="en">A biological ecosystem management process in which a human uses biological means to reduce or increase a population of fauna.</obo:IAO_0000115>
        <dcterms:contributor rdf:resource="https://orcid.org/0000-0002-4366-3088"/>
        <dcterms:contributor rdf:resource="https://orcid.org/0000-0003-4817-0423"/>
        <oboInOwl:created_by rdf:resource="https://orcid.org/0000-0002-1296-2528"/>
        <rdfs:label xml:lang="en">biological fauna control process</rdfs:label>
    </owl:Class>
    


    <!-- https://w3id.org/elmo/elmo_3620624 -->

    <owl:Class rdf:about="https://w3id.org/elmo/elmo_3620624">
        <rdfs:subClassOf rdf:resource="https://w3id.org/elmo/elmo_3620600"/>
        <obo:IAO_0000115 xml:lang="en">A biological ecosystem management process in which a human facilitates the breeding of fauna, rears the young for a period of time and releases them in some environment.</obo:IAO_0000115>
        <dcterms:contributor rdf:resource="https://orcid.org/0000-0002-4366-3088"/>
        <dcterms:contributor rdf:resource="https://orcid.org/0000-0003-4817-0423"/>
        <oboInOwl:created_by rdf:resource="https://orcid.org/0000-0002-1296-2528"/>
        <rdfs:label xml:lang="en">captive breeding and release process</rdfs:label>
    </owl:Class>
    <owl:Axiom>
        <owl:annotatedSource rdf:resource="https://w3id.org/elmo/elmo_3620624"/>
        <owl:annotatedProperty rdf:resource="http://purl.obolibrary.org/obo/IAO_0000115"/>
        <owl:annotatedTarget xml:lang="en">A biological ecosystem management process in which a human facilitates the breeding of fauna, rears the young for a period of time and releases them in some environment.</owl:annotatedTarget>
        <oboInOwl:hasDbXref rdf:resource="doi:10.1111/j.1523-1739.2008.00967.x"/>
    </owl:Axiom>
    


    <!-- https://w3id.org/elmo/elmo_3620625 -->

    <owl:Class rdf:about="https://w3id.org/elmo/elmo_3620625">
        <rdfs:subClassOf rdf:resource="https://w3id.org/elmo/elmo_3620624"/>
        <obo:IAO_0000115 xml:lang="en">A captive breeding and release process in which a human collects eggs and relocates them to a safe environment, whereupon they are allowed to hatch.</obo:IAO_0000115>
        <dcterms:contributor rdf:resource="https://orcid.org/0000-0002-4366-3088"/>
        <dcterms:contributor rdf:resource="https://orcid.org/0000-0003-4817-0423"/>
        <oboInOwl:created_by rdf:resource="https://orcid.org/0000-0002-1296-2528"/>
        <rdfs:label xml:lang="en">egg relocation and release process</rdfs:label>
    </owl:Class>
    


    <!-- https://w3id.org/elmo/elmo_3620626 -->

    <owl:Class rdf:about="https://w3id.org/elmo/elmo_3620626">
        <rdfs:subClassOf rdf:resource="https://w3id.org/elmo/elmo_3620625"/>
        <obo:IAO_0000115 xml:lang="en">An egg relocation and release process in which a human collects eggs and relocates them into an incubator, whereupon they are allowed to hatch and released into some environment.</obo:IAO_0000115>
        <dcterms:contributor rdf:resource="https://orcid.org/0000-0002-4366-3088"/>
        <dcterms:contributor rdf:resource="https://orcid.org/0000-0003-4817-0423"/>
        <oboInOwl:created_by rdf:resource="https://orcid.org/0000-0002-1296-2528"/>
        <rdfs:label xml:lang="en">egg incubation and release process</rdfs:label>
    </owl:Class>
    


    <!-- https://w3id.org/elmo/elmo_3620627 -->

    <owl:Class rdf:about="https://w3id.org/elmo/elmo_3620627">
        <rdfs:subClassOf rdf:resource="https://w3id.org/elmo/elmo_3620624"/>
        <obo:IAO_0000115 xml:lang="en">A captive breeding and release process in which a human captures young fauna, rears them into adulthood and releases them into some environment.</obo:IAO_0000115>
        <dcterms:contributor rdf:resource="https://orcid.org/0000-0002-4366-3088"/>
        <dcterms:contributor rdf:resource="https://orcid.org/0000-0003-4817-0423"/>
        <oboInOwl:created_by rdf:resource="https://orcid.org/0000-0002-1296-2528"/>
        <rdfs:label xml:lang="en">young capture, rearing and release</rdfs:label>
    </owl:Class>
    


    <!-- https://w3id.org/elmo/elmo_3620628 -->

    <owl:Class rdf:about="https://w3id.org/elmo/elmo_3620628">
        <rdfs:subClassOf rdf:resource="https://w3id.org/elmo/elmo_3620600"/>
        <obo:IAO_0000115 xml:lang="en">A biological ecosystem management process in which a human provides supplemental water to flora or fauna.</obo:IAO_0000115>
        <dcterms:contributor rdf:resource="https://orcid.org/0000-0002-4366-3088"/>
        <dcterms:contributor rdf:resource="https://orcid.org/0000-0003-4817-0423"/>
        <oboInOwl:created_by rdf:resource="https://orcid.org/0000-0002-1296-2528"/>
        <rdfs:label xml:lang="en">supplemental water process</rdfs:label>
    </owl:Class>
    


    <!-- https://w3id.org/elmo/elmo_3620629 -->

    <owl:Class rdf:about="https://w3id.org/elmo/elmo_3620629">
        <rdfs:subClassOf rdf:resource="https://w3id.org/elmo/elmo_3620600"/>
        <obo:IAO_0000115 xml:lang="en">A biological ecosystem management process in which a human provides supplemental food to fauna.</obo:IAO_0000115>
        <dcterms:contributor rdf:resource="https://orcid.org/0000-0002-4366-3088"/>
        <dcterms:contributor rdf:resource="https://orcid.org/0000-0003-4817-0423"/>
        <oboInOwl:created_by rdf:resource="https://orcid.org/0000-0002-1296-2528"/>
        <rdfs:label xml:lang="en">supplemental feeding process</rdfs:label>
    </owl:Class>
    


    <!-- https://w3id.org/elmo/elmo_3620630 -->

    <owl:Class rdf:about="https://w3id.org/elmo/elmo_3620630">
        <rdfs:subClassOf rdf:resource="https://w3id.org/elmo/elmo_3620600"/>
        <obo:IAO_0000115 xml:lang="en">A biological ecosystem management process in which a human transfers plant material from some area to another.</obo:IAO_0000115>
        <dcterms:contributor rdf:resource="https://orcid.org/0000-0002-4366-3088"/>
        <dcterms:contributor rdf:resource="https://orcid.org/0000-0003-4817-0423"/>
        <oboInOwl:created_by rdf:resource="https://orcid.org/0000-0002-1296-2528"/>
        <rdfs:label xml:lang="en">plant material transfer process</rdfs:label>
    </owl:Class>
    


    <!-- https://w3id.org/elmo/elmo_3620631 -->

    <owl:Class rdf:about="https://w3id.org/elmo/elmo_3620631">
        <rdfs:subClassOf rdf:resource="https://w3id.org/elmo/elmo_3620630"/>
        <obo:IAO_0000115 xml:lang="en">A plant material transfer process in which a human restores the hydroperiod of a peatland by blocking drainage ditches or other means and subsequently moves material from the moss layer (top 10 cm) of another peatland onto the one being restored.</obo:IAO_0000115>
        <dcterms:contributor rdf:resource="https://orcid.org/0000-0002-4366-3088"/>
        <dcterms:contributor rdf:resource="https://orcid.org/0000-0003-4817-0423"/>
        <oboInOwl:created_by rdf:resource="https://orcid.org/0000-0002-1296-2528"/>
        <rdfs:label xml:lang="en">moss layer transfer process</rdfs:label>
    </owl:Class>
    <owl:Axiom>
        <owl:annotatedSource rdf:resource="https://w3id.org/elmo/elmo_3620631"/>
        <owl:annotatedProperty rdf:resource="http://purl.obolibrary.org/obo/IAO_0000115"/>
        <owl:annotatedTarget xml:lang="en">A plant material transfer process in which a human restores the hydroperiod of a peatland by blocking drainage ditches or other means and subsequently moves material from the moss layer (top 10 cm) of another peatland onto the one being restored.</owl:annotatedTarget>
        <oboInOwl:hasDbXref rdf:resource="doi:10.1016/j.ecoleng.2014.03.051"/>
    </owl:Axiom>
    


    <!-- https://w3id.org/elmo/elmo_3620632 -->

    <owl:Class rdf:about="https://w3id.org/elmo/elmo_3620632">
        <rdfs:subClassOf rdf:resource="https://w3id.org/elmo/elmo_3620600"/>
        <obo:IAO_0000115 xml:lang="en">A biological ecosystem management process in which a human transfers soil from one area to another.</obo:IAO_0000115>
        <dcterms:contributor rdf:resource="https://orcid.org/0000-0002-4366-3088"/>
        <dcterms:contributor rdf:resource="https://orcid.org/0000-0003-4817-0423"/>
        <oboInOwl:created_by rdf:resource="https://orcid.org/0000-0002-1296-2528"/>
        <rdfs:label xml:lang="en">soil transfer process</rdfs:label>
    </owl:Class>
    


    <!-- https://w3id.org/elmo/elmo_3620633 -->

    <owl:Class rdf:about="https://w3id.org/elmo/elmo_3620633">
        <rdfs:subClassOf rdf:resource="https://w3id.org/elmo/elmo_3620623"/>
        <obo:IAO_0000115 xml:lang="en">A biological fauna control process in which a human renders some fauna sterile in order to reduce their population.</obo:IAO_0000115>
        <dcterms:contributor rdf:resource="https://orcid.org/0000-0002-4366-3088"/>
        <dcterms:contributor rdf:resource="https://orcid.org/0000-0003-4817-0423"/>
        <oboInOwl:created_by rdf:resource="https://orcid.org/0000-0002-1296-2528"/>
        <rdfs:label xml:lang="en">fauna sterilization process</rdfs:label>
    </owl:Class>
    


    <!-- https://w3id.org/elmo/elmo_3620634 -->

    <owl:Class rdf:about="https://w3id.org/elmo/elmo_3620634">
        <rdfs:subClassOf rdf:resource="https://w3id.org/elmo/elmo_3620623"/>
        <obo:IAO_0000115 xml:lang="en">A biological fauna control process in which a human destroys the eggs of some fauna (e.g. oiling goose eggs).</obo:IAO_0000115>
        <dcterms:contributor rdf:resource="https://orcid.org/0000-0002-4366-3088"/>
        <dcterms:contributor rdf:resource="https://orcid.org/0000-0003-4817-0423"/>
        <oboInOwl:created_by rdf:resource="https://orcid.org/0000-0002-1296-2528"/>
        <rdfs:label xml:lang="en">egg destruction process</rdfs:label>
    </owl:Class>
    


    <!-- https://w3id.org/elmo/elmo_3620635 -->

    <owl:Class rdf:about="https://w3id.org/elmo/elmo_3620635">
        <rdfs:subClassOf rdf:resource="https://w3id.org/elmo/elmo_3620623"/>
        <obo:IAO_0000115 xml:lang="en">A biological ecosystem management process in which a human implements measures to deter fauna from establishing nest sites in a given area.</obo:IAO_0000115>
        <dcterms:contributor rdf:resource="https://orcid.org/0000-0002-4366-3088"/>
        <dcterms:contributor rdf:resource="https://orcid.org/0000-0003-4817-0423"/>
        <oboInOwl:created_by rdf:resource="https://orcid.org/0000-0002-1296-2528"/>
        <rdfs:label xml:lang="en">nest establishment deterrence process</rdfs:label>
    </owl:Class>
    


    <!-- https://w3id.org/elmo/elmo_3620636 -->

    <owl:Class rdf:about="https://w3id.org/elmo/elmo_3620636">
        <rdfs:subClassOf rdf:resource="https://w3id.org/elmo/elmo_3620600"/>
        <obo:IAO_0000115 xml:lang="en">A biological ecosystem management process in which a human adds material to a seabed to facilitate nesting.</obo:IAO_0000115>
        <dcterms:contributor rdf:resource="https://orcid.org/0000-0002-4366-3088"/>
        <dcterms:contributor rdf:resource="https://orcid.org/0000-0003-4817-0423"/>
        <oboInOwl:created_by rdf:resource="https://orcid.org/0000-0002-1296-2528"/>
        <rdfs:label xml:lang="en">seabed amendment process</rdfs:label>
    </owl:Class>
    


    <!-- https://w3id.org/elmo/elmo_3620637 -->

    <owl:Class rdf:about="https://w3id.org/elmo/elmo_3620637">
        <rdfs:subClassOf rdf:resource="https://w3id.org/elmo/elmo_3620600"/>
        <obo:IAO_0000115 xml:lang="en">A biological ecosystem management process in which a human adds some material to soil.</obo:IAO_0000115>
        <dcterms:contributor rdf:resource="https://orcid.org/0000-0002-4366-3088"/>
        <dcterms:contributor rdf:resource="https://orcid.org/0000-0003-4817-0423"/>
        <oboInOwl:created_by rdf:resource="https://orcid.org/0000-0002-1296-2528"/>
        <rdfs:label xml:lang="en">soil amendment process</rdfs:label>
    </owl:Class>
    <owl:Axiom>
        <owl:annotatedSource rdf:resource="https://w3id.org/elmo/elmo_3620637"/>
        <owl:annotatedProperty rdf:resource="http://purl.obolibrary.org/obo/IAO_0000115"/>
        <owl:annotatedTarget xml:lang="en">A biological ecosystem management process in which a human adds some material to soil.</owl:annotatedTarget>
        <oboInOwl:hasDbXref rdf:resource="doi:10.2134/jeq2015.01.0009"/>
    </owl:Axiom>
    


    <!-- https://w3id.org/elmo/elmo_3620638 -->

    <owl:Class rdf:about="https://w3id.org/elmo/elmo_3620638">
        <rdfs:subClassOf rdf:resource="https://w3id.org/elmo/elmo_3620637"/>
        <obo:IAO_0000115 xml:lang="en">A soil amendment process in which a human adds mulch (i.e. woody debris).</obo:IAO_0000115>
        <dcterms:contributor rdf:resource="https://orcid.org/0000-0002-4366-3088"/>
        <dcterms:contributor rdf:resource="https://orcid.org/0000-0003-4817-0423"/>
        <oboInOwl:created_by rdf:resource="https://orcid.org/0000-0002-1296-2528"/>
        <rdfs:label xml:lang="en">mulch addition process</rdfs:label>
    </owl:Class>
    


    <!-- https://w3id.org/elmo/elmo_3620639 -->

    <owl:Class rdf:about="https://w3id.org/elmo/elmo_3620639">
        <rdfs:subClassOf rdf:resource="https://w3id.org/elmo/elmo_3620637"/>
        <obo:IAO_0000115 xml:lang="en">A soil amendment process in which a human adds peat.</obo:IAO_0000115>
        <dcterms:contributor rdf:resource="https://orcid.org/0000-0002-4366-3088"/>
        <dcterms:contributor rdf:resource="https://orcid.org/0000-0003-4817-0423"/>
        <oboInOwl:created_by rdf:resource="https://orcid.org/0000-0002-1296-2528"/>
        <rdfs:label xml:lang="en">peat addition process</rdfs:label>
    </owl:Class>
    


    <!-- https://w3id.org/elmo/elmo_3620640 -->

    <owl:Class rdf:about="https://w3id.org/elmo/elmo_3620640">
        <rdfs:subClassOf rdf:resource="https://w3id.org/elmo/elmo_3620637"/>
        <obo:IAO_0000115 xml:lang="en">A soil amendment process in which a human adds topsoil.</obo:IAO_0000115>
        <dcterms:contributor rdf:resource="https://orcid.org/0000-0002-4366-3088"/>
        <dcterms:contributor rdf:resource="https://orcid.org/0000-0003-4817-0423"/>
        <oboInOwl:created_by rdf:resource="https://orcid.org/0000-0002-1296-2528"/>
        <rdfs:label xml:lang="en">topsoil addition process</rdfs:label>
    </owl:Class>
    


    <!-- https://w3id.org/elmo/elmo_3620641 -->

    <owl:Class rdf:about="https://w3id.org/elmo/elmo_3620641">
        <rdfs:subClassOf rdf:resource="https://w3id.org/elmo/elmo_3620637"/>
        <obo:IAO_0000115 xml:lang="en">A soil amendment process in which a human adds some composted organic material.</obo:IAO_0000115>
        <dcterms:contributor rdf:resource="https://orcid.org/0000-0002-4366-3088"/>
        <dcterms:contributor rdf:resource="https://orcid.org/0000-0003-4817-0423"/>
        <oboInOwl:created_by rdf:resource="https://orcid.org/0000-0002-1296-2528"/>
        <rdfs:label xml:lang="en">compost addition process</rdfs:label>
    </owl:Class>
    <owl:Axiom>
        <owl:annotatedSource rdf:resource="https://w3id.org/elmo/elmo_3620641"/>
        <owl:annotatedProperty rdf:resource="http://purl.obolibrary.org/obo/IAO_0000115"/>
        <owl:annotatedTarget xml:lang="en">A soil amendment process in which a human adds some composted organic material.</owl:annotatedTarget>
        <oboInOwl:hasDbXref rdf:resource="doi:10.2134/jeq2015.01.0009"/>
    </owl:Axiom>
    


    <!-- https://w3id.org/elmo/elmo_3620642 -->

    <owl:Class rdf:about="https://w3id.org/elmo/elmo_3620642">
        <rdfs:subClassOf rdf:resource="https://w3id.org/elmo/elmo_3620637"/>
        <obo:IAO_0000115 xml:lang="en">A soil amendment process in which a human adds some manure.</obo:IAO_0000115>
        <dcterms:contributor rdf:resource="https://orcid.org/0000-0002-4366-3088"/>
        <dcterms:contributor rdf:resource="https://orcid.org/0000-0003-4817-0423"/>
        <oboInOwl:created_by rdf:resource="https://orcid.org/0000-0002-1296-2528"/>
        <rdfs:label xml:lang="en">manure addition process</rdfs:label>
    </owl:Class>
    <owl:Axiom>
        <owl:annotatedSource rdf:resource="https://w3id.org/elmo/elmo_3620642"/>
        <owl:annotatedProperty rdf:resource="http://purl.obolibrary.org/obo/IAO_0000115"/>
        <owl:annotatedTarget xml:lang="en">A soil amendment process in which a human adds some manure.</owl:annotatedTarget>
        <oboInOwl:hasDbXref rdf:resource="doi:10.2134/jeq2015.01.0009"/>
    </owl:Axiom>
    


    <!-- https://w3id.org/elmo/elmo_3620643 -->

    <owl:Class rdf:about="https://w3id.org/elmo/elmo_3620643">
        <rdfs:subClassOf rdf:resource="https://w3id.org/elmo/elmo_3620600"/>
        <obo:IAO_0000115 xml:lang="en">A biological ecosystem management process in which a human creates an artificial reef out of materials with the goal of attracting coral.</obo:IAO_0000115>
        <dcterms:contributor rdf:resource="https://orcid.org/0000-0002-4366-3088"/>
        <dcterms:contributor rdf:resource="https://orcid.org/0000-0003-4817-0423"/>
        <oboInOwl:created_by rdf:resource="https://orcid.org/0000-0002-1296-2528"/>
        <rdfs:label xml:lang="en">artificial reef creation process</rdfs:label>
    </owl:Class>
    <owl:Axiom>
        <owl:annotatedSource rdf:resource="https://w3id.org/elmo/elmo_3620643"/>
        <owl:annotatedProperty rdf:resource="http://purl.obolibrary.org/obo/IAO_0000115"/>
        <owl:annotatedTarget xml:lang="en">A biological ecosystem management process in which a human creates an artificial reef out of materials with the goal of attracting coral.</owl:annotatedTarget>
        <oboInOwl:hasDbXref rdf:resource="doi:10.1111/1365-2664.13748"/>
    </owl:Axiom>
    


    <!-- https://w3id.org/elmo/elmo_3620644 -->

    <owl:Class rdf:about="https://w3id.org/elmo/elmo_3620644">
        <rdfs:subClassOf rdf:resource="https://w3id.org/elmo/elmo_3620600"/>
        <obo:IAO_0000115 xml:lang="en">A biological ecosystem management process in which a human introduces grazing animals to an area with the goal of recreating a disturbance regime.</obo:IAO_0000115>
        <dcterms:contributor rdf:resource="https://orcid.org/0000-0002-4366-3088"/>
        <dcterms:contributor rdf:resource="https://orcid.org/0000-0003-4817-0423"/>
        <oboInOwl:created_by rdf:resource="https://orcid.org/0000-0002-1296-2528"/>
        <rdfs:label xml:lang="en">intentional grazing</rdfs:label>
    </owl:Class>
    <owl:Axiom>
        <owl:annotatedSource rdf:resource="https://w3id.org/elmo/elmo_3620644"/>
        <owl:annotatedProperty rdf:resource="http://purl.obolibrary.org/obo/IAO_0000115"/>
        <owl:annotatedTarget xml:lang="en">A biological ecosystem management process in which a human introduces grazing animals to an area with the goal of recreating a disturbance regime.</owl:annotatedTarget>
        <oboInOwl:hasDbXref rdf:resource="doi:10.1111/j.1526-100X.2009.00567.x"/>
    </owl:Axiom>
    


    <!-- https://w3id.org/elmo/elmo_3620645 -->

    <owl:Class rdf:about="https://w3id.org/elmo/elmo_3620645">
        <rdfs:subClassOf rdf:resource="https://w3id.org/elmo/elmo_3620600"/>
        <obo:IAO_0000115 xml:lang="en">A biological ecosystem management process in which a human adds mycorrhizae spores to some environment.</obo:IAO_0000115>
        <dcterms:contributor rdf:resource="https://orcid.org/0000-0002-4366-3088"/>
        <dcterms:contributor rdf:resource="https://orcid.org/0000-0003-4817-0423"/>
        <oboInOwl:created_by rdf:resource="https://orcid.org/0000-0002-1296-2528"/>
        <rdfs:label xml:lang="en">mycorrhizae addition process</rdfs:label>
    </owl:Class>
    <owl:Axiom>
        <owl:annotatedSource rdf:resource="https://w3id.org/elmo/elmo_3620645"/>
        <owl:annotatedProperty rdf:resource="http://purl.obolibrary.org/obo/IAO_0000115"/>
        <owl:annotatedTarget xml:lang="en">A biological ecosystem management process in which a human adds mycorrhizae spores to some environment.</owl:annotatedTarget>
        <oboInOwl:hasDbXref rdf:resource="doi:10.3389/fmicb.2016.01095"/>
    </owl:Axiom>
    


    <!-- https://w3id.org/elmo/elmo_3620646 -->

    <owl:Class rdf:about="https://w3id.org/elmo/elmo_3620646">
        <rdfs:subClassOf rdf:resource="https://w3id.org/elmo/elmo_3620600"/>
        <obo:IAO_0000115 xml:lang="en">A biological ecosystem management process in which a human alters the hydroperiod of a peatland such that more water is available.</obo:IAO_0000115>
        <dcterms:contributor rdf:resource="https://orcid.org/0000-0002-4366-3088"/>
        <dcterms:contributor rdf:resource="https://orcid.org/0000-0003-4817-0423"/>
        <oboInOwl:created_by rdf:resource="https://orcid.org/0000-0002-1296-2528"/>
        <rdfs:label xml:lang="en">peatland rewetting process</rdfs:label>
    </owl:Class>
    <owl:Axiom>
        <owl:annotatedSource rdf:resource="https://w3id.org/elmo/elmo_3620646"/>
        <owl:annotatedProperty rdf:resource="http://purl.obolibrary.org/obo/IAO_0000115"/>
        <owl:annotatedTarget xml:lang="en">A biological ecosystem management process in which a human alters the hydroperiod of a peatland such that more water is available.</owl:annotatedTarget>
        <oboInOwl:hasDbXref rdf:resource="doi:10.1007/s11027-023-10046-9"/>
    </owl:Axiom>
    


    <!-- https://w3id.org/elmo/elmo_3620647 -->

    <owl:Class rdf:about="https://w3id.org/elmo/elmo_3620647">
        <rdfs:subClassOf rdf:resource="https://w3id.org/elmo/elmo_3620623"/>
        <obo:IAO_0000115 xml:lang="en">A biological fauna control process in which a human captures injured fauna from some environment, rehabilitates and releases them.</obo:IAO_0000115>
        <dcterms:contributor rdf:resource="https://orcid.org/0000-0002-4366-3088"/>
        <dcterms:contributor rdf:resource="https://orcid.org/0000-0003-4817-0423"/>
        <oboInOwl:created_by rdf:resource="https://orcid.org/0000-0002-1296-2528"/>
        <rdfs:label xml:lang="en">fauna rescue, rehabilitation and release process</rdfs:label>
    </owl:Class>
    <owl:Axiom>
        <owl:annotatedSource rdf:resource="https://w3id.org/elmo/elmo_3620647"/>
        <owl:annotatedProperty rdf:resource="http://purl.obolibrary.org/obo/IAO_0000115"/>
        <owl:annotatedTarget xml:lang="en">A biological fauna control process in which a human captures injured fauna from some environment, rehabilitates and releases them.</owl:annotatedTarget>
        <oboInOwl:hasDbXref rdf:resource="doi:10.1371/journal.pone.0265514"/>
    </owl:Axiom>
    


    <!-- https://w3id.org/elmo/elmo_3620648 -->

    <owl:Class rdf:about="https://w3id.org/elmo/elmo_3620648">
        <rdfs:subClassOf rdf:resource="https://w3id.org/elmo/elmo_3620623"/>
        <obo:IAO_0000115 xml:lang="en">A biological fauna control process in which a human reintroduces fauna into some environment where the fauna once existed.</obo:IAO_0000115>
        <dcterms:contributor rdf:resource="https://orcid.org/0000-0002-4366-3088"/>
        <dcterms:contributor rdf:resource="https://orcid.org/0000-0003-4817-0423"/>
        <oboInOwl:created_by rdf:resource="https://orcid.org/0000-0002-1296-2528"/>
        <rdfs:label xml:lang="en">fauna reintroduction process</rdfs:label>
    </owl:Class>
    


    <!-- https://w3id.org/elmo/elmo_3620649 -->

    <owl:Class rdf:about="https://w3id.org/elmo/elmo_3620649">
        <rdfs:subClassOf rdf:resource="https://w3id.org/elmo/elmo_3620623"/>
        <obo:IAO_0000115 xml:lang="en">A biological fauna control process in which a human provides medical care to some fauna.</obo:IAO_0000115>
        <dcterms:contributor rdf:resource="https://orcid.org/0000-0002-4366-3088"/>
        <dcterms:contributor rdf:resource="https://orcid.org/0000-0003-4817-0423"/>
        <oboInOwl:created_by rdf:resource="https://orcid.org/0000-0002-1296-2528"/>
        <rdfs:label xml:lang="en">fauna medical care process</rdfs:label>
    </owl:Class>
    


    <!-- https://w3id.org/elmo/elmo_3620650 -->

    <owl:Class rdf:about="https://w3id.org/elmo/elmo_3620650">
        <rdfs:subClassOf rdf:resource="https://w3id.org/elmo/elmo_3620600"/>
        <obo:IAO_0000115 xml:lang="en">A biological ecosystem management process in which a human translocates some flora or fauna from one area to another.</obo:IAO_0000115>
        <dcterms:contributor rdf:resource="https://orcid.org/0000-0002-4366-3088"/>
        <dcterms:contributor rdf:resource="https://orcid.org/0000-0003-4817-0423"/>
        <oboInOwl:created_by rdf:resource="https://orcid.org/0000-0002-1296-2528"/>
        <rdfs:label xml:lang="en">translocation process</rdfs:label>
    </owl:Class>
    


    <!-- https://w3id.org/elmo/elmo_3620651 -->

    <owl:Class rdf:about="https://w3id.org/elmo/elmo_3620651">
        <rdfs:subClassOf rdf:resource="https://w3id.org/elmo/elmo_3620650"/>
        <obo:IAO_0000115 xml:lang="en">A translocation process in which a human translocates some fauna from one area to another.</obo:IAO_0000115>
        <dcterms:contributor rdf:resource="https://orcid.org/0000-0002-4366-3088"/>
        <dcterms:contributor rdf:resource="https://orcid.org/0000-0003-4817-0423"/>
        <oboInOwl:created_by rdf:resource="https://orcid.org/0000-0002-1296-2528"/>
        <rdfs:label xml:lang="en">fauna translocation process</rdfs:label>
    </owl:Class>
    


    <!-- https://w3id.org/elmo/elmo_3620652 -->

    <owl:Class rdf:about="https://w3id.org/elmo/elmo_3620652">
        <rdfs:subClassOf rdf:resource="https://w3id.org/elmo/elmo_3620650"/>
        <obo:IAO_0000115 xml:lang="en">A translocation process in which a human translocates coral from one area to another.</obo:IAO_0000115>
        <dcterms:contributor rdf:resource="https://orcid.org/0000-0002-4366-3088"/>
        <dcterms:contributor rdf:resource="https://orcid.org/0000-0003-4817-0423"/>
        <oboInOwl:created_by rdf:resource="https://orcid.org/0000-0002-1296-2528"/>
        <rdfs:label xml:lang="en">coral translocation process</rdfs:label>
    </owl:Class>
    <owl:Axiom>
        <owl:annotatedSource rdf:resource="https://w3id.org/elmo/elmo_3620652"/>
        <owl:annotatedProperty rdf:resource="http://purl.obolibrary.org/obo/IAO_0000115"/>
        <owl:annotatedTarget xml:lang="en">A translocation process in which a human translocates coral from one area to another.</owl:annotatedTarget>
        <oboInOwl:hasDbXref rdf:resource="doi:10.3389/fmars.2019.00540"/>
    </owl:Axiom>
    


    <!-- https://w3id.org/elmo/elmo_3620800 -->

    <owl:Class rdf:about="https://w3id.org/elmo/elmo_3620800">
        <rdfs:subClassOf rdf:resource="http://purl.obolibrary.org/obo/ENVO_02500000"/>
        <obo:IAO_0000115 xml:lang="en">An environmental system process in which a human employs social means to realize some ecosystem management goal.</obo:IAO_0000115>
        <dcterms:contributor rdf:resource="https://orcid.org/0000-0002-4366-3088"/>
        <dcterms:contributor rdf:resource="https://orcid.org/0000-0003-4817-0423"/>
        <oboInOwl:created_by rdf:resource="https://orcid.org/0000-0002-1296-2528"/>
        <rdfs:label xml:lang="en">ecosystem-oriented social process</rdfs:label>
    </owl:Class>
    


    <!-- https://w3id.org/elmo/elmo_3620801 -->

    <owl:Class rdf:about="https://w3id.org/elmo/elmo_3620801">
        <rdfs:subClassOf rdf:resource="https://w3id.org/elmo/elmo_3620800"/>
        <obo:IAO_0000115 xml:lang="en">A ecosystem-oriented social process in which a humans collectively implement legislation with pro-environmental goals.</obo:IAO_0000115>
        <dcterms:contributor rdf:resource="https://orcid.org/0000-0002-4366-3088"/>
        <dcterms:contributor rdf:resource="https://orcid.org/0000-0003-4817-0423"/>
        <oboInOwl:created_by rdf:resource="https://orcid.org/0000-0002-1296-2528"/>
        <rdfs:label xml:lang="en">legislation process</rdfs:label>
    </owl:Class>
    


    <!-- https://w3id.org/elmo/elmo_3620802 -->

    <owl:Class rdf:about="https://w3id.org/elmo/elmo_3620802">
        <rdfs:subClassOf rdf:resource="https://w3id.org/elmo/elmo_3620801"/>
        <obo:IAO_0000115 xml:lang="en">A legislation process in which the legislation explicitly protects something from degradation.</obo:IAO_0000115>
        <dcterms:contributor rdf:resource="https://orcid.org/0000-0002-4366-3088"/>
        <dcterms:contributor rdf:resource="https://orcid.org/0000-0003-4817-0423"/>
        <oboInOwl:created_by rdf:resource="https://orcid.org/0000-0002-1296-2528"/>
        <rdfs:label xml:lang="en">legal protection process</rdfs:label>
    </owl:Class>
    


    <!-- https://w3id.org/elmo/elmo_3620803 -->

    <owl:Class rdf:about="https://w3id.org/elmo/elmo_3620803">
        <rdfs:subClassOf rdf:resource="https://w3id.org/elmo/elmo_3620802"/>
        <obo:IAO_0000115 xml:lang="en">A legal protection process in which the legal protection applies to a specific habitat.</obo:IAO_0000115>
        <dcterms:contributor rdf:resource="https://orcid.org/0000-0002-4366-3088"/>
        <dcterms:contributor rdf:resource="https://orcid.org/0000-0003-4817-0423"/>
        <oboInOwl:created_by rdf:resource="https://orcid.org/0000-0002-1296-2528"/>
        <rdfs:label xml:lang="en">legal habitat protection process</rdfs:label>
    </owl:Class>
    


    <!-- https://w3id.org/elmo/elmo_3620804 -->

    <owl:Class rdf:about="https://w3id.org/elmo/elmo_3620804">
        <rdfs:subClassOf rdf:resource="https://w3id.org/elmo/elmo_3620802"/>
        <obo:IAO_0000115 xml:lang="en">A legal protection process in which the legal protection applies to a specific landscape.</obo:IAO_0000115>
        <dcterms:contributor rdf:resource="https://orcid.org/0000-0002-4366-3088"/>
        <dcterms:contributor rdf:resource="https://orcid.org/0000-0003-4817-0423"/>
        <oboInOwl:created_by rdf:resource="https://orcid.org/0000-0002-1296-2528"/>
        <rdfs:label xml:lang="en">legal landscape protection process</rdfs:label>
    </owl:Class>
    


    <!-- https://w3id.org/elmo/elmo_3620805 -->

    <owl:Class rdf:about="https://w3id.org/elmo/elmo_3620805">
        <rdfs:subClassOf rdf:resource="https://w3id.org/elmo/elmo_3620802"/>
        <obo:IAO_0000115 xml:lang="en">A legal protection process in which the legal protection applies to some taxa.</obo:IAO_0000115>
        <dcterms:contributor rdf:resource="https://orcid.org/0000-0002-4366-3088"/>
        <dcterms:contributor rdf:resource="https://orcid.org/0000-0003-4817-0423"/>
        <oboInOwl:created_by rdf:resource="https://orcid.org/0000-0002-1296-2528"/>
        <rdfs:label xml:lang="en">legal species protection process</rdfs:label>
    </owl:Class>
    


    <!-- https://w3id.org/elmo/elmo_3620806 -->

    <owl:Class rdf:about="https://w3id.org/elmo/elmo_3620806">
        <rdfs:subClassOf rdf:resource="https://w3id.org/elmo/elmo_3620802"/>
        <obo:IAO_0000115 xml:lang="en">A legal protection process in which the legal protection applies to some marine area.</obo:IAO_0000115>
        <dcterms:contributor rdf:resource="https://orcid.org/0000-0002-4366-3088"/>
        <dcterms:contributor rdf:resource="https://orcid.org/0000-0003-4817-0423"/>
        <oboInOwl:created_by rdf:resource="https://orcid.org/0000-0002-1296-2528"/>
        <rdfs:label xml:lang="en">legal marine area protection process</rdfs:label>
    </owl:Class>
    


    <!-- https://w3id.org/elmo/elmo_3620807 -->

    <owl:Class rdf:about="https://w3id.org/elmo/elmo_3620807">
        <rdfs:subClassOf rdf:resource="https://w3id.org/elmo/elmo_3620802"/>
        <obo:IAO_0000115 xml:lang="en">A legal protection process in which the legal protection applies to some privately held land.</obo:IAO_0000115>
        <dcterms:contributor rdf:resource="https://orcid.org/0000-0002-4366-3088"/>
        <dcterms:contributor rdf:resource="https://orcid.org/0000-0003-4817-0423"/>
        <oboInOwl:created_by rdf:resource="https://orcid.org/0000-0002-1296-2528"/>
        <rdfs:label xml:lang="en">private land protection process</rdfs:label>
    </owl:Class>
    


    <!-- https://w3id.org/elmo/elmo_3620808 -->

    <owl:Class rdf:about="https://w3id.org/elmo/elmo_3620808">
        <rdfs:subClassOf rdf:resource="https://w3id.org/elmo/elmo_3620807"/>
        <obo:IAO_0000115 xml:lang="en">A private land protection process in which a landowner agrees to conserve a portion of their land in perpetuity.</obo:IAO_0000115>
        <dcterms:contributor rdf:resource="https://orcid.org/0000-0002-4366-3088"/>
        <dcterms:contributor rdf:resource="https://orcid.org/0000-0003-4817-0423"/>
        <oboInOwl:created_by rdf:resource="https://orcid.org/0000-0002-1296-2528"/>
        <rdfs:label xml:lang="en">conservation easement process</rdfs:label>
    </owl:Class>
    


    <!-- https://w3id.org/elmo/elmo_3620809 -->

    <owl:Class rdf:about="https://w3id.org/elmo/elmo_3620809">
        <rdfs:subClassOf rdf:resource="https://w3id.org/elmo/elmo_3620801"/>
        <obo:IAO_0000115 xml:lang="en">A legislation process in which some legislation applies to some area.</obo:IAO_0000115>
        <dcterms:contributor rdf:resource="https://orcid.org/0000-0002-4366-3088"/>
        <dcterms:contributor rdf:resource="https://orcid.org/0000-0003-4817-0423"/>
        <oboInOwl:created_by rdf:resource="https://orcid.org/0000-0002-1296-2528"/>
        <rdfs:label xml:lang="en">area policy process</rdfs:label>
    </owl:Class>
    


    <!-- https://w3id.org/elmo/elmo_3620810 -->

    <owl:Class rdf:about="https://w3id.org/elmo/elmo_3620810">
        <rdfs:subClassOf rdf:resource="https://w3id.org/elmo/elmo_3620809"/>
        <obo:IAO_0000115 xml:lang="en">An area policy process in which some pro-conservation bylaw is established by a local authority.</obo:IAO_0000115>
        <dcterms:contributor rdf:resource="https://orcid.org/0000-0002-4366-3088"/>
        <dcterms:contributor rdf:resource="https://orcid.org/0000-0003-4817-0423"/>
        <oboInOwl:created_by rdf:resource="https://orcid.org/0000-0002-1296-2528"/>
        <rdfs:label xml:lang="en">local bylaw process</rdfs:label>
    </owl:Class>
    


    <!-- https://w3id.org/elmo/elmo_3620811 -->

    <owl:Class rdf:about="https://w3id.org/elmo/elmo_3620811">
        <rdfs:subClassOf rdf:resource="https://w3id.org/elmo/elmo_3620801"/>
        <obo:IAO_0000115 xml:lang="en">A legislation process in which some group passes pro-conservation legislation at the state or province level.</obo:IAO_0000115>
        <dcterms:contributor rdf:resource="https://orcid.org/0000-0002-4366-3088"/>
        <dcterms:contributor rdf:resource="https://orcid.org/0000-0003-4817-0423"/>
        <oboInOwl:created_by rdf:resource="https://orcid.org/0000-0002-1296-2528"/>
        <rdfs:label xml:lang="en">provincial or state legislation process</rdfs:label>
    </owl:Class>
    


    <!-- https://w3id.org/elmo/elmo_3620812 -->

    <owl:Class rdf:about="https://w3id.org/elmo/elmo_3620812">
        <rdfs:subClassOf rdf:resource="https://w3id.org/elmo/elmo_3620801"/>
        <obo:IAO_0000115 xml:lang="en">A legislation process in which some group passes pro-conservation legislation at the national level.</obo:IAO_0000115>
        <dcterms:contributor rdf:resource="https://orcid.org/0000-0002-4366-3088"/>
        <dcterms:contributor rdf:resource="https://orcid.org/0000-0003-4817-0423"/>
        <oboInOwl:created_by rdf:resource="https://orcid.org/0000-0002-1296-2528"/>
        <rdfs:label xml:lang="en">national legislation process</rdfs:label>
    </owl:Class>
    


    <!-- https://w3id.org/elmo/elmo_3620813 -->

    <owl:Class rdf:about="https://w3id.org/elmo/elmo_3620813">
        <rdfs:subClassOf rdf:resource="https://w3id.org/elmo/elmo_3620800"/>
        <obo:IAO_0000115 xml:lang="en">A ecosystem-oriented social process in which a humans collectively agree to measures that protect, conserve and restore biodiversity.</obo:IAO_0000115>
        <dcterms:contributor rdf:resource="https://orcid.org/0000-0002-4366-3088"/>
        <dcterms:contributor rdf:resource="https://orcid.org/0000-0003-4817-0423"/>
        <oboInOwl:created_by rdf:resource="https://orcid.org/0000-0002-1296-2528"/>
        <rdfs:label xml:lang="en">international agreement process</rdfs:label>
    </owl:Class>
    


    <!-- https://w3id.org/elmo/elmo_3620814 -->

    <owl:Class rdf:about="https://w3id.org/elmo/elmo_3620814">
        <rdfs:subClassOf rdf:resource="https://w3id.org/elmo/elmo_3620800"/>
        <obo:IAO_0000115 xml:lang="en">A ecosystem-oriented social process in which a human actively enforces the pro-conservation legislation or policies governing a specific area.</obo:IAO_0000115>
        <dcterms:contributor rdf:resource="https://orcid.org/0000-0002-4366-3088"/>
        <dcterms:contributor rdf:resource="https://orcid.org/0000-0003-4817-0423"/>
        <oboInOwl:created_by rdf:resource="https://orcid.org/0000-0002-1296-2528"/>
        <rdfs:label xml:lang="en">active enforcement process</rdfs:label>
    </owl:Class>
    


    <!-- https://w3id.org/elmo/elmo_3620815 -->

    <owl:Class rdf:about="https://w3id.org/elmo/elmo_3620815">
        <rdfs:subClassOf rdf:resource="https://w3id.org/elmo/elmo_3620800"/>
        <obo:IAO_0000115 xml:lang="en">A ecosystem-oriented social process in which a human implements measures to reduce conflict between fauna and humans.</obo:IAO_0000115>
        <dcterms:contributor rdf:resource="https://orcid.org/0000-0002-4366-3088"/>
        <dcterms:contributor rdf:resource="https://orcid.org/0000-0003-4817-0423"/>
        <oboInOwl:created_by rdf:resource="https://orcid.org/0000-0002-1296-2528"/>
        <rdfs:label xml:lang="en">human-wildlife conflict reduction process</rdfs:label>
    </owl:Class>
    


    <!-- https://w3id.org/elmo/elmo_3620816 -->

    <owl:Class rdf:about="https://w3id.org/elmo/elmo_3620816">
        <rdfs:subClassOf rdf:resource="https://w3id.org/elmo/elmo_3620800"/>
        <obo:IAO_0000115 xml:lang="en">A ecosystem-oriented social process in which a human assists a species in crossing a road.</obo:IAO_0000115>
        <dcterms:contributor rdf:resource="https://orcid.org/0000-0002-4366-3088"/>
        <dcterms:contributor rdf:resource="https://orcid.org/0000-0003-4817-0423"/>
        <oboInOwl:created_by rdf:resource="https://orcid.org/0000-0002-1296-2528"/>
        <rdfs:label xml:lang="en">human-assisted road crossing process</rdfs:label>
    </owl:Class>
    


    <!-- https://w3id.org/elmo/elmo_3620817 -->

    <owl:Class rdf:about="https://w3id.org/elmo/elmo_3620817">
        <rdfs:subClassOf rdf:resource="https://w3id.org/elmo/elmo_3620800"/>
        <obo:IAO_0000115 xml:lang="en">A ecosystem-oriented social process in which a human undertakes a process in order to make others more aware of threats to biodiversity.</obo:IAO_0000115>
        <dcterms:contributor rdf:resource="https://orcid.org/0000-0002-4366-3088"/>
        <dcterms:contributor rdf:resource="https://orcid.org/0000-0003-4817-0423"/>
        <oboInOwl:created_by rdf:resource="https://orcid.org/0000-0002-1296-2528"/>
        <rdfs:label xml:lang="en">awareness-raising process</rdfs:label>
    </owl:Class>
    


    <!-- https://w3id.org/elmo/elmo_3620818 -->

    <owl:Class rdf:about="https://w3id.org/elmo/elmo_3620818">
        <rdfs:subClassOf rdf:resource="https://w3id.org/elmo/elmo_3620817"/>
        <obo:IAO_0000115 xml:lang="en">An awareness-raising process in which a human uses social media to spread messages about threats to biodiversity.</obo:IAO_0000115>
        <dcterms:contributor rdf:resource="https://orcid.org/0000-0002-4366-3088"/>
        <dcterms:contributor rdf:resource="https://orcid.org/0000-0003-4817-0423"/>
        <oboInOwl:created_by rdf:resource="https://orcid.org/0000-0002-1296-2528"/>
        <rdfs:label xml:lang="en">social media campaign process</rdfs:label>
    </owl:Class>
    


    <!-- https://w3id.org/elmo/elmo_3620819 -->

    <owl:Class rdf:about="https://w3id.org/elmo/elmo_3620819">
        <rdfs:subClassOf rdf:resource="https://w3id.org/elmo/elmo_3620817"/>
        <obo:IAO_0000115 xml:lang="en">An awareness-raising process in which a human hosts an event for the community in a given area.</obo:IAO_0000115>
        <dcterms:contributor rdf:resource="https://orcid.org/0000-0002-4366-3088"/>
        <dcterms:contributor rdf:resource="https://orcid.org/0000-0003-4817-0423"/>
        <oboInOwl:created_by rdf:resource="https://orcid.org/0000-0002-1296-2528"/>
        <rdfs:label xml:lang="en">community event creation process</rdfs:label>
    </owl:Class>
    


    <!-- https://w3id.org/elmo/elmo_3620820 -->

    <owl:Class rdf:about="https://w3id.org/elmo/elmo_3620820">
        <rdfs:subClassOf rdf:resource="https://w3id.org/elmo/elmo_3620817"/>
        <obo:IAO_0000115 xml:lang="en">An awareness-raising process in which a human endeavours to improve the knowledge of others vis-a-vis restoration or conservation of biodiversity.</obo:IAO_0000115>
        <dcterms:contributor rdf:resource="https://orcid.org/0000-0002-4366-3088"/>
        <dcterms:contributor rdf:resource="https://orcid.org/0000-0003-4817-0423"/>
        <oboInOwl:created_by rdf:resource="https://orcid.org/0000-0002-1296-2528"/>
        <rdfs:label xml:lang="en">education process</rdfs:label>
    </owl:Class>
    


    <!-- https://w3id.org/elmo/elmo_3620821 -->

    <owl:Class rdf:about="https://w3id.org/elmo/elmo_3620821">
        <rdfs:subClassOf rdf:resource="https://w3id.org/elmo/elmo_3620817"/>
        <obo:IAO_0000115 xml:lang="en">An awareness-raising process in which a humans gather measurements of some ecosystem elements.</obo:IAO_0000115>
        <dcterms:contributor rdf:resource="https://orcid.org/0000-0002-4366-3088"/>
        <dcterms:contributor rdf:resource="https://orcid.org/0000-0003-4817-0423"/>
        <oboInOwl:created_by rdf:resource="https://orcid.org/0000-0002-1296-2528"/>
        <rdfs:label xml:lang="en">citizen science process</rdfs:label>
    </owl:Class>
    


    <!-- https://w3id.org/elmo/elmo_3620822 -->

    <owl:Class rdf:about="https://w3id.org/elmo/elmo_3620822">
        <rdfs:subClassOf rdf:resource="https://w3id.org/elmo/elmo_3620817"/>
        <obo:IAO_0000115 xml:lang="en">An awareness-raising process in which a humans are gathered in a given area and engaged in the restoration and conservation of biodiversity.</obo:IAO_0000115>
        <dcterms:contributor rdf:resource="https://orcid.org/0000-0002-4366-3088"/>
        <dcterms:contributor rdf:resource="https://orcid.org/0000-0003-4817-0423"/>
        <oboInOwl:created_by rdf:resource="https://orcid.org/0000-0002-1296-2528"/>
        <rdfs:label xml:lang="en">community engagement process</rdfs:label>
    </owl:Class>
    


    <!-- https://w3id.org/elmo/elmo_3620823 -->

    <owl:Class rdf:about="https://w3id.org/elmo/elmo_3620823">
        <rdfs:subClassOf rdf:resource="https://w3id.org/elmo/elmo_3620800"/>
        <obo:IAO_0000115 xml:lang="en">A ecosystem-oriented social process in which a human endeavours to alter the behaviour of others vis-a-vis the degradation of ecosystems.</obo:IAO_0000115>
        <dcterms:contributor rdf:resource="https://orcid.org/0000-0002-4366-3088"/>
        <dcterms:contributor rdf:resource="https://orcid.org/0000-0003-4817-0423"/>
        <oboInOwl:created_by rdf:resource="https://orcid.org/0000-0002-1296-2528"/>
        <rdfs:label xml:lang="en">pro-environmental behaviour change process</rdfs:label>
    </owl:Class>
    <owl:Axiom>
        <owl:annotatedSource rdf:resource="https://w3id.org/elmo/elmo_3620823"/>
        <owl:annotatedProperty rdf:resource="http://purl.obolibrary.org/obo/IAO_0000115"/>
        <owl:annotatedTarget xml:lang="en">A ecosystem-oriented social process in which a human endeavours to alter the behaviour of others vis-a-vis the degradation of ecosystems.</owl:annotatedTarget>
        <oboInOwl:hasDbXref rdf:resource="doi:10.1038/s41562-022-01473-w"/>
    </owl:Axiom>
    


    <!-- https://w3id.org/elmo/elmo_3620824 -->

    <owl:Class rdf:about="https://w3id.org/elmo/elmo_3620824">
        <rdfs:subClassOf rdf:resource="https://w3id.org/elmo/elmo_3620823"/>
        <obo:IAO_0000115 xml:lang="en">A pro-environmental behaviour change process in which signage is installed to encourage or deter activities in an area.</obo:IAO_0000115>
        <dcterms:contributor rdf:resource="https://orcid.org/0000-0002-4366-3088"/>
        <dcterms:contributor rdf:resource="https://orcid.org/0000-0003-4817-0423"/>
        <oboInOwl:created_by rdf:resource="https://orcid.org/0000-0002-1296-2528"/>
        <rdfs:label xml:lang="en">signage installation process</rdfs:label>
    </owl:Class>
    


    <!-- https://w3id.org/elmo/elmo_3620825 -->

    <owl:Class rdf:about="https://w3id.org/elmo/elmo_3620825">
        <rdfs:subClassOf rdf:resource="https://w3id.org/elmo/elmo_3620823"/>
        <obo:IAO_0000115 xml:lang="en">A pro-environmental behaviour change process in which a human reaches out to people directly to encourage or deter activities in an area.</obo:IAO_0000115>
        <dcterms:contributor rdf:resource="https://orcid.org/0000-0002-4366-3088"/>
        <dcterms:contributor rdf:resource="https://orcid.org/0000-0003-4817-0423"/>
        <oboInOwl:created_by rdf:resource="https://orcid.org/0000-0002-1296-2528"/>
        <rdfs:label xml:lang="en">individual outreach process</rdfs:label>
    </owl:Class>
    


    <!-- https://w3id.org/elmo/elmo_3620826 -->

    <owl:Class rdf:about="https://w3id.org/elmo/elmo_3620826">
        <rdfs:subClassOf rdf:resource="https://w3id.org/elmo/elmo_3620823"/>
        <obo:IAO_0000115 xml:lang="en">A pro-environmental behaviour change process in which a human reaches out to a landowner to encourage or deter activities in an area.</obo:IAO_0000115>
        <dcterms:contributor rdf:resource="https://orcid.org/0000-0002-4366-3088"/>
        <dcterms:contributor rdf:resource="https://orcid.org/0000-0003-4817-0423"/>
        <oboInOwl:created_by rdf:resource="https://orcid.org/0000-0002-1296-2528"/>
        <rdfs:label xml:lang="en">landowner outreach process</rdfs:label>
    </owl:Class>
    


    <!-- https://w3id.org/elmo/elmo_3620827 -->

    <owl:Class rdf:about="https://w3id.org/elmo/elmo_3620827">
        <rdfs:subClassOf rdf:resource="https://w3id.org/elmo/elmo_3620823"/>
        <obo:IAO_0000115 xml:lang="en">A pro-environmental behaviour change process in which a human marks environmentally sensitive features to deter degradation or interference.</obo:IAO_0000115>
        <dcterms:contributor rdf:resource="https://orcid.org/0000-0002-4366-3088"/>
        <dcterms:contributor rdf:resource="https://orcid.org/0000-0003-4817-0423"/>
        <oboInOwl:created_by rdf:resource="https://orcid.org/0000-0002-1296-2528"/>
        <rdfs:label xml:lang="en">sensitive features marking process</rdfs:label>
    </owl:Class>
    


    <!-- https://w3id.org/elmo/elmo_3620828 -->

    <owl:Class rdf:about="https://w3id.org/elmo/elmo_3620828">
        <rdfs:subClassOf rdf:resource="https://w3id.org/elmo/elmo_3620800"/>
        <obo:IAO_0000115 xml:lang="en">A ecosystem-oriented social process in which a human raises funds to support the restoration and conservation of a specific area.</obo:IAO_0000115>
        <dcterms:contributor rdf:resource="https://orcid.org/0000-0002-4366-3088"/>
        <dcterms:contributor rdf:resource="https://orcid.org/0000-0003-4817-0423"/>
        <oboInOwl:created_by rdf:resource="https://orcid.org/0000-0002-1296-2528"/>
        <rdfs:label xml:lang="en">fundraising process</rdfs:label>
    </owl:Class>
    


    <!-- https://w3id.org/elmo/elmo_3620829 -->

    <owl:Class rdf:about="https://w3id.org/elmo/elmo_3620829">
        <rdfs:subClassOf rdf:resource="https://w3id.org/elmo/elmo_3620800"/>
        <obo:IAO_0000115 xml:lang="en">A ecosystem-oriented social process in which financial incentives are offered to a humans in order to take pro-environmental measures.</obo:IAO_0000115>
        <dcterms:contributor rdf:resource="https://orcid.org/0000-0002-4366-3088"/>
        <dcterms:contributor rdf:resource="https://orcid.org/0000-0003-4817-0423"/>
        <oboInOwl:created_by rdf:resource="https://orcid.org/0000-0002-1296-2528"/>
        <rdfs:label xml:lang="en">financial incentive process</rdfs:label>
    </owl:Class>
    


    <!-- https://w3id.org/elmo/elmo_3620830 -->

    <owl:Class rdf:about="https://w3id.org/elmo/elmo_3620830">
        <rdfs:subClassOf rdf:resource="https://w3id.org/elmo/elmo_3620800"/>
        <obo:IAO_0000115 xml:lang="en">A ecosystem-oriented social process in which some authority regulates the usage of environments.</obo:IAO_0000115>
        <dcterms:contributor rdf:resource="https://orcid.org/0000-0002-4366-3088"/>
        <dcterms:contributor rdf:resource="https://orcid.org/0000-0003-4817-0423"/>
        <oboInOwl:created_by rdf:resource="https://orcid.org/0000-0002-1296-2528"/>
        <rdfs:label xml:lang="en">environmental usage regulation process</rdfs:label>
    </owl:Class>
    


    <!-- https://w3id.org/elmo/elmo_3620831 -->

    <owl:Class rdf:about="https://w3id.org/elmo/elmo_3620831">
        <rdfs:subClassOf rdf:resource="https://w3id.org/elmo/elmo_3620830"/>
        <obo:IAO_0000115 xml:lang="en">An environmental usage regulation process in which some authority regulates grazing in a given area.</obo:IAO_0000115>
        <dcterms:contributor rdf:resource="https://orcid.org/0000-0002-4366-3088"/>
        <dcterms:contributor rdf:resource="https://orcid.org/0000-0003-4817-0423"/>
        <oboInOwl:created_by rdf:resource="https://orcid.org/0000-0002-1296-2528"/>
        <rdfs:label xml:lang="en">regulate grazing</rdfs:label>
    </owl:Class>
    


    <!-- https://w3id.org/elmo/elmo_3620832 -->

    <owl:Class rdf:about="https://w3id.org/elmo/elmo_3620832">
        <rdfs:subClassOf rdf:resource="https://w3id.org/elmo/elmo_3620831"/>
        <obo:IAO_0000115 xml:lang="en">An environmental usage regulation process in which some authority prohibits grazing in a given area.</obo:IAO_0000115>
        <dcterms:contributor rdf:resource="https://orcid.org/0000-0002-4366-3088"/>
        <dcterms:contributor rdf:resource="https://orcid.org/0000-0003-4817-0423"/>
        <oboInOwl:created_by rdf:resource="https://orcid.org/0000-0002-1296-2528"/>
        <rdfs:label xml:lang="en">prohibit grazing</rdfs:label>
    </owl:Class>
    


    <!-- https://w3id.org/elmo/elmo_3620833 -->

    <owl:Class rdf:about="https://w3id.org/elmo/elmo_3620833">
        <rdfs:subClassOf rdf:resource="https://w3id.org/elmo/elmo_3620830"/>
        <obo:IAO_0000115 xml:lang="en">An environmental usage regulation process in which some authority regulates fishing in a given area.</obo:IAO_0000115>
        <dcterms:contributor rdf:resource="https://orcid.org/0000-0002-4366-3088"/>
        <dcterms:contributor rdf:resource="https://orcid.org/0000-0003-4817-0423"/>
        <oboInOwl:created_by rdf:resource="https://orcid.org/0000-0002-1296-2528"/>
        <rdfs:label xml:lang="en">regulate fishing</rdfs:label>
    </owl:Class>
    


    <!-- https://w3id.org/elmo/elmo_3620834 -->

    <owl:Class rdf:about="https://w3id.org/elmo/elmo_3620834">
        <rdfs:subClassOf rdf:resource="https://w3id.org/elmo/elmo_3620833"/>
        <obo:IAO_0000115 xml:lang="en">An environmental usage regulation process in which some authority prohibits fishing in a given area.</obo:IAO_0000115>
        <dcterms:contributor rdf:resource="https://orcid.org/0000-0002-4366-3088"/>
        <dcterms:contributor rdf:resource="https://orcid.org/0000-0003-4817-0423"/>
        <oboInOwl:created_by rdf:resource="https://orcid.org/0000-0002-1296-2528"/>
        <rdfs:label xml:lang="en">prohibit fishing</rdfs:label>
    </owl:Class>
    


    <!-- https://w3id.org/elmo/elmo_3620835 -->

    <owl:Class rdf:about="https://w3id.org/elmo/elmo_3620835">
        <rdfs:subClassOf rdf:resource="https://w3id.org/elmo/elmo_3620830"/>
        <obo:IAO_0000115 xml:lang="en">An environmental usage regulation process in which some authority regulates chemical usage in a given area.</obo:IAO_0000115>
        <dcterms:contributor rdf:resource="https://orcid.org/0000-0002-4366-3088"/>
        <dcterms:contributor rdf:resource="https://orcid.org/0000-0003-4817-0423"/>
        <oboInOwl:created_by rdf:resource="https://orcid.org/0000-0002-1296-2528"/>
        <rdfs:label xml:lang="en">regulate chemical usage</rdfs:label>
    </owl:Class>
    


    <!-- https://w3id.org/elmo/elmo_3620836 -->

    <owl:Class rdf:about="https://w3id.org/elmo/elmo_3620836">
        <rdfs:subClassOf rdf:resource="https://w3id.org/elmo/elmo_3620835"/>
        <obo:IAO_0000115 xml:lang="en">An environmental usage regulation process in which some authority prohibits chemical usage in a given area.</obo:IAO_0000115>
        <dcterms:contributor rdf:resource="https://orcid.org/0000-0002-4366-3088"/>
        <dcterms:contributor rdf:resource="https://orcid.org/0000-0003-4817-0423"/>
        <oboInOwl:created_by rdf:resource="https://orcid.org/0000-0002-1296-2528"/>
        <rdfs:label xml:lang="en">prohibit chemical usage</rdfs:label>
    </owl:Class>
    


    <!-- https://w3id.org/elmo/elmo_3620837 -->

    <owl:Class rdf:about="https://w3id.org/elmo/elmo_3620837">
        <rdfs:subClassOf rdf:resource="https://w3id.org/elmo/elmo_3620830"/>
        <obo:IAO_0000115 xml:lang="en">An environmental usage regulation process in which some authority regulates hunting in a given area.</obo:IAO_0000115>
        <dcterms:contributor rdf:resource="https://orcid.org/0000-0002-4366-3088"/>
        <dcterms:contributor rdf:resource="https://orcid.org/0000-0003-4817-0423"/>
        <oboInOwl:created_by rdf:resource="https://orcid.org/0000-0002-1296-2528"/>
        <rdfs:label xml:lang="en">regulate hunting</rdfs:label>
    </owl:Class>
    


    <!-- https://w3id.org/elmo/elmo_3620838 -->

    <owl:Class rdf:about="https://w3id.org/elmo/elmo_3620838">
        <rdfs:subClassOf rdf:resource="https://w3id.org/elmo/elmo_3620837"/>
        <obo:IAO_0000115 xml:lang="en">An environmental usage regulation process in which some authority prohibits hunting in a given area.</obo:IAO_0000115>
        <dcterms:contributor rdf:resource="https://orcid.org/0000-0002-4366-3088"/>
        <dcterms:contributor rdf:resource="https://orcid.org/0000-0003-4817-0423"/>
        <oboInOwl:created_by rdf:resource="https://orcid.org/0000-0002-1296-2528"/>
        <rdfs:label xml:lang="en">prohibit hunting</rdfs:label>
    </owl:Class>
    


    <!-- https://w3id.org/elmo/elmo_3620839 -->

    <owl:Class rdf:about="https://w3id.org/elmo/elmo_3620839">
        <rdfs:subClassOf rdf:resource="https://w3id.org/elmo/elmo_3620830"/>
        <obo:IAO_0000115 xml:lang="en">An environmental usage regulation process in which some authority regulates recreational activities in a given area.</obo:IAO_0000115>
        <dcterms:contributor rdf:resource="https://orcid.org/0000-0002-4366-3088"/>
        <dcterms:contributor rdf:resource="https://orcid.org/0000-0003-4817-0423"/>
        <oboInOwl:created_by rdf:resource="https://orcid.org/0000-0002-1296-2528"/>
        <rdfs:label xml:lang="en">regulate recreational activities</rdfs:label>
    </owl:Class>
    


    <!-- https://w3id.org/elmo/elmo_3620840 -->

    <owl:Class rdf:about="https://w3id.org/elmo/elmo_3620840">
        <rdfs:subClassOf rdf:resource="https://w3id.org/elmo/elmo_3620839"/>
        <obo:IAO_0000115 xml:lang="en">An environmental usage regulation process in which some authority prohibits recreational activities in a given area.</obo:IAO_0000115>
        <dcterms:contributor rdf:resource="https://orcid.org/0000-0002-4366-3088"/>
        <dcterms:contributor rdf:resource="https://orcid.org/0000-0003-4817-0423"/>
        <oboInOwl:created_by rdf:resource="https://orcid.org/0000-0002-1296-2528"/>
        <rdfs:label xml:lang="en">prohibit recreational activities</rdfs:label>
    </owl:Class>
    


    <!-- https://w3id.org/elmo/elmo_3620841 -->

    <owl:Class rdf:about="https://w3id.org/elmo/elmo_3620841">
        <rdfs:subClassOf rdf:resource="https://w3id.org/elmo/elmo_3620830"/>
        <obo:IAO_0000115 xml:lang="en">An environmental usage regulation process in which some authority limits public access to a given area.</obo:IAO_0000115>
        <dcterms:contributor rdf:resource="https://orcid.org/0000-0002-4366-3088"/>
        <dcterms:contributor rdf:resource="https://orcid.org/0000-0003-4817-0423"/>
        <oboInOwl:created_by rdf:resource="https://orcid.org/0000-0002-1296-2528"/>
        <rdfs:label xml:lang="en">limit public access</rdfs:label>
    </owl:Class>
    


    <!-- https://w3id.org/elmo/elmo_3620842 -->

    <owl:Class rdf:about="https://w3id.org/elmo/elmo_3620842">
        <rdfs:subClassOf rdf:resource="https://w3id.org/elmo/elmo_3620841"/>
        <obo:IAO_0000115 xml:lang="en">An environmental usage regulation process in which some authority prohibits public access to a given area.</obo:IAO_0000115>
        <dcterms:contributor rdf:resource="https://orcid.org/0000-0002-4366-3088"/>
        <dcterms:contributor rdf:resource="https://orcid.org/0000-0003-4817-0423"/>
        <oboInOwl:created_by rdf:resource="https://orcid.org/0000-0002-1296-2528"/>
        <rdfs:label xml:lang="en">prohibit public access</rdfs:label>
    </owl:Class>
    


    <!-- https://w3id.org/elmo/elmo_3620843 -->

    <owl:Class rdf:about="https://w3id.org/elmo/elmo_3620843">
        <rdfs:subClassOf rdf:resource="https://w3id.org/elmo/elmo_3620830"/>
        <obo:IAO_0000115 xml:lang="en">An environmental usage regulation process in which some authority regulates dredging in a given area.</obo:IAO_0000115>
        <dcterms:contributor rdf:resource="https://orcid.org/0000-0002-4366-3088"/>
        <dcterms:contributor rdf:resource="https://orcid.org/0000-0003-4817-0423"/>
        <oboInOwl:created_by rdf:resource="https://orcid.org/0000-0002-1296-2528"/>
        <rdfs:label xml:lang="en">regulate dredging</rdfs:label>
    </owl:Class>
    


    <!-- https://w3id.org/elmo/elmo_3620844 -->

    <owl:Class rdf:about="https://w3id.org/elmo/elmo_3620844">
        <rdfs:subClassOf rdf:resource="https://w3id.org/elmo/elmo_3620843"/>
        <obo:IAO_0000115 xml:lang="en">An environmental usage regulation process in which some authority prohibits dredging in a given area.</obo:IAO_0000115>
        <dcterms:contributor rdf:resource="https://orcid.org/0000-0002-4366-3088"/>
        <dcterms:contributor rdf:resource="https://orcid.org/0000-0003-4817-0423"/>
        <oboInOwl:created_by rdf:resource="https://orcid.org/0000-0002-1296-2528"/>
        <rdfs:label xml:lang="en">prohibit dredging</rdfs:label>
    </owl:Class>
    


    <!-- https://w3id.org/elmo/elmo_3620845 -->

    <owl:Class rdf:about="https://w3id.org/elmo/elmo_3620845">
        <rdfs:subClassOf rdf:resource="https://w3id.org/elmo/elmo_3620830"/>
        <obo:IAO_0000115 xml:lang="en">An environmental usage regulation process in which some authority regulates aquaculture in a given area.</obo:IAO_0000115>
        <dcterms:contributor rdf:resource="https://orcid.org/0000-0002-4366-3088"/>
        <dcterms:contributor rdf:resource="https://orcid.org/0000-0003-4817-0423"/>
        <oboInOwl:created_by rdf:resource="https://orcid.org/0000-0002-1296-2528"/>
        <rdfs:label xml:lang="en">regulate aquaculture</rdfs:label>
    </owl:Class>
    


    <!-- https://w3id.org/elmo/elmo_3620846 -->

    <owl:Class rdf:about="https://w3id.org/elmo/elmo_3620846">
        <rdfs:subClassOf rdf:resource="https://w3id.org/elmo/elmo_3620845"/>
        <obo:IAO_0000115 xml:lang="en">An environmental usage regulation process in which some authority prohibits aquaculture in a given area.</obo:IAO_0000115>
        <dcterms:contributor rdf:resource="https://orcid.org/0000-0002-4366-3088"/>
        <dcterms:contributor rdf:resource="https://orcid.org/0000-0003-4817-0423"/>
        <oboInOwl:created_by rdf:resource="https://orcid.org/0000-0002-1296-2528"/>
        <rdfs:label xml:lang="en">prohibit aquaculture</rdfs:label>
    </owl:Class>
    


    <!-- https://w3id.org/elmo/elmo_3620847 -->

    <owl:Class rdf:about="https://w3id.org/elmo/elmo_3620847">
        <rdfs:subClassOf rdf:resource="https://w3id.org/elmo/elmo_3620800"/>
        <obo:IAO_0000115 xml:lang="en">A ecosystem-oriented social process in which a humans undertake shared practices passed down through generations to manage the ecosystem in which they live.</obo:IAO_0000115>
        <dcterms:contributor rdf:resource="https://orcid.org/0000-0002-4366-3088"/>
        <dcterms:contributor rdf:resource="https://orcid.org/0000-0003-4817-0423"/>
        <oboInOwl:created_by rdf:resource="https://orcid.org/0000-0002-1296-2528"/>
        <rdfs:label xml:lang="en">cultural ecosystem management process</rdfs:label>
    </owl:Class>
    


    <!-- https://w3id.org/elmo/elmo_3620848 -->

    <owl:Class rdf:about="https://w3id.org/elmo/elmo_3620848">
        <rdfs:subClassOf rdf:resource="https://w3id.org/elmo/elmo_3620800"/>
        <obo:IAO_0000115 xml:lang="en">A ecosystem-oriented social process in which a humans harvest resources from the environment for shared practices that are passed down through generations.</obo:IAO_0000115>
        <dcterms:contributor rdf:resource="https://orcid.org/0000-0002-4366-3088"/>
        <dcterms:contributor rdf:resource="https://orcid.org/0000-0003-4817-0423"/>
        <oboInOwl:created_by rdf:resource="https://orcid.org/0000-0002-1296-2528"/>
        <rdfs:label xml:lang="en">cultural ecosystem usage process</rdfs:label>
    </owl:Class>
    


    <!-- https://w3id.org/elmo/elmo_3620849 -->

    <owl:Class rdf:about="https://w3id.org/elmo/elmo_3620849">
        <rdfs:subClassOf rdf:resource="https://w3id.org/elmo/elmo_3620800"/>
        <obo:IAO_0000115 xml:lang="en">A ecosystem-oriented social process in which a human alters the way in which some planned process is undertaken.</obo:IAO_0000115>
        <dcterms:contributor rdf:resource="https://orcid.org/0000-0002-4366-3088"/>
        <dcterms:contributor rdf:resource="https://orcid.org/0000-0003-4817-0423"/>
        <oboInOwl:created_by rdf:resource="https://orcid.org/0000-0002-1296-2528"/>
        <rdfs:label xml:lang="en">plan specification change process</rdfs:label>
    </owl:Class>
    


    <!-- https://w3id.org/elmo/elmo_3620850 -->

    <owl:Class rdf:about="https://w3id.org/elmo/elmo_3620850">
        <rdfs:subClassOf rdf:resource="https://w3id.org/elmo/elmo_3620851"/>
        <obo:IAO_0000115 xml:lang="en">A change to the mowing regime in which a human alters the timing of regular mowing with the goal of protecting specific taxa.</obo:IAO_0000115>
        <dcterms:contributor rdf:resource="https://orcid.org/0000-0002-4366-3088"/>
        <dcterms:contributor rdf:resource="https://orcid.org/0000-0003-4817-0423"/>
        <oboInOwl:created_by rdf:resource="https://orcid.org/0000-0002-1296-2528"/>
        <rdfs:label xml:lang="en">alter mowing timing</rdfs:label>
    </owl:Class>
    


    <!-- https://w3id.org/elmo/elmo_3620851 -->

    <owl:Class rdf:about="https://w3id.org/elmo/elmo_3620851">
        <rdfs:subClassOf rdf:resource="https://w3id.org/elmo/elmo_3620849"/>
        <obo:IAO_0000115 xml:lang="en">A plan specification change process in which a human alters the mowing regime (i.e. frequency, height, timing)</obo:IAO_0000115>
        <dcterms:contributor rdf:resource="https://orcid.org/0000-0002-4366-3088"/>
        <dcterms:contributor rdf:resource="https://orcid.org/0000-0003-4817-0423"/>
        <oboInOwl:created_by rdf:resource="https://orcid.org/0000-0002-1296-2528"/>
        <rdfs:label xml:lang="en">alter mowing regime</rdfs:label>
    </owl:Class>
    


    <!-- https://w3id.org/elmo/elmo_3620852 -->

    <owl:Class rdf:about="https://w3id.org/elmo/elmo_3620852">
        <rdfs:subClassOf rdf:resource="https://w3id.org/elmo/elmo_3620851"/>
        <obo:IAO_0000115 xml:lang="en">A change to the mowing regime in which a human alters the height of a mower with the goal of protecting specific taxa.</obo:IAO_0000115>
        <dcterms:contributor rdf:resource="https://orcid.org/0000-0002-4366-3088"/>
        <dcterms:contributor rdf:resource="https://orcid.org/0000-0003-4817-0423"/>
        <oboInOwl:created_by rdf:resource="https://orcid.org/0000-0002-1296-2528"/>
        <rdfs:label xml:lang="en">alter mowing height</rdfs:label>
    </owl:Class>
    


    <!-- https://w3id.org/elmo/elmo_3620853 -->

    <owl:Class rdf:about="https://w3id.org/elmo/elmo_3620853">
        <rdfs:subClassOf rdf:resource="https://w3id.org/elmo/elmo_3620849"/>
        <obo:IAO_0000115 xml:lang="en">A change to the tilling regime in which a human alters the frequency, timing or severity of a regular tilling process.</obo:IAO_0000115>
        <dcterms:contributor rdf:resource="https://orcid.org/0000-0002-4366-3088"/>
        <dcterms:contributor rdf:resource="https://orcid.org/0000-0003-4817-0423"/>
        <oboInOwl:created_by rdf:resource="https://orcid.org/0000-0002-1296-2528"/>
        <rdfs:label xml:lang="en">alter tilling regime</rdfs:label>
    </owl:Class>
    


    <!-- https://w3id.org/elmo/elmo_3620854 -->

    <owl:Class rdf:about="https://w3id.org/elmo/elmo_3620854">
        <rdfs:subClassOf rdf:resource="https://w3id.org/elmo/elmo_3620849"/>
        <obo:IAO_0000115 xml:lang="en">A change to the chemical regime in which a human alters the frequency, timing or severity of a regular chemical application process.</obo:IAO_0000115>
        <dcterms:contributor rdf:resource="https://orcid.org/0000-0002-4366-3088"/>
        <dcterms:contributor rdf:resource="https://orcid.org/0000-0003-4817-0423"/>
        <oboInOwl:created_by rdf:resource="https://orcid.org/0000-0002-1296-2528"/>
        <rdfs:label xml:lang="en">alter chemical regime</rdfs:label>
    </owl:Class>
    


    <!-- https://w3id.org/elmo/elmo_3620855 -->

    <owl:Class rdf:about="https://w3id.org/elmo/elmo_3620855">
        <rdfs:subClassOf rdf:resource="https://w3id.org/elmo/elmo_3620854"/>
        <obo:IAO_0000115 xml:lang="en">A change to the insecticide regime in which a human alters the frequency, timing or severity of a regular insecticide application process.</obo:IAO_0000115>
        <dcterms:contributor rdf:resource="https://orcid.org/0000-0002-4366-3088"/>
        <dcterms:contributor rdf:resource="https://orcid.org/0000-0003-4817-0423"/>
        <oboInOwl:created_by rdf:resource="https://orcid.org/0000-0002-1296-2528"/>
        <rdfs:label xml:lang="en">alter insecticide regime</rdfs:label>
    </owl:Class>
    


    <!-- https://w3id.org/elmo/elmo_3620856 -->

    <owl:Class rdf:about="https://w3id.org/elmo/elmo_3620856">
        <rdfs:subClassOf rdf:resource="https://w3id.org/elmo/elmo_3620849"/>
        <obo:IAO_0000115 xml:lang="en">A change to the fertilizer regime in which a human alters the frequency, timing or severity of a regular fertilizer application process.</obo:IAO_0000115>
        <dcterms:contributor rdf:resource="https://orcid.org/0000-0002-4366-3088"/>
        <dcterms:contributor rdf:resource="https://orcid.org/0000-0003-4817-0423"/>
        <oboInOwl:created_by rdf:resource="https://orcid.org/0000-0002-1296-2528"/>
        <rdfs:label xml:lang="en">alter fertilizer regime</rdfs:label>
    </owl:Class>
    


    <!-- https://w3id.org/elmo/elmo_3620857 -->

    <owl:Class rdf:about="https://w3id.org/elmo/elmo_3620857">
        <rdfs:subClassOf rdf:resource="https://w3id.org/elmo/elmo_3620849"/>
        <obo:IAO_0000115 xml:lang="en">A change to the lighting regime in which a human alters the frequency, timing or intensity of lighting.</obo:IAO_0000115>
        <dcterms:contributor rdf:resource="https://orcid.org/0000-0002-4366-3088"/>
        <dcterms:contributor rdf:resource="https://orcid.org/0000-0003-4817-0423"/>
        <oboInOwl:created_by rdf:resource="https://orcid.org/0000-0002-1296-2528"/>
        <rdfs:label xml:lang="en">alter lighting regime</rdfs:label>
    </owl:Class>
    


    <!-- https://w3id.org/elmo/elmo_3620858 -->

    <owl:Class rdf:about="https://w3id.org/elmo/elmo_3620858">
        <rdfs:subClassOf rdf:resource="https://w3id.org/elmo/elmo_3620849"/>
        <obo:IAO_0000115 xml:lang="en">A change to the grazing regime in which a human alters the frequency, timing or intensity of grazing.</obo:IAO_0000115>
        <dcterms:contributor rdf:resource="https://orcid.org/0000-0002-4366-3088"/>
        <dcterms:contributor rdf:resource="https://orcid.org/0000-0003-4817-0423"/>
        <oboInOwl:created_by rdf:resource="https://orcid.org/0000-0002-1296-2528"/>
        <rdfs:label xml:lang="en">alter grazing regime</rdfs:label>
    </owl:Class>
    


    <!-- https://w3id.org/elmo/elmo_3620859 -->

    <owl:Class rdf:about="https://w3id.org/elmo/elmo_3620859">
        <rdfs:subClassOf rdf:resource="https://w3id.org/elmo/elmo_3620849"/>
        <obo:IAO_0000115 xml:lang="en">A change to the dam regime in which a human alters the frequency, timing or intensity of water released by a dam.</obo:IAO_0000115>
        <dcterms:contributor rdf:resource="https://orcid.org/0000-0002-4366-3088"/>
        <dcterms:contributor rdf:resource="https://orcid.org/0000-0003-4817-0423"/>
        <oboInOwl:created_by rdf:resource="https://orcid.org/0000-0002-1296-2528"/>
        <rdfs:label xml:lang="en">alter dam regime</rdfs:label>
    </owl:Class>
    


    <!-- https://w3id.org/elmo/elmo_3620860 -->

    <owl:Class rdf:about="https://w3id.org/elmo/elmo_3620860">
        <rdfs:subClassOf rdf:resource="https://w3id.org/elmo/elmo_3620854"/>
        <obo:IAO_0000115 xml:lang="en">A change to the herbicide regime in which a human alters the frequency, timing or severity of a regular herbicide application process.</obo:IAO_0000115>
        <dcterms:contributor rdf:resource="https://orcid.org/0000-0002-4366-3088"/>
        <dcterms:contributor rdf:resource="https://orcid.org/0000-0003-4817-0423"/>
        <oboInOwl:created_by rdf:resource="https://orcid.org/0000-0002-1296-2528"/>
        <rdfs:label xml:lang="en">alter herbicide regime</rdfs:label>
    </owl:Class>
    


    <!-- https://w3id.org/elmo/elmo_3620861 -->

    <owl:Class rdf:about="https://w3id.org/elmo/elmo_3620861">
        <rdfs:subClassOf rdf:resource="https://w3id.org/elmo/elmo_3620860"/>
        <obo:IAO_0000115 xml:lang="en">A change to the herbicide regime in which a human ceases some herbicide application process.</obo:IAO_0000115>
        <dcterms:contributor rdf:resource="https://orcid.org/0000-0002-4366-3088"/>
        <dcterms:contributor rdf:resource="https://orcid.org/0000-0003-4817-0423"/>
        <oboInOwl:created_by rdf:resource="https://orcid.org/0000-0002-1296-2528"/>
        <rdfs:label xml:lang="en">cease herbicide usage</rdfs:label>
    </owl:Class>
    


    <!-- https://w3id.org/elmo/elmo_3621000 -->

    <owl:Class rdf:about="https://w3id.org/elmo/elmo_3621000">
        <rdfs:subClassOf rdf:resource="http://purl.obolibrary.org/obo/ENVO_01001436"/>
        <obo:IAO_0000115 xml:lang="en">A planned environmental usage process in which fishing equipment is modified for conservation (e.g. bycatch deterrent devices are installed)</obo:IAO_0000115>
        <dcterms:contributor rdf:resource="https://orcid.org/0000-0002-1296-2528"/>
        <rdfs:label xml:lang="en">fishing with equipment modified for conservation</rdfs:label>
    </owl:Class>
    


    <!-- https://w3id.org/elmo/elmo_3621001 -->

    <owl:Class rdf:about="https://w3id.org/elmo/elmo_3621001">
        <rdfs:subClassOf rdf:resource="https://w3id.org/elmo/elmo_3621000"/>
        <obo:IAO_0000115 xml:lang="en">A fishing process in which a human uses a net that has been modified to reduce bycatch or accomplish some other conservation-oriented goal.</obo:IAO_0000115>
        <dcterms:contributor rdf:resource="https://orcid.org/0000-0002-1296-2528"/>
        <rdfs:label xml:lang="en">fishing with net modified for conservation</rdfs:label>
    </owl:Class>
    


    <!-- https://w3id.org/elmo/elmo_3621002 -->

    <owl:Class rdf:about="https://w3id.org/elmo/elmo_3621002">
        <rdfs:subClassOf rdf:resource="https://w3id.org/elmo/elmo_3621000"/>
        <obo:IAO_0000115 xml:lang="en">A fishing process in which a human uses a hook that has been modified for conservation.</obo:IAO_0000115>
        <dcterms:contributor rdf:resource="https://orcid.org/0000-0002-1296-2528"/>
        <rdfs:label xml:lang="en">fishing with hook modified for conservation</rdfs:label>
    </owl:Class>
    


    <!-- https://w3id.org/elmo/elmo_3621003 -->

    <owl:Class rdf:about="https://w3id.org/elmo/elmo_3621003">
        <rdfs:subClassOf rdf:resource="https://w3id.org/elmo/elmo_3621000"/>
        <obo:IAO_0000115 xml:lang="en">A fishing process in which a human adds acoustic devices to fishing gear to deter bycatch.</obo:IAO_0000115>
        <dcterms:contributor rdf:resource="https://orcid.org/0000-0002-1296-2528"/>
        <rdfs:label xml:lang="en">fishing with added acoustic devices for conservation</rdfs:label>
    </owl:Class>
    


    <!-- https://w3id.org/elmo/elmo_3621004 -->

    <owl:Class rdf:about="https://w3id.org/elmo/elmo_3621004">
        <rdfs:subClassOf rdf:resource="https://w3id.org/elmo/elmo_3621000"/>
        <obo:IAO_0000115 xml:lang="en">A fishing process in which a human uses traps modified to deter bycatch.</obo:IAO_0000115>
        <dcterms:contributor rdf:resource="https://orcid.org/0000-0002-1296-2528"/>
        <rdfs:label xml:lang="en">fishing with modified traps</rdfs:label>
    </owl:Class>
    


    <!-- https://w3id.org/elmo/elmo_3621005 -->

    <owl:Class rdf:about="https://w3id.org/elmo/elmo_3621005">
        <rdfs:subClassOf rdf:resource="https://w3id.org/elmo/elmo_3621000"/>
        <obo:IAO_0000115 xml:lang="en">A fishing process in which a human attaches bait to lines in a way that deters seabird scavenging (i.e. underwater)</obo:IAO_0000115>
        <dcterms:contributor rdf:resource="https://orcid.org/0000-0002-1296-2528"/>
        <rdfs:label xml:lang="en">fishing with modified line-setting procedure</rdfs:label>
    </owl:Class>
    


    <!-- https://w3id.org/elmo/elmo_3621006 -->

    <owl:Class rdf:about="https://w3id.org/elmo/elmo_3621006">
        <rdfs:subClassOf rdf:resource="http://purl.obolibrary.org/obo/ENVO_01001436"/>
        <obo:IAO_0000115 xml:lang="en">A planned environmental usage process in which a human engages in aquaculture with modifications for conservation (e.g. disease control measures)</obo:IAO_0000115>
        <dcterms:contributor rdf:resource="https://orcid.org/0000-0002-1296-2528"/>
        <rdfs:label xml:lang="en">aquaculture process modified for conservation</rdfs:label>
    </owl:Class>
    


    <!-- https://w3id.org/elmo/elmo_3621007 -->

    <owl:Class rdf:about="https://w3id.org/elmo/elmo_3621007">
        <rdfs:subClassOf rdf:resource="http://purl.obolibrary.org/obo/ENVO_01001436"/>
        <obo:IAO_0000115 xml:lang="en">A planned environmental usage process in which a human installs an underwater turbine modified for conservation.</obo:IAO_0000115>
        <dcterms:contributor rdf:resource="https://orcid.org/0000-0002-1296-2528"/>
        <rdfs:label xml:lang="en">underwater turbine modified for conservation</rdfs:label>
    </owl:Class>
    


    <!-- https://w3id.org/elmo/elmo_3621008 -->

    <owl:Class rdf:about="https://w3id.org/elmo/elmo_3621008">
        <rdfs:subClassOf rdf:resource="http://purl.obolibrary.org/obo/ENVO_01001436"/>
        <obo:IAO_0000115 xml:lang="en">A planned environmental usage process in which a human engages in farming with modifications for the conservation of biodiversity.</obo:IAO_0000115>
        <dcterms:contributor rdf:resource="https://orcid.org/0000-0002-1296-2528"/>
        <rdfs:label xml:lang="en">farming process modified for conservation</rdfs:label>
    </owl:Class>
    


    <!-- https://w3id.org/elmo/elmo_3621009 -->

    <owl:Class rdf:about="https://w3id.org/elmo/elmo_3621009">
        <rdfs:subClassOf rdf:resource="https://w3id.org/elmo/elmo_3621008"/>
        <obo:IAO_0000115 xml:lang="en">A farming process modified for conservation in which a human grows two or more crop varities in close proximity to one another.</obo:IAO_0000115>
        <dcterms:contributor rdf:resource="https://orcid.org/0000-0002-1296-2528"/>
        <rdfs:label xml:lang="en">farming with intercropping</rdfs:label>
    </owl:Class>
    <owl:Axiom>
        <owl:annotatedSource rdf:resource="https://w3id.org/elmo/elmo_3621009"/>
        <owl:annotatedProperty rdf:resource="http://purl.obolibrary.org/obo/IAO_0000115"/>
        <owl:annotatedTarget xml:lang="en">A farming process modified for conservation in which a human grows two or more crop varities in close proximity to one another.</owl:annotatedTarget>
        <oboInOwl:hasDbXref rdf:resource="ISBN:9781933395210"/>
    </owl:Axiom>
    


    <!-- https://w3id.org/elmo/elmo_3621010 -->

    <owl:Class rdf:about="https://w3id.org/elmo/elmo_3621010">
        <rdfs:subClassOf rdf:resource="https://w3id.org/elmo/elmo_3621008"/>
        <obo:IAO_0000115 xml:lang="en">A farming process modified for conservation in which a human integrates trees and crops or pasture.</obo:IAO_0000115>
        <dcterms:contributor rdf:resource="https://orcid.org/0000-0002-1296-2528"/>
        <rdfs:label xml:lang="en">agroforestry process</rdfs:label>
    </owl:Class>
    <owl:Axiom>
        <owl:annotatedSource rdf:resource="https://w3id.org/elmo/elmo_3621010"/>
        <owl:annotatedProperty rdf:resource="http://purl.obolibrary.org/obo/IAO_0000115"/>
        <owl:annotatedTarget xml:lang="en">A farming process modified for conservation in which a human integrates trees and crops or pasture.</owl:annotatedTarget>
        <oboInOwl:hasDbXref rdf:resource="wd:Q397350"/>
    </owl:Axiom>
    


    <!-- https://w3id.org/elmo/elmo_3621011 -->

    <owl:Class rdf:about="https://w3id.org/elmo/elmo_3621011">
        <rdfs:subClassOf rdf:resource="https://w3id.org/elmo/elmo_3621010"/>
        <obo:IAO_0000115 xml:lang="en">An agroforestry process in which crops are grown in between rows of trees and shrubs.</obo:IAO_0000115>
        <dcterms:contributor rdf:resource="https://orcid.org/0000-0002-1296-2528"/>
        <rdfs:label xml:lang="en">alley cropping farming process</rdfs:label>
    </owl:Class>
    <owl:Axiom>
        <owl:annotatedSource rdf:resource="https://w3id.org/elmo/elmo_3621011"/>
        <owl:annotatedProperty rdf:resource="http://purl.obolibrary.org/obo/IAO_0000115"/>
        <owl:annotatedTarget xml:lang="en">An agroforestry process in which crops are grown in between rows of trees and shrubs.</owl:annotatedTarget>
        <oboInOwl:hasDbXref rdf:resource="ISBN:9781933395210"/>
    </owl:Axiom>
    


    <!-- https://w3id.org/elmo/elmo_3621012 -->

    <owl:Class rdf:about="https://w3id.org/elmo/elmo_3621012">
        <rdfs:subClassOf rdf:resource="https://w3id.org/elmo/elmo_3621008"/>
        <obo:IAO_0000115 xml:lang="en">A farming process modified for conservation in which a human does not disturb the soil in between crop plantings.</obo:IAO_0000115>
        <dcterms:contributor rdf:resource="https://orcid.org/0000-0002-1296-2528"/>
        <rdfs:label xml:lang="en">no-till farming</rdfs:label>
    </owl:Class>
    <owl:Axiom>
        <owl:annotatedSource rdf:resource="https://w3id.org/elmo/elmo_3621012"/>
        <owl:annotatedProperty rdf:resource="http://purl.obolibrary.org/obo/IAO_0000115"/>
        <owl:annotatedTarget xml:lang="en">A farming process modified for conservation in which a human does not disturb the soil in between crop plantings.</owl:annotatedTarget>
        <oboInOwl:hasDbXref rdf:resource="wd:Q1227672"/>
    </owl:Axiom>
    


    <!-- https://w3id.org/elmo/elmo_3621013 -->

    <owl:Class rdf:about="https://w3id.org/elmo/elmo_3621013">
        <rdfs:subClassOf rdf:resource="https://w3id.org/elmo/elmo_3621008"/>
        <obo:IAO_0000115 xml:lang="en">A farming process modified for conservation in which a human avoids synthetic or chemical inputs in the farming process. The definition of organic is often the subject of government regulation.</obo:IAO_0000115>
        <dcterms:contributor rdf:resource="https://orcid.org/0000-0002-1296-2528"/>
        <rdfs:label xml:lang="en">organic farming regime</rdfs:label>
    </owl:Class>
    <owl:Axiom>
        <owl:annotatedSource rdf:resource="https://w3id.org/elmo/elmo_3621013"/>
        <owl:annotatedProperty rdf:resource="http://purl.obolibrary.org/obo/IAO_0000115"/>
        <owl:annotatedTarget xml:lang="en">A farming process modified for conservation in which a human avoids synthetic or chemical inputs in the farming process. The definition of organic is often the subject of government regulation.</owl:annotatedTarget>
        <oboInOwl:hasDbXref rdf:resource="https://en.wikipedia.org/wiki/Organic_farming"/>
    </owl:Axiom>
    


    <!-- https://w3id.org/elmo/elmo_3621014 -->

    <owl:Class rdf:about="https://w3id.org/elmo/elmo_3621014">
        <rdfs:subClassOf rdf:resource="https://w3id.org/elmo/elmo_3621008"/>
        <obo:IAO_0000115 xml:lang="en">A farming process modified for conservation in which the crop type is rotated year over year.</obo:IAO_0000115>
        <dcterms:contributor rdf:resource="https://orcid.org/0000-0002-1296-2528"/>
        <rdfs:label xml:lang="en">crop rotation</rdfs:label>
    </owl:Class>
    <owl:Axiom>
        <owl:annotatedSource rdf:resource="https://w3id.org/elmo/elmo_3621014"/>
        <owl:annotatedProperty rdf:resource="http://purl.obolibrary.org/obo/IAO_0000115"/>
        <owl:annotatedTarget xml:lang="en">A farming process modified for conservation in which the crop type is rotated year over year.</owl:annotatedTarget>
        <oboInOwl:hasDbXref rdf:resource="ISBN:9781933395210"/>
    </owl:Axiom>
    


    <!-- https://w3id.org/elmo/elmo_3621015 -->

    <owl:Class rdf:about="https://w3id.org/elmo/elmo_3621015">
        <rdfs:subClassOf rdf:resource="https://w3id.org/elmo/elmo_3621008"/>
        <obo:IAO_0000115 xml:lang="en">A farming process modified for conservation in which a human agrees not to farm some portion of a landscape.</obo:IAO_0000115>
        <dcterms:contributor rdf:resource="https://orcid.org/0000-0002-1296-2528"/>
        <rdfs:label xml:lang="en">set aside farmland for conservation</rdfs:label>
    </owl:Class>
    <owl:Axiom>
        <owl:annotatedSource rdf:resource="https://w3id.org/elmo/elmo_3621015"/>
        <owl:annotatedProperty rdf:resource="http://purl.obolibrary.org/obo/IAO_0000115"/>
        <owl:annotatedTarget xml:lang="en">A farming process modified for conservation in which a human agrees not to farm some portion of a landscape.</owl:annotatedTarget>
        <oboInOwl:hasDbXref rdf:resource="https://en.wikipedia.org/wiki/Set-aside"/>
    </owl:Axiom>
    


    <!-- https://w3id.org/elmo/elmo_3621016 -->

    <owl:Class rdf:about="https://w3id.org/elmo/elmo_3621016">
        <rdfs:subClassOf rdf:resource="http://purl.obolibrary.org/obo/ENVO_01001436"/>
        <obo:IAO_0000115 xml:lang="en">A planned environmental usage process in which a human harvests trees in a manner that attempts to ameliorate the impact on the landscape.</obo:IAO_0000115>
        <dcterms:contributor rdf:resource="https://orcid.org/0000-0002-1296-2528"/>
        <rdfs:label xml:lang="en">forestry process modified for conservation</rdfs:label>
    </owl:Class>
    


    <!-- https://w3id.org/elmo/elmo_3621017 -->

    <owl:Class rdf:about="https://w3id.org/elmo/elmo_3621017">
        <rdfs:subClassOf rdf:resource="https://w3id.org/elmo/elmo_3621016"/>
        <obo:IAO_0000115 xml:lang="en">A forestry process in which a human cuts trees down to the stump, allowing the trees to regenerate from the stump.</obo:IAO_0000115>
        <dcterms:contributor rdf:resource="https://orcid.org/0000-0002-1296-2528"/>
        <rdfs:label xml:lang="en">coppice process</rdfs:label>
    </owl:Class>
    <owl:Axiom>
        <owl:annotatedSource rdf:resource="https://w3id.org/elmo/elmo_3621017"/>
        <owl:annotatedProperty rdf:resource="http://purl.obolibrary.org/obo/IAO_0000115"/>
        <owl:annotatedTarget xml:lang="en">A forestry process in which a human cuts trees down to the stump, allowing the trees to regenerate from the stump.</owl:annotatedTarget>
        <oboInOwl:hasDbXref rdf:resource="https://en.wikipedia.org/wiki/Coppicing"/>
    </owl:Axiom>
    


    <!-- https://w3id.org/elmo/elmo_3621018 -->

    <owl:Class rdf:about="https://w3id.org/elmo/elmo_3621018">
        <rdfs:subClassOf rdf:resource="https://w3id.org/elmo/elmo_3621016"/>
        <obo:IAO_0000115 xml:lang="en">A forestry process in which a human harvests trees according to their age with the goal of preserving some overall age for a forest stand.</obo:IAO_0000115>
        <dcterms:contributor rdf:resource="https://orcid.org/0000-0002-1296-2528"/>
        <rdfs:label xml:lang="en">selective harvesting process</rdfs:label>
    </owl:Class>
    <owl:Axiom>
        <owl:annotatedSource rdf:resource="https://w3id.org/elmo/elmo_3621018"/>
        <owl:annotatedProperty rdf:resource="http://purl.obolibrary.org/obo/IAO_0000115"/>
        <owl:annotatedTarget xml:lang="en">A forestry process in which a human harvests trees according to their age with the goal of preserving some overall age for a forest stand.</owl:annotatedTarget>
        <oboInOwl:hasDbXref rdf:resource="https://en.wikipedia.org/wiki/Selection_cutting"/>
    </owl:Axiom>
    


    <!-- https://w3id.org/elmo/elmo_3621019 -->

    <owl:Class rdf:about="https://w3id.org/elmo/elmo_3621019">
        <rdfs:subClassOf rdf:resource="https://w3id.org/elmo/elmo_3621016"/>
        <obo:IAO_0000115 xml:lang="en">A forestry process in which a human removes coarse woody debris after harvesting trees, thereby reducing the risk and intensity of forest fire.</obo:IAO_0000115>
        <dcterms:contributor rdf:resource="https://orcid.org/0000-0002-1296-2528"/>
        <rdfs:label xml:lang="en">woody debris removal process</rdfs:label>
    </owl:Class>
    <owl:Axiom>
        <owl:annotatedSource rdf:resource="https://w3id.org/elmo/elmo_3621019"/>
        <owl:annotatedProperty rdf:resource="http://purl.obolibrary.org/obo/IAO_0000115"/>
        <owl:annotatedTarget xml:lang="en">A forestry process in which a human removes coarse woody debris after harvesting trees, thereby reducing the risk and intensity of forest fire.</owl:annotatedTarget>
        <oboInOwl:hasDbXref rdf:resource="https://en.wikipedia.org/wiki/Coarse_woody_debris"/>
    </owl:Axiom>
    


    <!-- https://w3id.org/elmo/elmo_3621020 -->

    <owl:Class rdf:about="https://w3id.org/elmo/elmo_3621020">
        <rdfs:subClassOf rdf:resource="https://w3id.org/elmo/elmo_3621016"/>
        <obo:IAO_0000115 xml:lang="en">A forestry process in which a human leaves coarse woody debris after harvesting, thereby increasing available resources.</obo:IAO_0000115>
        <dcterms:contributor rdf:resource="https://orcid.org/0000-0002-1296-2528"/>
        <rdfs:label xml:lang="en">leave woody debris</rdfs:label>
    </owl:Class>
    <owl:Axiom>
        <owl:annotatedSource rdf:resource="https://w3id.org/elmo/elmo_3621020"/>
        <owl:annotatedProperty rdf:resource="http://purl.obolibrary.org/obo/IAO_0000115"/>
        <owl:annotatedTarget xml:lang="en">A forestry process in which a human leaves coarse woody debris after harvesting, thereby increasing available resources.</owl:annotatedTarget>
        <oboInOwl:hasDbXref rdf:resource="https://en.wikipedia.org/wiki/Coarse_woody_debris"/>
    </owl:Axiom>
    


    <!-- https://w3id.org/elmo/elmo_3621021 -->

    <owl:Class rdf:about="https://w3id.org/elmo/elmo_3621021">
        <rdfs:subClassOf rdf:resource="https://w3id.org/elmo/elmo_3621016"/>
        <obo:IAO_0000115 xml:lang="en">A forestry process in which a human primarily harvests large trees in order to increase light availability for seedling species.</obo:IAO_0000115>
        <dcterms:contributor rdf:resource="https://orcid.org/0000-0002-1296-2528"/>
        <rdfs:label xml:lang="en">shelterwood cutting process</rdfs:label>
    </owl:Class>
    <owl:Axiom>
        <owl:annotatedSource rdf:resource="https://w3id.org/elmo/elmo_3621021"/>
        <owl:annotatedProperty rdf:resource="http://purl.obolibrary.org/obo/IAO_0000115"/>
        <owl:annotatedTarget xml:lang="en">A forestry process in which a human primarily harvests large trees in order to increase light availability for seedling species.</owl:annotatedTarget>
        <oboInOwl:hasDbXref rdf:resource="https://en.wikipedia.org/wiki/Shelterwood_cutting"/>
    </owl:Axiom>
    


    <!-- https://w3id.org/elmo/elmo_3621022 -->

    <owl:Class rdf:about="https://w3id.org/elmo/elmo_3621022">
        <rdfs:subClassOf rdf:resource="http://purl.obolibrary.org/obo/ENVO_01001436"/>
        <obo:IAO_0000115 xml:lang="en">A planned environmental usage process in which a human modifies the level of wind speed required to spin turbines, thereby preventing avifauna fatalities.</obo:IAO_0000115>
        <dcterms:contributor rdf:resource="https://orcid.org/0000-0002-1296-2528"/>
        <oboInOwl:hasBroadSynonym xml:lang="en">doi:10.1002/2688-8319.12371</oboInOwl:hasBroadSynonym>
        <oboInOwl:hasExactSynonym xml:lang="en">curtailment</oboInOwl:hasExactSynonym>
        <rdfs:label xml:lang="en">regulate wind turbine speed</rdfs:label>
    </owl:Class>
    <owl:Axiom>
        <owl:annotatedSource rdf:resource="https://w3id.org/elmo/elmo_3621022"/>
        <owl:annotatedProperty rdf:resource="http://purl.obolibrary.org/obo/IAO_0000115"/>
        <owl:annotatedTarget xml:lang="en">A planned environmental usage process in which a human modifies the level of wind speed required to spin turbines, thereby preventing avifauna fatalities.</owl:annotatedTarget>
        <oboInOwl:hasDbXref rdf:resource="doi:10.1002/2688-8319.12371"/>
    </owl:Axiom>
    


    <!-- 
    ///////////////////////////////////////////////////////////////////////////////////////
    //
    // Individuals
    //
    ///////////////////////////////////////////////////////////////////////////////////////
     -->

    


    <!-- https://orcid.org/0000-0002-1296-2528 -->

    <owl:NamedIndividual rdf:about="https://orcid.org/0000-0002-1296-2528">
        <dcterms:description>postdoctoral fellow</dcterms:description>
        <rdfs:label>Tim Alamenciak</rdfs:label>
    </owl:NamedIndividual>
    <owl:Axiom>
        <owl:annotatedSource rdf:resource="https://orcid.org/0000-0002-1296-2528"/>
        <owl:annotatedProperty rdf:resource="http://purl.org/dc/terms/description"/>
        <owl:annotatedTarget>postdoctoral fellow</owl:annotatedTarget>
        <dcterms:source rdf:resource="http://www.wikidata.org/entity/Q120766436"/>
    </owl:Axiom>
    <owl:Axiom>
        <owl:annotatedSource rdf:resource="https://orcid.org/0000-0002-1296-2528"/>
        <owl:annotatedProperty rdf:resource="http://www.w3.org/2000/01/rdf-schema#label"/>
        <owl:annotatedTarget>Tim Alamenciak</owl:annotatedTarget>
        <dcterms:source rdf:resource="http://www.wikidata.org/entity/Q120766436"/>
    </owl:Axiom>
    


    <!-- https://orcid.org/0000-0002-4366-3088 -->

    <owl:NamedIndividual rdf:about="https://orcid.org/0000-0002-4366-3088">
        <dcterms:description>researcher</dcterms:description>
        <rdfs:label>Pier Luigi Buttigieg</rdfs:label>
    </owl:NamedIndividual>
    <owl:Axiom>
        <owl:annotatedSource rdf:resource="https://orcid.org/0000-0002-4366-3088"/>
        <owl:annotatedProperty rdf:resource="http://purl.org/dc/terms/description"/>
        <owl:annotatedTarget>researcher</owl:annotatedTarget>
        <dcterms:source rdf:resource="http://www.wikidata.org/entity/Q41566750"/>
    </owl:Axiom>
    <owl:Axiom>
        <owl:annotatedSource rdf:resource="https://orcid.org/0000-0002-4366-3088"/>
        <owl:annotatedProperty rdf:resource="http://www.w3.org/2000/01/rdf-schema#label"/>
        <owl:annotatedTarget>Pier Luigi Buttigieg</owl:annotatedTarget>
        <dcterms:source rdf:resource="http://www.wikidata.org/entity/Q41566750"/>
    </owl:Axiom>
</rdf:RDF>



<!-- Generated by the OWL API (version 4.5.29) https://github.com/owlcs/owlapi -->

